Convert to version with labels

new-semantics/coq/events/Defs.v
@@ -1,20 +1,18 @@
 From Basics Require Import Basics.
 
 Section PreDefs.
-  Variable var : Type.
-  Variable loc : Type.
-  Variable lang : Type.
+  Context {var lbl loc lang : Type}.
 
   (* pre-values *)
   Inductive wvl :=
   | wvl_v (v : vl) (* v *)
-  | wvl_recv (v : vl) (* μ.v *)
+  | wvl_recv (p : lbl) (v : vl) (* μ.v *)
 
   with nv :=
   | nv_mt (* • *)
   | nv_ev (E : vnt) (* [E] *)
   | nv_bloc (x : var) (n : nat) (σ : nv) (* bound location *)
-  | nv_floc (x : var) (ℓ : loc) (σ : nv) (* free location *)
+  | nv_floc (x : var) (ℓ : loc * lbl) (σ : nv) (* free location *)
   | nv_bval (x : var) (w : wvl) (σ : nv) (* bound value *)
 
   with vl :=
@@ -36,31 +34,22 @@ Section PreDefs.
   Combined Scheme pre_val_ind from wvl_ind_mut, nv_ind_mut, vl_ind_mut, vnt_ind_mut.
 End PreDefs.
 
-Arguments wvl_v {var loc lang}.
-Arguments wvl_recv {var loc lang}.
-Arguments nv_mt {var loc lang}.
-Arguments nv_ev {var loc lang}.
-Arguments nv_bloc {var loc lang}.
-Arguments nv_floc {var loc lang}.
-Arguments nv_bval {var loc lang}.
-Arguments vl_exp {var loc lang}.
-Arguments vl_clos {var loc lang}.
-Arguments vl_ev {var loc lang}.
-Arguments Init {var loc lang}.
-Arguments Read {var loc lang}.
-Arguments Call {var loc lang}.
+Arguments wvl : clear implicits.
+Arguments nv : clear implicits.
+Arguments vl : clear implicits.
+Arguments vnt : clear implicits.
 
 (* mutual fixpoints must be defined outside of Section to be simpl'd *)
 (* https://github.com/coq/coq/issues/3488 *)
 
 (* open the bound location i with ℓ *)
-Fixpoint open_loc_wvl {var loc lang} (i : nat) (ℓ : loc) (w : wvl var loc lang) :=
+Fixpoint open_loc_wvl {var lbl loc lang} (i : nat) (ℓ : loc * lbl) (w : wvl var lbl loc lang) :=
   match w with
   | wvl_v v => wvl_v (open_loc_vl i ℓ v)
-  | wvl_recv v => wvl_recv (open_loc_vl (S i) ℓ v)
+  | wvl_recv p v => wvl_recv p (open_loc_vl (S i) ℓ v)
   end
 
-with open_loc_nv {var loc lang} (i : nat) (ℓ : loc) (σ : nv var loc lang) :=
+with open_loc_nv {var lbl loc lang} (i : nat) (ℓ : loc * lbl) (σ : nv var lbl loc lang) :=
   match σ with
   | nv_mt => nv_mt
   | nv_ev E => nv_ev (open_loc_vnt i ℓ E)
@@ -74,14 +63,14 @@ with open_loc_nv {var loc lang} (i : nat) (ℓ : loc) (σ : nv var loc lang) :=
     nv_bval x (open_loc_wvl i ℓ w) (open_loc_nv i ℓ σ')
   end
 
-with open_loc_vl {var loc lang} (i : nat) (ℓ : loc) (v : vl var loc lang) :=
+with open_loc_vl {var lbl loc lang} (i : nat) (ℓ : loc * lbl) (v : vl var lbl loc lang) :=
   match v with
   | vl_ev E => vl_ev (open_loc_vnt i ℓ E)
   | vl_exp σ => vl_exp (open_loc_nv i ℓ σ)
   | vl_clos e σ => vl_clos e (open_loc_nv i ℓ σ)
   end
 
-with open_loc_vnt {var loc lang} (i : nat) (ℓ : loc) (E : vnt var loc lang) :=
+with open_loc_vnt {var lbl loc lang} (i : nat) (ℓ : loc * lbl) (E : vnt var lbl loc lang) :=
   match E with
   | Init => Init
   | Read E x => Read (open_loc_vnt i ℓ E) x
@@ -89,13 +78,13 @@ with open_loc_vnt {var loc lang} (i : nat) (ℓ : loc) (E : vnt var loc lang) :=
   end.
 
 (* close the free location ℓ with the binding depth i *)
-Fixpoint close_wvl {var loc lang} `{Eq loc} (i : nat) (ℓ : loc) (w : wvl var loc lang) :=
+Fixpoint close_wvl {var lbl loc lang} `{Eq lbl} `{Eq loc} (i : nat) (ℓ : loc * lbl) (w : wvl var lbl loc lang) :=
   match w with
   | wvl_v v => wvl_v (close_vl i ℓ v)
-  | wvl_recv v => wvl_recv (close_vl (S i) ℓ v)
+  | wvl_recv p v => wvl_recv p (close_vl (S i) ℓ v)
   end
 
-with close_nv {var loc lang} `{Eq loc} (i : nat) (ℓ : loc) (σ : nv var loc lang) :=
+with close_nv {var lbl loc lang} `{Eq lbl} `{Eq loc} (i : nat) (ℓ : loc * lbl) (σ : nv var lbl loc lang) :=
   match σ with
   | nv_mt => nv_mt
   | nv_ev E => nv_ev (close_vnt i ℓ E)
@@ -109,14 +98,14 @@ with close_nv {var loc lang} `{Eq loc} (i : nat) (ℓ : loc) (σ : nv var loc la
     nv_bval x (close_wvl i ℓ w) (close_nv i ℓ σ')
   end
 
-with close_vl {var loc lang} `{Eq loc} (i : nat) (ℓ : loc) (v : vl var loc lang) :=
+with close_vl {var lbl loc lang} `{Eq lbl} `{Eq loc} (i : nat) (ℓ : loc * lbl) (v : vl var lbl loc lang) :=
   match v with
   | vl_ev E => vl_ev (close_vnt i ℓ E)
   | vl_exp σ => vl_exp (close_nv i ℓ σ)
   | vl_clos e σ => vl_clos e (close_nv i ℓ σ)
   end
 
-with close_vnt {var loc lang} `{Eq loc} (i : nat) (ℓ : loc) (E : vnt var loc lang) :=
+with close_vnt {var lbl loc lang} `{Eq lbl} `{Eq loc} (i : nat) (ℓ : loc * lbl) (E : vnt var lbl loc lang) :=
   match E with
   | Init => Init
   | Read E x => Read (close_vnt i ℓ E) x
@@ -124,13 +113,13 @@ with close_vnt {var loc lang} `{Eq loc} (i : nat) (ℓ : loc) (E : vnt var loc l
   end.
 
 (* open the bound location i with u *)
-Fixpoint open_wvl_wvl {var loc lang} (i : nat) (u : wvl var loc lang) (w : wvl var loc lang) :=
+Fixpoint open_wvl_wvl {var lbl loc lang} (i : nat) (u : wvl var lbl loc lang) (w : wvl var lbl loc lang) :=
   match w with
   | wvl_v v => wvl_v (open_wvl_vl i u v)
-  | wvl_recv v => wvl_recv (open_wvl_vl (S i) u v)
+  | wvl_recv p v => wvl_recv p (open_wvl_vl (S i) u v)
   end
 
-with open_wvl_nv {var loc lang} (i : nat) (u : wvl var loc lang) (σ : nv var loc lang) :=
+with open_wvl_nv {var lbl loc lang} (i : nat) (u : wvl var lbl loc lang) (σ : nv var lbl loc lang) :=
   match σ with
   | nv_mt => nv_mt
   | nv_ev E => nv_ev (open_wvl_vnt i u E)
@@ -144,14 +133,14 @@ with open_wvl_nv {var loc lang} (i : nat) (u : wvl var loc lang) (σ : nv var lo
     nv_bval x (open_wvl_wvl i u w) (open_wvl_nv i u σ')
   end
 
-with open_wvl_vl {var loc lang} (i : nat) (u : wvl var loc lang) (v : vl var loc lang) :=
+with open_wvl_vl {var lbl loc lang} (i : nat) (u : wvl var lbl loc lang) (v : vl var lbl loc lang) :=
   match v with
   | vl_ev E => vl_ev (open_wvl_vnt i u E)
   | vl_exp σ => vl_exp (open_wvl_nv i u σ)
   | vl_clos e σ => vl_clos e (open_wvl_nv i u σ)
   end
 
-with open_wvl_vnt {var loc lang} (i : nat) (u : wvl var loc lang) (E : vnt var loc lang) :=
+with open_wvl_vnt {var lbl loc lang} (i : nat) (u : wvl var lbl loc lang) (E : vnt var lbl loc lang) :=
   match E with
   | Init => Init
   | Read E x => Read (open_wvl_vnt i u E) x
@@ -159,13 +148,13 @@ with open_wvl_vnt {var loc lang} (i : nat) (u : wvl var loc lang) (E : vnt var l
   end.
 
 (* substitute the free location ℓ for ℓ' *)
-Fixpoint subst_loc_wvl {var loc lang} `{Eq loc} (ν ℓ : loc) (w : wvl var loc lang) :=
+Fixpoint subst_loc_wvl {var lbl loc lang} `{Eq lbl} `{Eq loc} (ν ℓ : loc * lbl) (w : wvl var lbl loc lang) :=
   match w with
   | wvl_v v => wvl_v (subst_loc_vl ν ℓ v)
-  | wvl_recv v => wvl_recv (subst_loc_vl ν ℓ v)
+  | wvl_recv p v => wvl_recv p (subst_loc_vl ν ℓ v)
   end
 
-with subst_loc_nv {var loc lang} `{Eq loc} (ν ℓ : loc) (σ : nv var loc lang) :=
+with subst_loc_nv {var lbl loc lang} `{Eq lbl} `{Eq loc} (ν ℓ : loc * lbl) (σ : nv var lbl loc lang) :=
   match σ with
   | nv_mt => nv_mt
   | nv_ev E => nv_ev (subst_loc_vnt ν ℓ E)
@@ -179,14 +168,14 @@ with subst_loc_nv {var loc lang} `{Eq loc} (ν ℓ : loc) (σ : nv var loc lang)
     nv_bval x (subst_loc_wvl ν ℓ w) (subst_loc_nv ν ℓ σ')
   end
 
-with subst_loc_vl {var loc lang} `{Eq loc} (ν ℓ : loc) (v : vl var loc lang) :=
+with subst_loc_vl {var lbl loc lang} `{Eq lbl} `{Eq loc} (ν ℓ : loc * lbl) (v : vl var lbl loc lang) :=
   match v with
   | vl_ev E => vl_ev (subst_loc_vnt ν ℓ E)
   | vl_exp σ => vl_exp (subst_loc_nv ν ℓ σ)
   | vl_clos e σ => vl_clos e (subst_loc_nv ν ℓ σ)
   end
 
-with subst_loc_vnt {var loc lang} `{Eq loc} (ν ℓ : loc) (E : vnt var loc lang) :=
+with subst_loc_vnt {var lbl loc lang} `{Eq lbl} `{Eq loc} (ν ℓ : loc * lbl) (E : vnt var lbl loc lang) :=
   match E with
   | Init => Init
   | Read E x => Read (subst_loc_vnt ν ℓ E) x
@@ -194,32 +183,32 @@ with subst_loc_vnt {var loc lang} `{Eq loc} (ν ℓ : loc) (E : vnt var loc lang
   end.
 
 (* multiple substitutions *)
-Fixpoint map_wvl {var loc lang} (φ : loc -> loc) (w : wvl var loc lang) :=
+Fixpoint map_wvl {var lbl loc lang} (φ : loc -> loc) (w : wvl var lbl loc lang) :=
   match w with
   | wvl_v v => wvl_v (map_vl φ v)
-  | wvl_recv v => wvl_recv (map_vl φ v)
+  | wvl_recv p v => wvl_recv p (map_vl φ v)
   end
 
-with map_nv {var loc lang} (φ : loc-> loc) (σ : nv var loc lang) :=
+with map_nv {var lbl loc lang} (φ : loc -> loc) (σ : nv var lbl loc lang) :=
   match σ with
   | nv_mt => nv_mt
   | nv_ev E => nv_ev (map_vnt φ E)
   | nv_bloc x n σ' =>
     nv_bloc x n (map_nv φ σ')
-  | nv_floc x ℓ' σ' =>
-    nv_floc x (φ ℓ') (map_nv φ σ')
+  | nv_floc x (ℓ', p') σ' =>
+    nv_floc x (φ ℓ', p') (map_nv φ σ')
   | nv_bval x w σ' =>
     nv_bval x (map_wvl φ w) (map_nv φ σ')
   end
 
-with map_vl {var loc lang} (φ : loc -> loc) (v : vl var loc lang) :=
+with map_vl {var lbl loc lang} (φ : loc -> loc) (v : vl var lbl loc lang) :=
   match v with
   | vl_ev E => vl_ev (map_vnt φ E)
   | vl_exp σ => vl_exp (map_nv φ σ)
   | vl_clos e σ => vl_clos e (map_nv φ σ)
   end
 
-with map_vnt {var loc lang} (φ : loc -> loc) (E : vnt var loc lang) :=
+with map_vnt {var lbl loc lang} (φ : loc -> loc) (E : vnt var lbl loc lang) :=
   match E with
   | Init => Init
   | Read E x => Read (map_vnt φ E) x
@@ -227,13 +216,13 @@ with map_vnt {var loc lang} (φ : loc -> loc) (E : vnt var loc lang) :=
   end.
 
 (* substitute the free location ℓ for u *)
-Fixpoint subst_wvl_wvl {var loc lang} `{Eq loc} (u : wvl var loc lang) (ℓ : loc) (w : wvl var loc lang) :=
+Fixpoint subst_wvl_wvl {var lbl loc lang} `{Eq lbl} `{Eq loc} (u : wvl var lbl loc lang) (ℓ : loc * lbl) (w : wvl var lbl loc lang) :=
   match w with
   | wvl_v v => wvl_v (subst_wvl_vl u ℓ v)
-  | wvl_recv v => wvl_recv (subst_wvl_vl u ℓ v)
+  | wvl_recv p v => wvl_recv p (subst_wvl_vl u ℓ v)
   end
 
-with subst_wvl_nv {var loc lang} `{Eq loc} (u : wvl var loc lang) (ℓ : loc) (σ : nv var loc lang) :=
+with subst_wvl_nv {var lbl loc lang} `{Eq lbl} `{Eq loc} (u : wvl var lbl loc lang) (ℓ : loc * lbl) (σ : nv var lbl loc lang) :=
   match σ with
   | nv_mt => nv_mt
   | nv_ev E => nv_ev (subst_wvl_vnt u ℓ E)
@@ -247,14 +236,14 @@ with subst_wvl_nv {var loc lang} `{Eq loc} (u : wvl var loc lang) (ℓ : loc) (�
     nv_bval x (subst_wvl_wvl u ℓ w) (subst_wvl_nv u ℓ σ')
   end
 
-with subst_wvl_vl {var loc lang} `{Eq loc} (u : wvl var loc lang) (ℓ : loc) (v : vl var loc lang) :=
+with subst_wvl_vl {var lbl loc lang} `{Eq lbl} `{Eq loc} (u : wvl var lbl loc lang) (ℓ : loc * lbl) (v : vl var lbl loc lang) :=
   match v with
   | vl_ev E => vl_ev (subst_wvl_vnt u ℓ E)
   | vl_exp σ => vl_exp (subst_wvl_nv u ℓ σ)
   | vl_clos e σ => vl_clos e (subst_wvl_nv u ℓ σ)
   end
 
-with subst_wvl_vnt {var loc lang} `{Eq loc} (u : wvl var loc lang) (ℓ : loc) (E : vnt var loc lang) :=
+with subst_wvl_vnt {var lbl loc lang} `{Eq lbl} `{Eq loc} (u : wvl var lbl loc lang) (ℓ : loc * lbl) (E : vnt var lbl loc lang) :=
   match E with
   | Init => Init
   | Read E x => Read (subst_wvl_vnt u ℓ E) x
@@ -262,57 +251,83 @@ with subst_wvl_vnt {var loc lang} `{Eq loc} (u : wvl var loc lang) (ℓ : loc) (
   end.
 
 (* free locations *)
-Fixpoint floc_wvl {var loc lang} (w : wvl var loc lang) :=
+Fixpoint floc_wvl {var lbl loc lang} (w : wvl var lbl loc lang) :=
   match w with
-  | wvl_v v | wvl_recv v => floc_vl v
+  | wvl_v v | wvl_recv _ v => floc_vl v
   end
 
-with floc_nv {var loc lang} (σ : nv var loc lang) :=
+with floc_nv {var lbl loc lang} (σ : nv var lbl loc lang) :=
   match σ with
   | nv_mt => []
   | nv_ev E => floc_vnt E
   | nv_bloc _ _ σ' => floc_nv σ'
-  | nv_floc _ ℓ σ' => ℓ :: floc_nv σ'
+  | nv_floc _ (ℓ, p) σ' => ℓ :: floc_nv σ'
   | nv_bval _ w σ' => floc_wvl w ++ floc_nv σ'
   end
 
-with floc_vl {var loc lang} (v : vl var loc lang) :=
+with floc_vl {var lbl loc lang} (v : vl var lbl loc lang) :=
   match v with
   | vl_ev E => floc_vnt E
   | vl_exp σ | vl_clos _ σ => floc_nv σ
   end
 
-with floc_vnt {var loc lang} (E : vnt var loc lang) :=
+with floc_vnt {var lbl loc lang} (E : vnt var lbl loc lang) :=
   match E with
   | Init => []
   | Read E x => floc_vnt E
   | Call E v => floc_vnt E ++ floc_vl v
   end.
 
-Section LCDefs.
-  Variable var : Type.
-  Variable loc : Type.
-  Variable lang : Type.
-  
-  (* locally closed predicates *)
-  Inductive wvalue : wvl var loc lang -> Prop :=
-  | wvalue_v v (VAL : value v) : wvalue (wvl_v v)
-  | wvalue_recv L v
-    (VAL : forall ℓ, ~ In ℓ L -> value (open_loc_vl 0 ℓ v))
-  : wvalue (wvl_recv v)
+(* free labelled locations *)
+Fixpoint flloc_wvl {var lbl loc lang} (w : wvl var lbl loc lang) :=
+  match w with
+  | wvl_v v | wvl_recv _ v => flloc_vl v
+  end
 
-  with env : nv var loc lang -> Prop :=
+with flloc_nv {var lbl loc lang} (σ : nv var lbl loc lang) :=
+  match σ with
+  | nv_mt => []
+  | nv_ev E => flloc_vnt E
+  | nv_bloc _ _ σ' => flloc_nv σ'
+  | nv_floc _ ℓ σ' => ℓ :: flloc_nv σ'
+  | nv_bval _ w σ' => flloc_wvl w ++ flloc_nv σ'
+  end
+
+with flloc_vl {var lbl loc lang} (v : vl var lbl loc lang) :=
+  match v with
+  | vl_ev E => flloc_vnt E
+  | vl_exp σ | vl_clos _ σ => flloc_nv σ
+  end
+
+with flloc_vnt {var lbl loc lang} (E : vnt var lbl loc lang) :=
+  match E with
+  | Init => []
+  | Read E x => flloc_vnt E
+  | Call E v => flloc_vnt E ++ flloc_vl v
+  end.
+
+Section LCDefs.
+  Context {var lbl loc lang : Type}.
+ 
+  (* locally closed predicates *)
+  Inductive wvalue : wvl var lbl loc lang -> Prop :=
+  | wvalue_v v (VAL : value v) : wvalue (wvl_v v)
+  | wvalue_recv L p v
+    (VAL : forall ℓ, ~ In ℓ L -> value (open_loc_vl 0 (ℓ, p) v))
+  : wvalue (wvl_recv p v)
+
+  with env : nv var lbl loc lang -> Prop :=
   | env_mt : env nv_mt
   | env_ev E (EVENT : event E) : env (nv_ev E)
   | env_floc x ℓ σ (ENV : env σ) : env (nv_floc x ℓ σ)
   | env_bval x w σ (WVALUE : wvalue w) (ENV : env σ) : env (nv_bval x w σ)
 
-  with value : vl var loc lang -> Prop :=
+  with value : vl var lbl loc lang -> Prop :=
   | value_ev E (EVENT : event E) : value (vl_ev E)
   | value_exp σ (ENV : env σ) : value (vl_exp σ)
   | value_clos e σ (ENV : env σ) : value (vl_clos e σ)
 
-  with event : vnt var loc lang -> Prop :=
+  with event : vnt var lbl loc lang -> Prop :=
   | event_Init : event Init
   | event_Read E x (EVENT : event E) : event (Read E x)
   | event_Call E v (EVENT : event E) (VAL : value v) : event (Call E v)
@@ -325,23 +340,6 @@ Section LCDefs.
 
   Combined Scheme val_ind from wvalue_ind_mut, env_ind_mut, value_ind_mut, event_ind_mut.
 End LCDefs.
-
-Arguments wvalue {var loc lang}.
-Arguments wvalue_v {var loc lang}.
-Arguments wvalue_recv {var loc lang}.
-Arguments env {var loc lang}.
-Arguments env_ev {var loc lang}.
-Arguments env_mt {var loc lang}.
-Arguments env_floc {var loc lang}.
-Arguments env_bval {var loc lang}.
-Arguments value {var loc lang}.
-Arguments value_ev {var loc lang}.
-Arguments value_exp {var loc lang}.
-Arguments value_clos {var loc lang}.
-Arguments event {var loc lang}.
-Arguments event_Init {var loc lang}.
-Arguments event_Read {var loc lang}.
-Arguments event_Call {var loc lang}.
 
 Definition update {loc T} `{Eq loc} (f : loc -> option T) ℓ ℓ' ℓ_param :=
   if eqb ℓ ℓ_param then Some ℓ' else f ℓ_param.
