new-semantics/coq/events/EnvSemantics.v
@@ -3,13 +3,13 @@ From With_events Require Import Defs.
 From With_events Require Import Syntax.
 From With_events Require Import SubstFacts.
 
-Variant read_env_res {var loc lang} :=
+Variant read_env_res {var lbl loc lang} :=
   | Env_err
-  | Env_loc (ℓ : loc)
-  | Env_wvl (w : wvl var loc lang)
+  | Env_loc (ℓ : loc * lbl)
+  | Env_wvl (w : wvl var lbl loc lang)
 .
 
-Fixpoint read_env {var loc lang} `{Eq var} (σ : nv var loc lang) (x : var) :=
+Fixpoint read_env {var lbl loc lang} `{Eq var} (σ : nv var lbl loc lang) (x : var) :=
   match σ with
   | nv_mt | nv_bloc _ _ _ => Env_err
   | nv_ev E => Env_wvl (wvl_v (vl_ev (Read E x)))
@@ -19,45 +19,51 @@ Fixpoint read_env {var loc lang} `{Eq var} (σ : nv var loc lang) (x : var) :=
     if eqb x x' then Env_wvl w else read_env σ' x
   end.
 
-Inductive eval {var loc} `{Eq var} `{Eq loc} (σ : nv var loc (@val var)): tm -> (vl var loc val) -> Prop :=
-| ev_id x v (READ : read_env σ x = Env_wvl (wvl_v v))
-: eval σ (tm_var x) v
-| ev_rec x v (READ : read_env σ x = Env_wvl (wvl_recv v))
-: eval σ (tm_var x) (open_wvl_vl 0 (wvl_recv v) v)
-| ev_fn x t
-: eval σ (tm_lam x t) (vl_clos (v_fn x t) σ)
-| ev_app t1 t2 x e σ1 v2 v
+Definition get_lbl {var lbl} (t : @tm var lbl) :=
+  match t with
+  | tm_var p _ | tm_lam p _ _ | tm_app p _ _ | tm_link p _ _ | tm_mt p | tm_bind p _ _ _ => p
+  end.
+
+Inductive eval {var lbl loc} `{Eq var} `{Eq lbl} `{Eq loc}
+  (σ : nv var lbl loc (@val var lbl)): tm -> (vl var lbl loc val) -> Prop :=
+| ev_id p x v (READ : read_env σ x = Env_wvl (wvl_v v))
+: eval σ (tm_var p x) v
+| ev_rec p x p' v (READ : read_env σ x = Env_wvl (wvl_recv p' v))
+: eval σ (tm_var p x) (open_wvl_vl 0 (wvl_recv p' v) v)
+| ev_fn p x t
+: eval σ (tm_lam p x t) (vl_clos (v_fn x t) σ)
+| ev_app p t1 t2 x e σ1 v2 v
   (FN : eval σ t1 (vl_clos (v_fn x e) σ1))
   (ARG : eval σ t2 v2)
   (BODY : eval (nv_bval x (wvl_v v2) σ1) e v)
-: eval σ (tm_app t1 t2) v
-| ev_appevent t1 t2 E1 v2
+: eval σ (tm_app p t1 t2) v
+| ev_appevent p t1 t2 E1 v2
   (FN : eval σ t1 (vl_ev E1))
   (ARG : eval σ t2 v2)
-: eval σ (tm_app t1 t2) (vl_ev (Call E1 v2))
-| ev_link t1 t2 σ1 v
+: eval σ (tm_app p t1 t2) (vl_ev (Call E1 v2))
+| ev_link p t1 t2 σ1 v
   (MOD : eval σ t1 (vl_exp σ1))
   (IMP : eval σ1 t2 v)
-: eval σ (tm_link t1 t2) v
-| ev_linkevent t1 t2 E1 v
+: eval σ (tm_link p t1 t2) v
+| ev_linkevent p t1 t2 E1 v
   (MOD : eval σ t1 (vl_ev E1))
   (IMP : eval (nv_ev E1) t2 v)
-: eval σ (tm_link t1 t2) v
-| ev_mt
-: eval σ tm_mt (vl_exp nv_mt)
-| ev_bind x t1 t2 ℓ v1 σ2
+: eval σ (tm_link p t1 t2) v
+| ev_mt p
+: eval σ (tm_mt p) (vl_exp nv_mt)
+| ev_bind p x t1 t2 ℓ v1 σ2
   (FRESH : ~ In ℓ (floc_nv σ))
-  (BIND : eval (nv_floc x ℓ σ) t1 v1)
-  (MOD : eval (nv_bval x (wvl_recv (close_vl 0 ℓ v1)) σ) t2 (vl_exp σ2))
-: eval σ (tm_bind x t1 t2) (vl_exp (nv_bval x (wvl_recv (close_vl 0 ℓ v1)) σ2))
-| ev_bindevent x t1 t2 ℓ v1 E2
+  (BIND : eval (nv_floc x (ℓ, get_lbl t1) σ) t1 v1)
+  (MOD : eval (nv_bval x (wvl_recv (get_lbl t1) (close_vl 0 (ℓ, get_lbl t1) v1)) σ) t2 (vl_exp σ2))
+: eval σ (tm_bind p x t1 t2) (vl_exp (nv_bval x (wvl_recv (get_lbl t1) (close_vl 0 (ℓ, get_lbl t1) v1)) σ2))
+| ev_bindevent p x t1 t2 ℓ v1 E2
   (FRESH : ~ In ℓ (floc_nv σ))
-  (BIND : eval (nv_floc x ℓ σ) t1 v1)
-  (MOD : eval (nv_bval x (wvl_recv (close_vl 0 ℓ v1)) σ) t2 (vl_ev E2))
-: eval σ (tm_bind x t1 t2) (vl_exp (nv_bval x (wvl_recv (close_vl 0 ℓ v1)) (nv_ev E2)))
+  (BIND : eval (nv_floc x (ℓ, get_lbl t1) σ) t1 v1)
+  (MOD : eval (nv_bval x (wvl_recv (get_lbl t1) (close_vl 0 (ℓ, get_lbl t1) v1)) σ) t2 (vl_ev E2))
+: eval σ (tm_bind p x t1 t2) (vl_exp (nv_bval x (wvl_recv (get_lbl t1) (close_vl 0 (ℓ, get_lbl t1) v1)) (nv_ev E2)))
 .
 
-Lemma read_env_lc {var loc lang} `{Eq var} (σ : nv var loc lang) (Σ : env σ) :
+Lemma read_env_lc {var lbl loc lang} `{Eq var} (σ : nv var lbl loc lang) (Σ : env σ) :
   forall x w (READ : read_env σ x = Env_wvl w), wvalue w.
 Proof.
   induction σ; ii; ss;
@@ -65,7 +71,7 @@ Proof.
   eqb2eq var; clarify; eauto.
 Qed.
 
-Lemma eval_lc {var loc} `{Eq var} `{Name loc} t (σ : nv var loc (@val var)) v (EVAL : eval σ t v) :
+Lemma eval_lc {var lbl loc} `{Eq var} `{Eq lbl} `{Name loc} t (σ : nv var lbl loc (@val var lbl)) v (EVAL : eval σ t v) :
   forall (LC : env σ), value v.
 Proof.
   induction EVAL; ii; ss; eauto.
@@ -73,7 +79,7 @@ Proof.
   - eapply read_env_lc in READ; eauto.
     inversion READ; clarify.
     gensym_tac (L ++ floc_vl v) ν.
-    assert (subst_intro_vl _ _ _ v) by eapply subst_intro.
+    assert (subst_intro_vl v) by eapply subst_intro.
     rw; eauto.
     eapply subst_wvl_lc; eauto.
   - econstructor. auto.
@@ -88,22 +94,22 @@ Proof.
   - apply IHEVAL2. exploit IHEVAL1; eauto.
     intros LC'. inv LC'. econstructor; eauto.
   - repeat constructor.
-  - assert (wvalue (wvl_recv (close_vl 0 ℓ v1))).
+  - assert (wvalue (wvl_recv (get_lbl t1) (close_vl 0 (ℓ, get_lbl t1) v1))).
     econstructor. instantiate (1 := []). ii.
-    assert (close_open_loc_eq_vl _ _ _ v1) by eapply close_open_loc_eq; rw.
+    assert (close_open_loc_eq_vl v1) by eapply close_open_loc_eq; rw.
     exploit IHEVAL1; eauto. constructor; auto. intros VAL1.
-    assert (open_loc_lc_vl _ _ _ v1 VAL1) by (eapply open_loc_lc; auto).
+    assert (open_loc_lc_vl v1 VAL1) by (eapply open_loc_lc; auto).
     rw.
     eapply subst_loc_lc. auto.
     repeat constructor; eauto.
     exploit IHEVAL2.
     constructor; auto.
     intros VAL. inv VAL. auto.
-  - assert (wvalue (wvl_recv (close_vl 0 ℓ v1))).
+  - assert (wvalue (wvl_recv (get_lbl t1) (close_vl 0 (ℓ, get_lbl t1) v1))).
     econstructor. instantiate (1 := []). ii.
-    assert (close_open_loc_eq_vl _ _ _ v1) by eapply close_open_loc_eq; rw.
+    assert (close_open_loc_eq_vl v1) by eapply close_open_loc_eq; rw.
     exploit IHEVAL1; eauto. constructor; auto. intros VAL1.
-    assert (open_loc_lc_vl _ _ _ v1 VAL1) by (eapply open_loc_lc; auto).
+    assert (open_loc_lc_vl v1 VAL1) by (eapply open_loc_lc; auto).
     rw.
     eapply subst_loc_lc. auto.
     repeat constructor; eauto.
@@ -112,7 +118,7 @@ Proof.
     intros VAL. inv VAL. auto.
 Qed.
 
-Lemma read_env_map {var loc lang} `{Eq var} `{Eq loc} (σ : nv var loc lang) :
+Lemma read_env_map {var lbl loc lang} `{Eq var} `{Eq lbl} `{Eq loc} (σ : nv var lbl loc lang) :
   forall φ w x (READ : read_env σ x = Env_wvl w),
     read_env (map_nv φ σ) x = Env_wvl (map_wvl φ w).
 Proof.
@@ -122,7 +128,7 @@ Proof.
   try eqb2eq loc; clarify; eauto.
 Qed.
 
-Lemma read_env_subst_loc {var loc lang} `{Eq var} `{Eq loc} (σ : nv var loc lang) x :
+Lemma read_env_subst_loc {var lbl loc lang} `{Eq var} `{Eq lbl} `{Eq loc} (σ : nv var lbl loc lang) x :
  forall r ν ℓ (READ : read_env σ x = r),
     read_env (subst_loc_nv ν ℓ σ) x =
     match r with
@@ -134,12 +140,14 @@ Lemma read_env_subst_loc {var loc lang} `{Eq var} `{Eq loc} (σ : nv var loc lan
     end.
 Proof.
   induction σ; ii; ss;
-  des_ifs; ss;
-  des_ifs; exploit IHσ; eauto;
-  ss; repeat rw; eauto.
+  repeat des_goal; repeat des_hyp;
+  repeat first [eqb2eq var | eqb2eq loc | eqb2eq lbl]; clarify;
+  erewrite IHσ; eauto; ss;
+  repeat rewrite eqb_refl; ss;
+  des_goal; repeat first [eqb2eq loc | eqb2eq lbl]; clarify.
 Qed.
 
-Lemma read_env_subst_wvl {var loc lang} `{Eq var} `{Eq loc} (σ : nv var loc lang) x :
+Lemma read_env_subst_wvl {var lbl loc lang} `{Eq var} `{Eq lbl} `{Eq loc} (σ : nv var lbl loc lang) x :
   forall r w ℓ (READ : read_env σ x = r),
     read_env (subst_wvl_nv w ℓ σ) x =
     match r with
@@ -151,13 +159,24 @@ Lemma read_env_subst_wvl {var loc lang} `{Eq var} `{Eq loc} (σ : nv var loc lan
     end.
 Proof.
   induction σ; ii; ss;
-  des_ifs; ss;
-  des_ifs; exploit IHσ; eauto;
-  ss; repeat rw; eauto.
+  repeat des_goal; repeat des_hyp;
+  repeat first [eqb2eq var | eqb2eq loc | eqb2eq lbl]; clarify;
+  erewrite IHσ; eauto; ss;
+  repeat rewrite eqb_refl; ss;
+  des_goal; repeat first [eqb2eq loc | eqb2eq lbl]; clarify.
 Qed.
 
+Lemma read_env_flloc {var lbl loc lang} `{Eq var} `{Eq lbl} `{Eq loc} (σ : nv var lbl loc lang) :
+  forall w ℓ x (READ : read_env σ x = Env_wvl w) (IN : In ℓ (flloc_wvl w)),
+    In ℓ (flloc_nv σ).
+Proof.
+  induction σ; ii; ss;
+  des_ifs; ss;
+  eqb2eq var; clarify; eauto;
+  rewrite in_app_iff; eauto.
+Qed.
 
-Lemma read_env_floc {var loc lang} `{Eq var} `{Eq loc} (σ : nv var loc lang) :
+Lemma read_env_floc {var lbl loc lang} `{Eq var} `{Eq lbl} `{Eq loc} (σ : nv var lbl loc lang) :
   forall w ℓ x (READ : read_env σ x = Env_wvl w) (IN : In ℓ (floc_wvl w)),
     In ℓ (floc_nv σ).
 Proof.
@@ -167,51 +186,68 @@ Proof.
   rewrite in_app_iff; eauto.
 Qed.
 
-Lemma eval_floc_dec {var loc} `{Eq var} `{Eq loc} t (σ : nv var loc (@val var)) v (EVAL : eval σ t v) :
-  forall ℓ (IN : In ℓ (floc_vl v)), In ℓ (floc_nv σ).
+Lemma eval_flloc_dec {var lbl loc} `{Eq var} `{Eq lbl} `{Eq loc} t (σ : nv var lbl loc (@val var lbl)) v (EVAL : eval σ t v) :
+  forall ℓ (IN : In ℓ (flloc_vl v)), In ℓ (flloc_nv σ).
 Proof.
   induction EVAL; ii; ss; eauto.
-  - eapply read_env_floc; eauto.
-  - eapply open_wvl_floc in IN.
-    ss; des; eapply read_env_floc; eauto.
+  - eapply read_env_flloc; eauto.
+  - eapply open_wvl_flloc in IN.
+    ss; des; eapply read_env_flloc; eauto.
   - apply IHEVAL3 in IN.
     rewrite in_app_iff in IN; des; auto.
   - rewrite in_app_iff in IN; des; auto.
   - rewrite in_app_iff in *.
     des; eauto.
-    eapply close_floc in IN. des.
-    exploit IHEVAL1; eauto. ii; des; clarify.
+    eapply close_flloc in IN. des; ss.
+    exploit IHEVAL1; eauto.
+    ii; des; clarify.
     exploit IHEVAL2; eauto. intros IN'.
     rewrite in_app_iff in *.
     des; eauto.
-    eapply close_floc in IN'. des.
+    eapply close_flloc in IN'. des.
     exploit IHEVAL1; eauto. ii; des; clarify.
   - rewrite in_app_iff in *.
     des; eauto.
-    eapply close_floc in IN. des.
+    eapply close_flloc in IN. des.
     exploit IHEVAL1; eauto. ii; des; clarify.
     exploit IHEVAL2; eauto. intros IN'.
     rewrite in_app_iff in *.
     des; eauto.
-    eapply close_floc in IN'. des.
+    eapply close_flloc in IN'. des.
     exploit IHEVAL1; eauto. ii; des; clarify.
 Qed.
 
-Lemma eval_map {var loc} `{Eq var} `{Name loc} t (σ : nv var loc (@val var)) v (EVAL : eval σ t v) :
+Lemma eval_floc_dec {var lbl loc} `{Eq var} `{Eq lbl} `{Eq loc} t (σ : nv var lbl loc (@val var lbl)) v (EVAL : eval σ t v) :
+  forall ℓ (IN : In ℓ (floc_vl v)), In ℓ (floc_nv σ).
+Proof.
+  intros.
+  assert (trans_floc_vl v) as RR by apply trans_floc.
+  rewrite RR in IN. clear RR.
+  assert (trans_floc_nv σ) as RR by apply trans_floc.
+  rewrite RR. clear RR.
+  rewrite in_map_iff in IN.
+  destruct IN as [[ℓ' p'] [EQ IN]].
+  ss; clarify.
+  rewrite in_map_iff.
+  exists (ℓ, p'). split; auto.
+  eapply eval_flloc_dec; eauto.
+Qed.
+
+Lemma eval_map {var lbl loc} `{Eq var} `{Eq lbl} `{Name loc} t (σ : nv var lbl loc (@val var lbl)) v (EVAL : eval σ t v) :
   forall φ (INJ : oto φ),
     eval (map_nv φ σ) t (map_vl φ v).
 Proof.
   induction EVAL; ii; ss; try solve [econstructor; eauto].
   - econstructor. exploit (read_env_map σ); eauto.
-  - assert (map_open_wvl_vl _ _ _ v) by (eapply map_open_wvl).
+  - assert (map_open_wvl_vl v) by (eapply map_open_wvl).
     rw. eapply ev_rec.
     exploit (read_env_map σ); eauto.
-  - assert (map_close_vl _ _ _ v1) by (eapply map_close).
+  - assert (map_close_vl v1) by (eapply map_close).
     rw; eauto.
     econstructor; eauto.
     red. intros IN. eapply map_floc in IN; eauto.
     rrw; eauto.
-  - assert (map_close_vl _ _ _ v1) by (eapply map_close).
+  - assert (map_close_vl v1) by (eapply map_close).
     rw; eauto.
     eapply ev_bindevent; eauto.
     red. intros IN. eapply map_floc in IN; eauto.
