new-semantics/coq/events/EquivLink.v
@@ -8,8 +8,7 @@ From With_events Require Import LinkDefs.
 From With_events Require Import LinkFacts.
 
 Section EquivLink.
-  Variable var : Type.
-  Variable loc : Type.
+  Context {var lbl loc : Type}.
 
   #[local] Coercion vl_ev : vnt >-> vl.
   #[local] Coercion vl_exp : nv >-> vl.
@@ -17,51 +16,51 @@ Section EquivLink.
 
   (* local coercions were for this definition *)
   (* definition of Linking *)
-  Inductive Link `{Eq loc} `{Eq var} (σ0 : nv var loc (@val var)) :
-    wvl var loc (@val var) -> wvl var loc (@val var) -> Prop :=
-  | Link_Init
-  : Link σ0 Init σ0
-  | Link_Read E x (σ : nv _ _ _) w
-    (LINKσ : Link σ0 (nv_ev E) σ)
+  Inductive link' `{Eq var} `{Eq lbl} `{Eq loc} (σ0 : nv var lbl loc val) :
+    wvl var lbl loc (@val var lbl) -> wvl var lbl loc (@val var lbl) -> Prop :=
+  | link_Init'
+  : link' σ0 Init σ0
+  | link_Read' E x (σ : nv _ _ _ _) w
+    (LINKσ : link' σ0 (nv_ev E) σ)
     (READ : read_env σ x = Env_wvl w)
-  : Link σ0 (Read E x) (unroll w)
-  | Link_CallEval (E : vnt _ _ _) x t σ (v v' v'' : vl _ _ _)
-    (LINKE : Link σ0 E (vl_clos (v_fn x t) σ))
-    (LINKv : Link σ0 v v')
+  : link' σ0 (Read E x) (unroll w)
+  | link_CallEval' (E : vnt _ _ _ _) x t σ (v v' v'' : vl _ _ _ _)
+    (LINKE : link' σ0 E (vl_clos (v_fn x t) σ))
+    (LINKv : link' σ0 v v')
     (EVAL : nv_bval x v' σ ⊢ t ⇓ v'')
-  : Link σ0 (Call E v) v''
-  | Link_CallEvent (E E' : vnt _ _ _) (v v' : vl _ _ _)
-    (LINKE : Link σ0 E E')
-    (LINKv : Link σ0 v v')
-  : Link σ0 (Call E v) (Call E' v')
-  | Link_mt
-  : Link σ0 nv_mt nv_mt
-  | Link_holeEnv (E : vnt _ _ _) (σ : nv _ _ _)
-    (LINKE : Link σ0 E σ)
-  : Link σ0 (nv_ev E) σ
-  | Link_holeEvent (E E' : vnt _ _ _)
-    (LINKE : Link σ0 E E')
-  : Link σ0 (nv_ev E) (nv_ev E')
-  | Link_floc x ℓ (σ σ' : nv _ _ _)
-    (LINKσ : Link σ0 σ σ')
-  : Link σ0 (nv_floc x ℓ σ) (nv_floc x ℓ σ')
-  | Link_bval x w w' (σ σ' : nv _ _ _)
-    (LINKw : Link σ0 w w')
-    (LINKσ : Link σ0 σ σ')
-  : Link σ0 (nv_bval x w σ) (nv_bval x w' σ')
-  | Link_clos e (σ σ' : nv _ _ _)
-    (LINKσ : Link σ0 σ σ')
-  : Link σ0 (vl_clos e σ) (vl_clos e σ')
-  | Link_rec (v v' : vl _ _ _) L
+  : link' σ0 (Call E v) v''
+  | link_CallEvent' (E E' : vnt _ _ _ _) (v v' : vl _ _ _ _)
+    (LINKE : link' σ0 E E')
+    (LINKv : link' σ0 v v')
+  : link' σ0 (Call E v) (Call E' v')
+  | link_mt'
+  : link' σ0 nv_mt nv_mt
+  | link_holeEnv' (E : vnt _ _ _ _) (σ : nv _ _ _ _)
+    (LINKE : link' σ0 E σ)
+  : link' σ0 (nv_ev E) σ
+  | link_holeEvent' (E E' : vnt _ _ _ _)
+    (LINKE : link' σ0 E E')
+  : link' σ0 (nv_ev E) (nv_ev E')
+  | link_floc' x ℓ (σ σ' : nv _ _ _ _)
+    (LINKσ : link' σ0 σ σ')
+  : link' σ0 (nv_floc x ℓ σ) (nv_floc x ℓ σ')
+  | link_bval' x w w' (σ σ' : nv _ _ _ _)
+    (LINKw : link' σ0 w w')
+    (LINKσ : link' σ0 σ σ')
+  : link' σ0 (nv_bval x w σ) (nv_bval x w' σ')
+  | link_clos' e (σ σ' : nv _ _ _ _)
+    (LINKσ : link' σ0 σ σ')
+  : link' σ0 (vl_clos e σ) (vl_clos e σ')
+  | link_rec' p (v v' : vl _ _ _ _) L
     (LINKv : forall ℓ (nIN : ~ In ℓ L),
-      Link σ0 (open_loc_vl 0 ℓ v) (open_loc_vl 0 ℓ v'))
-  : Link σ0 (wvl_recv v) (wvl_recv v')
+      link' σ0 (open_loc_vl 0 (ℓ, p) v) (open_loc_vl 0 (ℓ, p) v'))
+  : link' σ0 (wvl_recv p v) (wvl_recv p v')
   .
 
-  #[local] Lemma equiv_link_l `{Eq var} `{Name loc}
-    (σ0 : nv var loc (@val var)) (Σ0 : env σ0) w w' (LINK : link σ0 w w') :
+  #[local] Lemma equiv_link_l `{Eq var} `{Eq lbl} `{Name loc}
+    (σ0 : nv var lbl loc val) (Σ0 : env σ0) w w' (LINK : link σ0 w w') :
     forall φ (INJ : oto φ),
-      Link (map_nv φ σ0) (map_wvl φ w) (map_wvl φ w').
+      link' (map_nv φ σ0) (map_wvl φ w) (map_wvl φ w').
   Proof.
     induction LINK; ii; ss;
     try solve [econstructor; eauto].
@@ -78,17 +77,18 @@ Section EquivLink.
       eapply linked_lc in LINK2 as V'; eauto.
       inv V. inv V'.
       repeat constructor; eapply map_lc; eauto.
+    - des_goal; ss; econstructor; eauto.
     - econstructor; eauto.
       instantiate (1 := φ ℓ :: floc_nv (map_nv φ σ0) ++ floc_vl (map_vl φ v) ++ floc_vl (map_vl φ v')).
       intros ℓ' nIN. split_nIn.
-      assert (map_close_vl _ _ _ v') by eapply map_close. rw; eauto.
-      assert (close_open_loc_eq_vl _ _ _ (map_vl φ v')) by eapply close_open_loc_eq. rw.
+      assert (map_close_vl v') by eapply map_close. rw; eauto.
+      assert (close_open_loc_eq_vl (map_vl φ v')) by eapply close_open_loc_eq. rw.
       assert (value (map_vl φ v')) as V'.
       { eapply map_lc; eauto. eapply linked_lc in LINK; eauto. inv LINK; auto. }
-      assert (open_loc_lc_vl _ _ _ (map_vl φ v') V') by (eapply open_loc_lc; eauto). rw.
-      set (compose loc (swap id ℓ' (φ ℓ)) φ) as φ'.
+      assert (open_loc_lc_vl (map_vl φ v') V') by (eapply open_loc_lc; eauto). rw.
+      set (swap id ℓ' (φ ℓ) <*> φ) as φ'.
       replace (map_nv φ σ0) with (map_nv φ' σ0).
-      replace (subst_loc_vl ℓ' (φ ℓ) (map_vl φ v')) with (map_vl φ' v').
+      replace (subst_loc_vl (ℓ', p) (φ ℓ, p) (map_vl φ v')) with (map_vl φ' v').
       exploit (IHLINK φ').
       + subst φ'. unfold compose, swap, id.
         ii; ss; des_ifs;
@@ -97,7 +97,7 @@ Section EquivLink.
         | H : φ _ = φ _ |- _ => apply INJ in H
         | _ => clarify
         end.
-      + assert (map_open_loc_vl _ _ _ v) by eapply map_open_loc. rw.
+      + assert (map_open_loc_vl v) by eapply map_open_loc. rw.
         replace (φ' ℓ) with ℓ'.
         replace (map_vl φ v) with (map_vl φ' v). auto.
         * eapply map_ext.
@@ -107,14 +107,27 @@ Section EquivLink.
           exploit INJ; eauto. ii; clarify.
         * subst φ'. unfold compose, swap, id.
           des_ifs; eqb2eq loc; clarify.
-      + assert (swap_is_subst_vl _ _ _ (map_vl φ v')) as RR by eapply swap_is_subst.
+      + assert (swap_is_subst_vl (map_vl φ v')) as RR by eapply swap_is_subst.
         specialize (RR id).
         exploit RR; eauto. unfold oto. auto.
-        instantiate (1 := φ ℓ).
-        replace (map_vl id (map_vl φ v')) with (map_vl φ v') by (symmetry; eapply map_id_is_id).
-        unfold id at 2. unfold id at 2.
-        intro. rrw.
-        subst φ'. symmetry. eapply map_compose.
+        instantiate (1 := p). instantiate (1 := φ ℓ).
+        * intros p' IN.
+          apply link_map with (φ := φ) in LINK; eauto.
+          eapply link_flloc_dec in LINK; eauto. ss; des; des_ifs.
+          apply (in_map fst) in LINK; ss.
+          assert (trans_floc_nv (map_nv φ σ0)) as RR' by apply trans_floc.
+          rewrite <- RR' in LINK. eapply map_floc in LINK; eauto. clarify.
+          assert (map_open_loc_vl v) as RR' by apply map_open_loc.
+          rewrite RR' in LINK.
+          eapply open_loc_flloc in LINK. des; clarify.
+          apply (in_map fst) in LINK; ss.
+          assert (trans_floc_vl (map_vl φ v)) as RR'' by apply trans_floc.
+          rewrite <- RR'' in LINK.
+          eapply map_floc in LINK; eauto. clarify.
+        * replace (map_vl id (map_vl φ v')) with (map_vl φ v') by (symmetry; eapply map_id_is_id).
+          unfold id at 2. unfold id at 2.
+          intro. rrw.
+          subst φ'. symmetry. eapply map_compose.
       + eapply map_ext.
         ii. subst φ'. unfold compose, swap, id.
         des_ifs; eqb2eq loc; clarify.
@@ -122,8 +135,8 @@ Section EquivLink.
         exploit INJ; eauto. ii; clarify.
   Qed.
 
-  #[local] Lemma equiv_link_r `{Eq var} `{Name loc}
-    (σ0 : nv var loc (@val var)) (Σ0 : env σ0) w w' (LINK : Link σ0 w w') :
+  #[local] Lemma equiv_link_r `{Eq var} `{Eq lbl} `{Name loc}
+    (σ0 : nv var lbl loc _) (Σ0 : env σ0) w w' (LINK : link' σ0 w w') :
     link σ0 w w'.
   Proof.
     induction LINK; ii; ss;
@@ -135,16 +148,16 @@ Section EquivLink.
       eapply linked_lc in IHLINK1; eauto.
       inv IHLINK1. inv VAL. auto.
     - gensym_tac (floc_nv σ0 ++ floc_vl v ++ floc_vl v' ++ L) ℓ.
-      assert (close_vl 0 ℓ (open_loc_vl 0 ℓ v') = v') as RR.
-      { assert (open_loc_close_vl _ _ _ v') by eapply open_loc_close.
+      assert (close_vl 0 (ℓ, p) (open_loc_vl 0 (ℓ, p) v') = v') as RR.
+      { assert (open_loc_close_vl v') by eapply open_loc_close.
         rw. eapply close_fresh; eauto. }
       rewrite <- RR.
       eapply link_rec; eauto.
   Qed.
 
-  Lemma equiv_link `{Eq var} `{Name loc}
-    (σ0 : nv var loc (@val var)) (Σ0 : env σ0) w w' :
-    link σ0 w w' <-> Link σ0 w w'.
+  Lemma equiv_link `{Eq var} `{Eq lbl} `{Name loc}
+    (σ0 : nv var lbl loc _) (Σ0 : env σ0) w w' :
+    link σ0 w w' <-> link' σ0 w w'.
   Proof.
     split; intro LINK.
     - replace σ0 with (map_nv id σ0) by eapply map_id_is_id.
@@ -165,8 +178,8 @@ Section EquivLink.
     | L : list _ |- _ => instantiate (1 := L)
     end.
   
-  Lemma Link_lc `{Eq loc} `{Eq var} (σ0 : nv var loc _) (w : wvl var loc _) :
-    forall w' (LINK : Link σ0 w w'), wvalue w.
+  Lemma link_lc' `{Eq var} `{Eq lbl} `{Eq loc} (σ0 : nv var lbl loc _) (w : wvl var lbl loc _) :
+    forall w' (LINK : link' σ0 w w'), wvalue w.
   Proof.
     ii. induction LINK;
     repeat econstructor; des;
@@ -187,21 +200,21 @@ Section EquivLink.
     | L : list _ |- _ => instantiate (1 := L)
     end.
   
-  Lemma Linked_lc `{Name loc} `{Eq var}
-    (σ0 : nv var loc _) (Σ0 : env σ0) (w : wvl var loc _) :
-    forall w' (LINK : Link σ0 w w'), wvalue w'.
+  Lemma linked_lc' `{Eq var} `{Eq lbl} `{Name loc}
+    (σ0 : nv var lbl loc _) (Σ0 : env σ0) (w : wvl var lbl loc _) :
+    forall w' (LINK : link' σ0 w w'), wvalue w'.
   Proof.
     ii. induction LINK;
     repeat econstructor; des;
     Linked_lc_tac; ii.
     - eapply read_env_lc in READ; auto.
       destruct w; inv READ; ss.
-      assert (subst_intro_vl _ _ _ v) by eapply subst_intro.
+      assert (subst_intro_vl v) by eapply subst_intro.
       gensym_tac (L ++ floc_vl v) ℓ.
       rw; eauto.
       eapply subst_wvl_lc; eauto.
       econstructor; eauto.
-    - eapply Eval_lc in EVAL; eauto.
+    - eapply eval_lc' in EVAL; eauto.
       repeat econstructor; eauto.
     - match goal with
       | H : forall _, _ |- _ => exploit H; eauto
@@ -209,10 +222,10 @@ Section EquivLink.
       intro W. inv W. auto.
   Qed.
   
-  Lemma Link_subst_loc `{Name loc} `{Eq var}
-    (σ0 : nv var loc _) (w w' : wvl var loc _) (LINK : Link σ0 w w') :
+  Lemma link_subst_loc' `{Eq var} `{Eq lbl} `{Name loc}
+    (σ0 : nv var lbl loc _) (w w' : wvl var lbl loc _) (LINK : link' σ0 w w') :
     forall ν ℓ',
-      Link (subst_loc_nv ν ℓ' σ0) (subst_loc_wvl ν ℓ' w) (subst_loc_wvl ν ℓ' w').
+      link' (subst_loc_nv ν ℓ' σ0) (subst_loc_wvl ν ℓ' w) (subst_loc_wvl ν ℓ' w').
   Proof.
     induction LINK; ii; ss;
     try solve [econstructor; eauto].
@@ -221,41 +234,41 @@ Section EquivLink.
       erewrite read_env_subst_loc; eauto. ss.
     - specialize (IHLINK1 ν ℓ').
       specialize (IHLINK2 ν ℓ').
-      eapply Link_CallEval; eauto.
-      apply Eval_subst_loc with (ν := ν) (ℓ' := ℓ') in EVAL; eauto.
-    - des_goal; eqb2eq loc; clarify;
+      eapply link_CallEval'; eauto.
+      apply eval_subst_loc' with (ν := ν) (ℓ' := ℓ') in EVAL; eauto.
+    - des_goal; repeat des_hyp; eqb2eq loc; clarify;
       econstructor; eauto.
     - econstructor; eauto.
-      instantiate (1 := ℓ' :: L).
+      instantiate (1 := fst ℓ' :: L).
       intros. split_nIn.
       match goal with
       | H : forall _, _ |- _ => exploit H; eauto
       end.
       instantiate (1 := ℓ'). instantiate (1 := ν).
-      assert (open_loc_subst_loc_vl _ _ _ v) by eapply open_loc_subst_loc. rw.
-      assert (open_loc_subst_loc_vl _ _ _ v') by eapply open_loc_subst_loc. rw.
-      des_goal; eqb2eq loc; clarify.
+      assert (open_loc_subst_loc_vl v) by eapply open_loc_subst_loc. rw.
+      assert (open_loc_subst_loc_vl v') by eapply open_loc_subst_loc. rw.
+      des_goal; ss; repeat des_hyp; eqb2eq loc; clarify.
   Qed.
-  
-  Lemma Link_subst_wvl `{Name loc} `{Eq var}
-    (σ0 : nv var loc _) (Σ0 : env σ0) (w w' : wvl var loc _) (LINK : Link σ0 w w') :
-    forall u u' (LINKu : Link σ0 u u') ℓ' (nIN : ~ In ℓ' (floc_nv σ0)),
-      Link σ0 (subst_wvl_wvl u ℓ' w) (subst_wvl_wvl u' ℓ' w').
+ 
+  Lemma link_subst_wvl' `{Eq var} `{Eq lbl} `{Name loc}
+    (σ0 : nv var lbl loc _) (Σ0 : env σ0) (w w' : wvl var lbl loc _) (LINK : link' σ0 w w') :
+    forall u u' (LINKu : link' σ0 u u') ℓ' p' (nIN : ~ In ℓ' (floc_nv σ0)),
+      link' σ0 (subst_wvl_wvl u (ℓ', p') w) (subst_wvl_wvl u' (ℓ', p') w').
   Proof.
     induction LINK; ii; ss;
     try solve [econstructor; eauto].
-    - assert (subst_wvl_fresh_nv _ _ _ σ0) by eapply subst_wvl_fresh. rw; eauto.
+    - assert (subst_wvl_fresh_nv σ0) by eapply subst_wvl_fresh. rw; eauto.
       econstructor; eauto.
     - rewrite <- subst_wvl_unroll; eauto.
       econstructor; eauto.
       erewrite read_env_subst_wvl; eauto. ss.
-      eapply Linked_lc in LINKu; eauto.
-    - specialize (IHLINK1 u u' LINKu ℓ' nIN).
-      specialize (IHLINK2 u u' LINKu ℓ' nIN).
-      eapply Link_CallEval; eauto.
-      apply Eval_subst_wvl with (u := u') (ℓ' := ℓ') in EVAL; eauto.
-      eapply Linked_lc in LINKu; eauto.
-    - des_goal; eqb2eq loc; clarify;
+      eapply linked_lc' in LINKu; eauto.
+    - specialize (IHLINK1 u u' LINKu ℓ' p' nIN).
+      specialize (IHLINK2 u u' LINKu ℓ' p' nIN).
+      eapply link_CallEval'; eauto.
+      apply eval_subst_wvl' with (u := u') (ℓ' := (ℓ', p')) in EVAL; eauto.
+      eapply linked_lc' in LINKu; eauto.
+    - des_goal; repeat des_hyp; eqb2eq loc; clarify;
       econstructor; eauto.
     - econstructor; eauto.
       instantiate (1 := ℓ' :: floc_wvl u ++ floc_wvl u' ++ L).
@@ -263,14 +276,15 @@ Section EquivLink.
       match goal with
       | H : forall _, _ |- _ => exploit H; eauto
       end.
-      assert (open_loc_subst_wvl_vl _ _ _ v) by (eapply open_loc_subst_wvl; eauto). rw; eauto.
-      assert (open_loc_subst_wvl_vl _ _ _ v') by (eapply open_loc_subst_wvl; eauto). rw; eauto.
-      eapply Linked_lc in LINKu; eauto.
-      eapply Link_lc in LINKu; eauto.
+      assert (open_loc_subst_wvl_vl v) by (eapply open_loc_subst_wvl; eauto). rw; eauto.
+      assert (open_loc_subst_wvl_vl v') by (eapply open_loc_subst_wvl; eauto). rw; eauto.
+      all: try solve [ii; des_ifs; clarify].
+      eapply linked_lc' in LINKu; eauto.
+      eapply link_lc' in LINKu; eauto.
   Qed.
     
-  Lemma Link_vl `{Eq loc} `{Eq var}
-    (σ0 : nv var loc _) (v : vl var loc _) w (LINK : Link σ0 v w) :
+  Lemma link_vl' `{Eq var} `{Eq lbl} `{Eq loc}
+    (σ0 : nv var lbl loc _) (v : vl var lbl loc _) w (LINK : link' σ0 v w) :
     match w with
     | wvl_v _ => True
     | _ => False
@@ -279,12 +293,12 @@ Section EquivLink.
     inv LINK; clarify.
   Qed.
   
-  Lemma Link_read `{Name loc} `{Eq var} (σ0 : nv var loc _) (Σ0 : env σ0) :
-    forall (σ : nv var loc _) (σ' : wvl var loc _) (LINK : Link σ0 σ σ'),
+  Lemma link_read' `{Eq var} `{Eq lbl} `{Name loc} (σ0 : nv var lbl loc _) (Σ0 : env σ0) :
+    forall (σ : nv var lbl loc _) (σ' : wvl var lbl loc _) (LINK : link' σ0 σ σ'),
     match σ' with
     | wvl_v (vl_exp σ') =>
       forall x w' (READ : read_env σ' x = Env_wvl w'),
-        exists w, read_env σ x = Env_wvl w /\ (Link σ0 (unroll w) (unroll w'))
+        exists w, read_env σ x = Env_wvl w /\ (link' σ0 (unroll w) (unroll w'))
     | _ => False
     end.
   Proof.
@@ -297,44 +311,31 @@ Section EquivLink.
     - exists (Read E x).
       split; auto.
       econstructor; eauto.
-      eapply Link_holeEvent; eauto.
+      eapply link_holeEvent'; eauto.
     - ss; des_ifs; eqb2eq var; clarify.
       exploit IHσ; eauto.
     - ss; des_ifs; eqb2eq var; clarify.
       + exists w. split; auto.
         destruct w; ss.
-        * eapply Link_vl in LINKw as HINT.
+        * eapply link_vl' in LINKw as HINT.
           des_hyp; clarify.
         * inv LINKw; ss.
           gensym_tac (L ++ floc_nv σ0 ++ floc_vl v' ++ floc_vl v) ℓ.
-          assert (subst_intro_vl _ _ _ v') by eapply subst_intro.
+          assert (subst_intro_vl v') by eapply subst_intro.
           rw; eauto.
-          assert (subst_intro_vl _ _ _ v) by eapply subst_intro.
+          assert (subst_intro_vl v) by eapply subst_intro.
           rw; eauto.
           repeat match goal with
           | |- context [wvl_v (subst_wvl_vl ?a ?b ?c)] =>
             replace (wvl_v (subst_wvl_vl a b c)) with
               (subst_wvl_wvl a b (wvl_v c)) by reflexivity
           end.
-          eapply Link_subst_wvl; eauto.
+          eapply link_subst_wvl'; eauto.
           econstructor; eauto.
       + exploit IHσ; eauto.
   Qed.
 End EquivLink.
 
-Arguments Link {var loc _ _}.
-Arguments Link_Init {var loc _ _}.
-Arguments Link_Read {var loc _ _}.
-Arguments Link_CallEval {var loc _ _}.
-Arguments Link_CallEvent {var loc _ _}.
-Arguments Link_mt {var loc _ _}.
-Arguments Link_holeEnv {var loc _ _}.
-Arguments Link_holeEvent {var loc _ _}.
-Arguments Link_floc {var loc _ _}.
-Arguments Link_bval {var loc _ _}.
-Arguments Link_clos {var loc _ _}.
-Arguments Link_rec {var loc _ _}.
-
-Notation " σ '⋊' w '∋' v " := (Link σ w v)
+Notation " σ '⋊' w '∋' v " := (link' σ w v)
   (at level 100, w at next level, v at next level, right associativity).
 
