new-semantics/coq/events/EquivSemantics.v
@@ -4,47 +4,48 @@ From With_events Require Import Syntax.
 From With_events Require Import SubstFacts.
 From With_events Require Import EnvSemantics.
 
-Inductive Eval {var loc} `{Eq var} `{Eq loc} (σ : nv var loc (@val var)): tm -> (vl var loc val) -> Prop :=
-| Ev_id x v (READ : read_env σ x = Env_wvl (wvl_v v))
-: Eval σ (tm_var x) v
-| Ev_rec x v (READ : read_env σ x = Env_wvl (wvl_recv v))
-: Eval σ (tm_var x) (open_wvl_vl 0 (wvl_recv v) v)
-| Ev_fn x t
-: Eval σ (tm_lam x t) (vl_clos (v_fn x t) σ)
-| Ev_app t1 t2 x e σ1 v2 v
-  (FN : Eval σ t1 (vl_clos (v_fn x e) σ1))
-  (ARG : Eval σ t2 v2)
-  (BODY : Eval (nv_bval x (wvl_v v2) σ1) e v)
-: Eval σ (tm_app t1 t2) v
-| Ev_appevent t1 t2 E1 v2
-  (FN : Eval σ t1 (vl_ev E1))
-  (ARG : Eval σ t2 v2)
-: Eval σ (tm_app t1 t2) (vl_ev (Call E1 v2))
-| Ev_link t1 t2 σ1 v
-  (MOD : Eval σ t1 (vl_exp σ1))
-  (IMP : Eval σ1 t2 v)
-: Eval σ (tm_link t1 t2) v
-| Ev_linkevent t1 t2 E1 v
-  (MOD : Eval σ t1 (vl_ev E1))
-  (IMP : Eval (nv_ev E1) t2 v)
-: Eval σ (tm_link t1 t2) v
-| Ev_mt
-: Eval σ tm_mt (vl_exp nv_mt)
-| Ev_bind x t1 t2 L v1 σ2
+Inductive eval' {var lbl loc} `{Eq var} `{Eq lbl} `{Eq loc}
+  (σ : nv var lbl loc (@val var lbl)): tm -> (vl var lbl loc val) -> Prop :=
+| ev_id' p x v (READ : read_env σ x = Env_wvl (wvl_v v))
+: eval' σ (tm_var p x) v
+| ev_rec' p x p' v (READ : read_env σ x = Env_wvl (wvl_recv p' v))
+: eval' σ (tm_var p x) (open_wvl_vl 0 (wvl_recv p' v) v)
+| ev_fn' p x t
+: eval' σ (tm_lam p x t) (vl_clos (v_fn x t) σ)
+| ev_app' p t1 t2 x e σ1 v2 v
+  (FN : eval' σ t1 (vl_clos (v_fn x e) σ1))
+  (ARG : eval' σ t2 v2)
+  (BODY : eval' (nv_bval x (wvl_v v2) σ1) e v)
+: eval' σ (tm_app p t1 t2) v
+| ev_appevent' p t1 t2 E1 v2
+  (FN : eval' σ t1 (vl_ev E1))
+  (ARG : eval' σ t2 v2)
+: eval' σ (tm_app p t1 t2) (vl_ev (Call E1 v2))
+| ev_link' p t1 t2 σ1 v
+  (MOD : eval' σ t1 (vl_exp σ1))
+  (IMP : eval' σ1 t2 v)
+: eval' σ (tm_link p t1 t2) v
+| ev_linkevent' p t1 t2 E1 v
+  (MOD : eval' σ t1 (vl_ev E1))
+  (IMP : eval' (nv_ev E1) t2 v)
+: eval' σ (tm_link p t1 t2) v
+| ev_mt' p
+: eval' σ (tm_mt p) (vl_exp nv_mt)
+| ev_bind' p x t1 t2 L v1 σ2
   (BIND : forall ℓ (nIN : ~ In ℓ L),
-    Eval (nv_floc x ℓ σ) t1 (open_loc_vl 0 ℓ v1))
-  (MOD : Eval (nv_bval x (wvl_recv v1) σ) t2 (vl_exp σ2))
-: Eval σ (tm_bind x t1 t2) (vl_exp (nv_bval x (wvl_recv v1) σ2))
-| Ev_bindevent x t1 t2 L v1 E2
+    eval' (nv_floc x (ℓ, get_lbl t1) σ) t1 (open_loc_vl 0 (ℓ, get_lbl t1) v1))
+  (MOD : eval' (nv_bval x (wvl_recv (get_lbl t1) v1) σ) t2 (vl_exp σ2))
+: eval' σ (tm_bind p x t1 t2) (vl_exp (nv_bval x (wvl_recv (get_lbl t1) v1) σ2))
+| ev_bindevent' p x t1 t2 L v1 E2
   (BIND : forall ℓ (nIN : ~ In ℓ L),
-    Eval (nv_floc x ℓ σ) t1 (open_loc_vl 0 ℓ v1))
-  (MOD : Eval (nv_bval x (wvl_recv v1) σ) t2 (vl_ev E2))
-: Eval σ (tm_bind x t1 t2) (vl_exp (nv_bval x (wvl_recv v1) (nv_ev E2)))
+    eval' (nv_floc x (ℓ, get_lbl t1) σ) t1 (open_loc_vl 0 (ℓ, get_lbl t1) v1))
+  (MOD : eval' (nv_bval x (wvl_recv (get_lbl t1) v1) σ) t2 (vl_ev E2))
+: eval' σ (tm_bind p x t1 t2) (vl_exp (nv_bval x (wvl_recv (get_lbl t1) v1) (nv_ev E2)))
 .
 
-Lemma equiv_l {var loc} `{Eq var} `{Name loc}
-  t (σ : nv var loc (@val var)) (Σ : env σ) v (EVAL : eval σ t v) :
-  forall φ (INJ : oto φ), Eval (map_nv φ σ) t (map_vl φ v).
+Lemma equiv_l {var lbl loc} `{Eq var} `{Eq lbl} `{Name loc}
+  t (σ : nv var lbl loc val) (Σ : env σ) v (EVAL : eval σ t v) :
+  forall φ (INJ : oto φ), eval' (map_nv φ σ) t (map_vl φ v).
 Proof.
   induction EVAL; ii; ss;
   try solve [econstructor; eauto].
@@ -52,9 +53,9 @@ Proof.
     ss. econstructor; eauto.
   - apply read_env_map with (φ := φ) in READ.
     ss. 
-    assert (map_open_wvl_vl _ _ _ v) by eapply map_open_wvl.
+    assert (map_open_wvl_vl v) by eapply map_open_wvl.
     rw.
-    eapply Ev_rec; ss; eauto.
+    eapply ev_rec'; ss; eauto.
   - apply eval_lc in EVAL1 as V1; eauto. inv V1.
     apply eval_lc in EVAL2 as V2; eauto.
     exploit IHEVAL3; eauto. repeat constructor; auto.
@@ -63,32 +64,32 @@ Proof.
     econstructor; eauto.
   - apply eval_lc in EVAL1 as Σ1; eauto. inv Σ1.
     exploit IHEVAL2; eauto. constructor; auto.
-    eapply Ev_linkevent; eauto.
+    eapply ev_linkevent'; eauto.
   - apply eval_lc in EVAL1 as V1; try solve [repeat constructor; auto].
     assert (value (map_vl φ v1)) as V1' by (eapply map_lc; auto).
-    assert (wvalue (wvl_recv (close_vl 0 ℓ v1))) as V1''.
+    assert (wvalue (wvl_recv (get_lbl t1) (close_vl 0 (ℓ, get_lbl t1) v1))) as V1''.
     econstructor. instantiate (1 := []). ii.
-    assert (close_open_loc_eq_vl _ _ _ v1) by eapply close_open_loc_eq. rw.
-    assert (open_loc_lc_vl _ _ _ v1 V1) by (eapply open_loc_lc; eauto). rw.
+    assert (close_open_loc_eq_vl v1) by eapply close_open_loc_eq. rw.
+    assert (open_loc_lc_vl v1 V1) by (eapply open_loc_lc; eauto). rw.
     eapply subst_loc_lc. auto.
     repeat match goal with
     | IH : env ?σ -> _ |- _ =>
       assert (env σ) as Σ' by repeat (constructor; auto);
       specialize (IH Σ'); clear Σ'
     end.
-    eapply Ev_bind; eauto.
+    eapply ev_bind'; eauto.
     instantiate (1 := φ ℓ :: floc_nv (map_nv φ σ)).
     intros ℓ'' nIN. split_nIn.
     assert (~ In ℓ'' (floc_vl (map_vl φ v1))) as HINT.
     { intro. apply eval_map with (φ := φ) in EVAL1; auto.
       eapply eval_floc_dec in EVAL1; eauto. ss. des; ss. }
-    assert (map_close_vl _ _ _ v1) by eapply map_close.
+    assert (map_close_vl v1) by eapply map_close.
     rw; eauto.
-    assert (close_open_loc_eq_vl _ _ _ (map_vl φ v1)) by eapply close_open_loc_eq. rw.
-    assert (open_loc_lc_vl _ _ _ (map_vl φ v1) V1') by (eapply open_loc_lc; eauto). rw.
-    set (compose loc (swap id ℓ'' (φ ℓ)) φ) as φ'.
+    assert (close_open_loc_eq_vl (map_vl φ v1)) by eapply close_open_loc_eq. rw.
+    assert (open_loc_lc_vl (map_vl φ v1) V1') by (eapply open_loc_lc; eauto). rw.
+    set (swap id ℓ'' (φ ℓ) <*> φ) as φ'.
     replace (map_nv φ σ) with (map_nv φ' σ).
-    replace (subst_loc_vl ℓ'' (φ ℓ) (map_vl φ v1)) with (map_vl φ' v1).
+    replace (subst_loc_vl (ℓ'', get_lbl t1) (φ ℓ, get_lbl t1) (map_vl φ v1)) with (map_vl φ' v1).
     exploit (IHEVAL1 φ').
     + subst φ'. unfold compose, swap, id.
       ii; ss; des_ifs;
@@ -100,14 +101,20 @@ Proof.
     + replace (φ' ℓ) with ℓ''; auto.
       subst φ'; unfold compose, swap, id; s.
       des_ifs; eqb2eq loc; clarify.
-    + assert (swap_is_subst_vl _ _ _ (map_vl φ v1)) as RR by eapply swap_is_subst.
+    + assert (swap_is_subst_vl (map_vl φ v1)) as RR by eapply swap_is_subst.
       specialize (RR id).
       exploit RR; eauto. unfold oto. auto.
-      instantiate (1 := φ ℓ).
-      replace (map_vl id (map_vl φ v1)) with (map_vl φ v1) by (symmetry; eapply map_id_is_id).
-      unfold id at 2. unfold id at 2.
-      intro. rrw.
-      subst φ'. symmetry. eapply map_compose. 
+      instantiate (1 := get_lbl t1). instantiate (1 := φ ℓ).
+      * intros p' IN.
+        apply eval_map with (φ := φ) in EVAL1; eauto.
+        eapply eval_flloc_dec in EVAL1; eauto. ss; des; des_ifs.
+        apply (in_map fst) in EVAL1; ss.
+        assert (trans_floc_nv (map_nv φ σ)) as RR' by apply trans_floc.
+        rewrite <- RR' in EVAL1. eapply map_floc in EVAL1; eauto. clarify.
+      * replace (map_vl id (map_vl φ v1)) with (map_vl φ v1) by (symmetry; eapply map_id_is_id).
+        unfold id at 2. unfold id at 2.
+        intro. rrw.
+        subst φ'. symmetry. eapply map_compose.
     + eapply map_ext.
       ii. subst φ'. unfold compose, swap, id.
       des_ifs; eqb2eq loc; clarify.
@@ -115,30 +122,29 @@ Proof.
       exploit INJ; eauto. ii; clarify.
   - apply eval_lc in EVAL1 as V1; try solve [repeat constructor; auto].
     assert (value (map_vl φ v1)) as V1' by (eapply map_lc; auto).
-    assert (wvalue (wvl_recv (close_vl 0 ℓ v1))) as V1''.
+    assert (wvalue (wvl_recv (get_lbl t1) (close_vl 0 (ℓ, get_lbl t1) v1))) as V1''.
     econstructor. instantiate (1 := []). ii.
-    assert (close_open_loc_eq_vl _ _ _ v1) by eapply close_open_loc_eq.
-    rw.
-    assert (open_loc_lc_vl _ _ _ v1 V1) by (eapply open_loc_lc; eauto).
-    rw.
+    assert (close_open_loc_eq_vl v1) by eapply close_open_loc_eq. rw.
+    assert (open_loc_lc_vl v1 V1) by (eapply open_loc_lc; eauto). rw.
     eapply subst_loc_lc. auto.
     repeat match goal with
     | IH : env ?σ -> _ |- _ =>
       assert (env σ) as Σ' by repeat (constructor; auto);
       specialize (IH Σ'); clear Σ'
     end.
-    eapply Ev_bindevent; eauto.
+    eapply ev_bindevent'; eauto.
     instantiate (1 := φ ℓ :: floc_nv (map_nv φ σ)).
     intros ℓ'' nIN. split_nIn.
     assert (~ In ℓ'' (floc_vl (map_vl φ v1))) as HINT.
     { intro. apply eval_map with (φ := φ) in EVAL1; auto.
       eapply eval_floc_dec in EVAL1; eauto. ss. des; ss. }
-    assert (map_close_vl _ _ _ v1) by eapply map_close. rw; eauto.
-    assert (close_open_loc_eq_vl _ _ _ (map_vl φ v1)) by eapply close_open_loc_eq. rw.
-    assert (open_loc_lc_vl _ _ _ (map_vl φ v1) V1') by (eapply open_loc_lc; eauto). rw.
-    set (compose loc (swap id ℓ'' (φ ℓ)) φ) as φ'.
+    assert (map_close_vl v1) by eapply map_close.
+    rw; eauto.
+    assert (close_open_loc_eq_vl (map_vl φ v1)) by eapply close_open_loc_eq. rw.
+    assert (open_loc_lc_vl (map_vl φ v1) V1') by (eapply open_loc_lc; eauto). rw.
+    set (swap id ℓ'' (φ ℓ) <*> φ) as φ'.
     replace (map_nv φ σ) with (map_nv φ' σ).
-    replace (subst_loc_vl ℓ'' (φ ℓ) (map_vl φ v1)) with (map_vl φ' v1).
+    replace (subst_loc_vl (ℓ'', get_lbl t1) (φ ℓ, get_lbl t1) (map_vl φ v1)) with (map_vl φ' v1).
     exploit (IHEVAL1 φ').
     + subst φ'. unfold compose, swap, id.
       ii; ss; des_ifs;
@@ -150,14 +156,20 @@ Proof.
     + replace (φ' ℓ) with ℓ''; auto.
       subst φ'; unfold compose, swap, id; s.
       des_ifs; eqb2eq loc; clarify.
-    + assert (swap_is_subst_vl _ _ _ (map_vl φ v1)) as RR by eapply swap_is_subst.
+    + assert (swap_is_subst_vl (map_vl φ v1)) as RR by eapply swap_is_subst.
       specialize (RR id).
       exploit RR; eauto. unfold oto. auto.
-      instantiate (1 := φ ℓ).
-      replace (map_vl id (map_vl φ v1)) with (map_vl φ v1) by (symmetry; eapply map_id_is_id).
-      unfold id at 2. unfold id at 2.
-      intro. rrw.
-      subst φ'. symmetry. eapply map_compose. 
+      instantiate (1 := get_lbl t1). instantiate (1 := φ ℓ).
+      * intros p' IN.
+        apply eval_map with (φ := φ) in EVAL1; eauto.
+        eapply eval_flloc_dec in EVAL1; eauto. ss; des; des_ifs.
+        apply (in_map fst) in EVAL1; ss.
+        assert (trans_floc_nv (map_nv φ σ)) as RR' by apply trans_floc.
+        rewrite <- RR' in EVAL1. eapply map_floc in EVAL1; eauto. clarify.
+      * replace (map_vl id (map_vl φ v1)) with (map_vl φ v1) by (symmetry; eapply map_id_is_id).
+        unfold id at 2. unfold id at 2.
+        intro. rrw.
+        subst φ'. symmetry. eapply map_compose.
     + eapply map_ext.
       ii. subst φ'. unfold compose, swap, id.
       des_ifs; eqb2eq loc; clarify.
@@ -165,31 +177,31 @@ Proof.
       exploit INJ; eauto. ii; clarify.
 Qed.
 
-Lemma equiv_r {var loc} `{Eq var} `{Name loc}
-  t (σ : nv var loc (@val var)) v (EVAL : Eval σ t v) :
+Lemma equiv_r {var lbl loc} `{Eq var} `{Eq lbl} `{Name loc}
+  t (σ : nv var lbl loc val) v (EVAL : eval' σ t v) :
   eval σ t v.
 Proof.
   induction EVAL; ii; ss;
   try solve [econstructor; eauto].
   - gensym_tac (floc_nv σ ++ floc_vl v1 ++ L) ℓ.
-    assert (close_vl 0 ℓ (open_loc_vl 0 ℓ v1) = v1) as RR.
-    { assert (open_loc_close_vl _ _ _ v1) by eapply open_loc_close.
+    assert (close_vl 0 (ℓ, get_lbl t1) (open_loc_vl 0 (ℓ, get_lbl t1) v1) = v1) as RR.
+    { assert (open_loc_close_vl v1) by eapply open_loc_close.
       rw. eapply close_fresh; eauto. }
     rewrite <- RR.
     eapply ev_bind; eauto.
     rw. auto.
   - gensym_tac (floc_nv σ ++ floc_vl v1 ++ L) ℓ.
-    assert (close_vl 0 ℓ (open_loc_vl 0 ℓ v1) = v1) as RR.
-    { assert (open_loc_close_vl _ _ _ v1) by eapply open_loc_close.
+    assert (close_vl 0 (ℓ, get_lbl t1) (open_loc_vl 0 (ℓ, get_lbl t1) v1) = v1) as RR.
+    { assert (open_loc_close_vl v1) by eapply open_loc_close.
       rw. eapply close_fresh; eauto. }
     rewrite <- RR.
     eapply ev_bindevent; eauto.
     rw. auto.
 Qed.
 
-Lemma equiv_semantics {var loc} `{Eq var} `{Name loc}
-  t (σ : nv var loc (@val var)) (Σ : env σ) v :
-  eval σ t v <-> Eval σ t v.
+Lemma equiv_semantics {var lbl loc} `{Eq var} `{Eq lbl} `{Name loc}
+  t (σ : nv var lbl loc val) (Σ : env σ) v :
+  eval σ t v <-> eval' σ t v.
 Proof.
   split.
   - intro.
@@ -199,7 +211,7 @@ Proof.
   - eapply equiv_r.
 Qed.
 
-Lemma Eval_lc {var loc} `{Eq var} `{Name loc} t (σ : nv var loc (@val var)) v (EVAL : Eval σ t v) :
+Lemma eval_lc' {var lbl loc} `{Eq var} `{Eq lbl} `{Name loc} t (σ : nv var lbl loc val) v (EVAL : eval' σ t v) :
   forall (LC : env σ), value v.
 Proof.
   induction EVAL; ii; ss; eauto.
@@ -207,7 +219,7 @@ Proof.
   - eapply read_env_lc in READ; eauto.
     inversion READ; clarify.
     gensym_tac (L ++ floc_vl v) ν.
-    assert (subst_intro_vl _ _ _ v) by eapply subst_intro.
+    assert (subst_intro_vl v) by eapply subst_intro.
     rw; eauto.
     eapply subst_wvl_lc; eauto.
   - econstructor. auto.
@@ -222,10 +234,10 @@ Proof.
   - apply IHEVAL2. exploit IHEVAL1; eauto.
     intros LC'. inv LC'. econstructor; eauto.
   - repeat constructor.
-  - assert (wvalue (wvl_recv v1)).
+  - assert (wvalue (wvl_recv (get_lbl t1) v1)).
     + econstructor. instantiate (1 := L).
       intros.
-      assert (env (nv_floc x ℓ σ)).
+      assert (env (nv_floc x (ℓ, get_lbl t1) σ)).
       repeat (econstructor; eauto).
       auto.
     + repeat (constructor; auto).
@@ -233,10 +245,10 @@ Proof.
       repeat (constructor; auto).
       intro LC'.
       inv LC'. auto.
-  - assert (wvalue (wvl_recv v1)).
+  - assert (wvalue (wvl_recv (get_lbl t1) v1)).
     + econstructor. instantiate (1 := L).
       intros.
-      assert (env (nv_floc x ℓ σ)).
+      assert (env (nv_floc x (ℓ, get_lbl t1) σ)).
       repeat (econstructor; eauto).
       auto.
     + repeat (constructor; auto).
@@ -246,21 +258,21 @@ Proof.
       inv LC'. auto.
 Qed.
 
-Lemma Eval_subst_loc {var loc} `{Eq var} `{Name loc} t (σ : nv var loc (@val var)) v (EVAL : Eval σ t v) :
-  forall ν ℓ', Eval (subst_loc_nv ν ℓ' σ) t (subst_loc_vl ν ℓ' v).
+Lemma eval_subst_loc' {var lbl loc} `{Eq var} `{Eq lbl} `{Name loc} t (σ : nv var lbl loc val) v (EVAL : eval' σ t v) :
+  forall ν ℓ', eval' (subst_loc_nv ν ℓ' σ) t (subst_loc_vl ν ℓ' v).
 Proof.
   induction EVAL; ii; ss;
   try solve [econstructor; eauto].
   - econstructor 1.
     erewrite read_env_subst_loc; eauto.
     ss.
-  - assert (open_wvl_subst_loc_vl _ _ _ v) by (eapply open_wvl_subst_loc; auto).
+  - assert (open_wvl_subst_loc_vl v) by (eapply open_wvl_subst_loc; auto).
     rw; eauto.
     econstructor 2.
     erewrite read_env_subst_loc; eauto.
     ss.
-  - eapply Ev_bind; eauto.
-    instantiate (1 := ℓ' :: L).
+  - eapply ev_bind'; eauto.
+    instantiate (1 := fst ℓ' :: L).
     ii. split_nIn.
     match goal with
     | IH : forall _, ~ In _ ?L -> _, nIN : ~ In ?ν ?L |- _ =>
@@ -268,11 +280,11 @@ Proof.
     end.
     instantiate (1 := ℓ'). instantiate (1 := ν).
     rewrite <- eqb_neq in nIN.
-    rw.
-    assert (open_loc_subst_loc_vl _ _ _ v1) by eapply open_loc_subst_loc.
-    rw. rw. auto.
-  - eapply Ev_bindevent; eauto.
-    instantiate (1 := ℓ' :: L).
+    destruct ℓ'; ss; rw.
+    assert (open_loc_subst_loc_vl v1) by eapply open_loc_subst_loc.
+    rw. s. rw. auto.
+  - eapply ev_bindevent'; eauto.
+    instantiate (1 := fst ℓ' :: L).
     ii. split_nIn.
     match goal with
     | IH : forall _, ~ In _ ?L -> _, nIN : ~ In ?ν ?L |- _ =>
@@ -280,48 +292,50 @@ Proof.
     end.
     instantiate (1 := ℓ'). instantiate (1 := ν).
     rewrite <- eqb_neq in nIN.
-    rw.
-    assert (open_loc_subst_loc_vl _ _ _ v1) by eapply open_loc_subst_loc.
-    rw. rw. auto.
+    destruct ℓ'; ss; rw.
+    assert (open_loc_subst_loc_vl v1) by eapply open_loc_subst_loc.
+    rw. s. rw. auto.
 Qed.
 
-Lemma Eval_subst_wvl {var loc} `{Eq var} `{Name loc} t (σ : nv var loc (@val var)) v (EVAL : Eval σ t v) :
-  forall u (U : wvalue u) ℓ', Eval (subst_wvl_nv u ℓ' σ) t (subst_wvl_vl u ℓ' v).
+Lemma eval_subst_wvl' {var lbl loc} `{Eq var} `{Eq lbl} `{Name loc} t (σ : nv var lbl loc val) v (EVAL : eval' σ t v) :
+  forall u (U : wvalue u) ℓ', eval' (subst_wvl_nv u ℓ' σ) t (subst_wvl_vl u ℓ' v).
 Proof.
   induction EVAL; ii; ss;
   try solve [econstructor; eauto].
   - econstructor 1.
     erewrite read_env_subst_wvl; eauto.
     ss.
-  - assert (open_wvl_subst_wvl_vl _ _ _ v) by (eapply open_wvl_subst_wvl; auto).
+  - assert (open_wvl_subst_wvl_vl v) by (eapply open_wvl_subst_wvl; auto).
     rw; eauto.
     econstructor 2.
     erewrite read_env_subst_wvl; eauto.
     ss.
-  - eapply Ev_bind; eauto.
-    instantiate (1 := ℓ' :: L).
+  - eapply ev_bind'; eauto.
+    instantiate (1 := fst ℓ' :: L).
     ii. split_nIn.
     match goal with
     | IH : forall _, ~ In _ ?L -> _, nIN : ~ In ?ν ?L |- _ =>
       exploit (IH ν nIN); eauto
     end.
     instantiate (1 := ℓ').
-    des_goal; eqb2eq loc; clarify.
-    assert (open_loc_subst_wvl_vl _ _ _ v1) by (eapply open_loc_subst_wvl; eauto).
-    rw; eauto.
-  - eapply Ev_bindevent; eauto.
-    instantiate (1 := ℓ' :: L).
+    rewrite <- eqb_neq in nIN.
+    destruct ℓ'; ss; rw.
+    assert (open_loc_subst_wvl_vl v1) by (eapply open_loc_subst_wvl; eauto).
+    rw; ii; ss; eqb2eq loc; clarify.
+  - eapply ev_bindevent'; eauto.
+    instantiate (1 := fst ℓ' :: L).
     ii. split_nIn.
     match goal with
     | IH : forall _, ~ In _ ?L -> _, nIN : ~ In ?ν ?L |- _ =>
       exploit (IH ν nIN); eauto
     end.
     instantiate (1 := ℓ').
-    des_goal; eqb2eq loc; clarify.
-    assert (open_loc_subst_wvl_vl _ _ _ v1) by (eapply open_loc_subst_wvl; eauto).
-    rw; eauto.
+    rewrite <- eqb_neq in nIN.
+    destruct ℓ'; ss; rw.
+    assert (open_loc_subst_wvl_vl v1) by (eapply open_loc_subst_wvl; eauto).
+    rw; ii; ss; eqb2eq loc; clarify.
 Qed.
 
-Notation " σ '⊢' t '⇓' v " := (Eval σ t v)
+Notation " σ '⊢' t '⇓' v " := (eval' σ t v)
   (at level 100, t at next level, v at next level, right associativity).
 
