new-semantics/coq/events/LinkDefs.v
@@ -3,15 +3,14 @@ From With_events Require Import Defs.
 From With_events Require Import Syntax.
 From With_events Require Import EnvSemantics.
 
-Definition unroll {var loc lang} (w : wvl var loc lang) :=
+Definition unroll {var lbl loc lang} (w : wvl var lbl loc lang) :=
   match w with
   | wvl_v v => v
-  | wvl_recv v => open_wvl_vl 0 (wvl_recv v) v
+  | wvl_recv p v => open_wvl_vl 0 (wvl_recv p v) v
   end.
 
 Section LinkDefs.
-  Variable var : Type.
-  Variable loc : Type.
+  Context {var lbl loc : Type}.
 
   #[local] Coercion vl_ev : vnt >-> vl.
   #[local] Coercion vl_exp : nv >-> vl.
@@ -19,59 +18,46 @@ Section LinkDefs.
 
   (* local coercions were for this definition *)
   (* definition of linking *)
-  Inductive link `{Eq loc} `{Eq var} (σ0 : nv var loc (@val var)) :
-    wvl var loc (@val var) -> wvl var loc (@val var) -> Prop :=
+  Inductive link `{Eq loc} `{Eq lbl} `{Eq var} (σ0 : nv var lbl loc val) :
+    wvl var lbl loc (@val var lbl) -> wvl var lbl loc (@val var lbl) -> Prop :=
   | link_Init
   : link σ0 Init σ0
-  | link_Read E x (σ : nv _ _ _) w
+  | link_Read E x (σ : nv _ _ _ _) w
     (LINKσ : link σ0 (nv_ev E) σ)
     (READ : read_env σ x = Env_wvl w)
   : link σ0 (Read E x) (unroll w)
-  | link_CallEval (E : vnt _ _ _) x t σ (v v' v'' : vl _ _ _)
+  | link_CallEval (E : vnt _ _ _ _) x t σ (v v' v'' : vl _ _ _ _)
     (LINKE : link σ0 E (vl_clos (v_fn x t) σ))
     (LINKv : link σ0 v v')
     (EVAL : eval (nv_bval x v' σ) t v'')
   : link σ0 (Call E v) v''
-  | link_CallEvent (E E' : vnt _ _ _) (v v' : vl _ _ _)
+  | link_CallEvent (E E' : vnt _ _ _ _) (v v' : vl _ _ _ _)
     (LINKE : link σ0 E E')
     (LINKv : link σ0 v v')
   : link σ0 (Call E v) (Call E' v')
   | link_mt
   : link σ0 nv_mt nv_mt
-  | link_holeEnv (E : vnt _ _ _) (σ : nv _ _ _)
+  | link_holeEnv (E : vnt _ _ _ _) (σ : nv _ _ _ _)
     (LINKE : link σ0 E σ)
   : link σ0 (nv_ev E) σ
-  | link_holeEvent (E E' : vnt _ _ _)
+  | link_holeEvent (E E' : vnt _ _ _ _)
     (LINKE : link σ0 E E')
   : link σ0 (nv_ev E) (nv_ev E')
-  | link_floc x ℓ (σ σ' : nv _ _ _)
+  | link_floc x ℓ (σ σ' : nv _ _ _ _)
     (LINKσ : link σ0 σ σ')
   : link σ0 (nv_floc x ℓ σ) (nv_floc x ℓ σ')
-  | link_bval x w w' (σ σ' : nv _ _ _)
+  | link_bval x w w' (σ σ' : nv _ _ _ _)
     (LINKw : link σ0 w w')
     (LINKσ : link σ0 σ σ')
   : link σ0 (nv_bval x w σ) (nv_bval x w' σ')
-  | link_clos e (σ σ' : nv _ _ _)
+  | link_clos e (σ σ' : nv _ _ _ _)
     (LINKσ : link σ0 σ σ')
   : link σ0 (vl_clos e σ) (vl_clos e σ')
-  | link_rec (v v' : vl _ _ _) ℓ
+  | link_rec p (v v' : vl _ _ _ _) ℓ
     (nInv : ~ In ℓ (floc_vl v))
     (nInσ0 : ~ In ℓ (floc_nv σ0))
-    (LINKv : link σ0 (open_loc_vl 0 ℓ v) v')
-  : link σ0 (wvl_recv v) (wvl_recv (close_vl 0 ℓ v'))
+    (LINKv : link σ0 (open_loc_vl 0 (ℓ, p) v) v')
+  : link σ0 (wvl_recv p v) (wvl_recv p (close_vl 0 (ℓ, p) v'))
   .
 End LinkDefs.
-
-Arguments link {var loc _ _}.
-Arguments link_Init {var loc _ _}.
-Arguments link_Read {var loc _ _}.
-Arguments link_CallEval {var loc _ _}.
-Arguments link_CallEvent {var loc _ _}.
-Arguments link_mt {var loc _ _}.
-Arguments link_holeEnv {var loc _ _}.
-Arguments link_holeEvent {var loc _ _}.
-Arguments link_floc {var loc _ _}.
-Arguments link_bval {var loc _ _}.
-Arguments link_clos {var loc _ _}.
-Arguments link_rec {var loc _ _}.
 
