new-semantics/coq/events/SubstFacts.v
@@ -1,22 +1,21 @@
 From Basics Require Import Basics.
+From Coq.Program Require Export Basics.
 From With_events Require Import Defs.
 
 Section SubstFacts.
-  Variable var : Type.
-  Variable loc : Type.
-  Variable lang : Type.
+  Context {var lbl loc lang : Type}.
 
-  Definition open_floc_wvl (w : wvl var loc lang) :=
-    forall i ℓ x, In x (floc_wvl (open_loc_wvl i ℓ w)) -> x = ℓ \/ In x (floc_wvl w).
+  Definition open_floc_wvl (w : wvl var lbl loc lang) :=
+    forall i ℓ x, In x (floc_wvl (open_loc_wvl i ℓ w)) -> x = fst ℓ \/ In x (floc_wvl w).
 
-  Definition open_floc_nv (σ : nv var loc lang) :=
-    forall i ℓ x, In x (floc_nv (open_loc_nv i ℓ σ)) -> x = ℓ \/ In x (floc_nv σ).
+  Definition open_floc_nv (σ : nv var lbl loc lang) :=
+    forall i ℓ x, In x (floc_nv (open_loc_nv i ℓ σ)) -> x = fst ℓ \/ In x (floc_nv σ).
 
-  Definition open_floc_vl (v : vl var loc lang) :=
-    forall i ℓ x, In x (floc_vl (open_loc_vl i ℓ v)) -> x = ℓ \/ In x (floc_vl v).
+  Definition open_floc_vl (v : vl var lbl loc lang) :=
+    forall i ℓ x, In x (floc_vl (open_loc_vl i ℓ v)) -> x = fst ℓ \/ In x (floc_vl v).
 
-  Definition open_floc_vnt (E : vnt var loc lang) :=
-    forall i ℓ x, In x (floc_vnt (open_loc_vnt i ℓ E)) -> x = ℓ \/ In x (floc_vnt E).
+  Definition open_floc_vnt (E : vnt var lbl loc lang) :=
+    forall i ℓ x, In x (floc_vnt (open_loc_vnt i ℓ E)) -> x = fst ℓ \/ In x (floc_vnt E).
 
   Lemma open_floc :
     (forall w, open_floc_wvl w) /\
@@ -40,130 +39,191 @@ Section SubstFacts.
     end.
   Qed.
 
-  Definition open_wvl_floc_wvl (w : wvl var loc lang) :=
-    forall i u x, In x (floc_wvl (open_wvl_wvl i u w)) ->
-      In x (floc_wvl u) \/ In x (floc_wvl w).
+  Definition close_flloc_wvl `{Eq lbl} `{Eq loc} (w : wvl var lbl loc lang) :=
+    forall i ℓ x, In x (flloc_wvl (close_wvl i ℓ w)) ->
+      (x <> ℓ /\ In x (flloc_wvl w)).
 
-  Definition open_wvl_floc_nv (σ : nv var loc lang) :=
-    forall i u x, In x (floc_nv (open_wvl_nv i u σ)) ->
-      In x (floc_wvl u) \/ In x (floc_nv σ).
+  Definition close_flloc_nv `{Eq lbl} `{Eq loc} (σ : nv var lbl loc lang) :=
+    forall i ℓ x, In x (flloc_nv (close_nv i ℓ σ)) ->
+      (x <> ℓ /\ In x (flloc_nv σ)).
 
-  Definition open_wvl_floc_vl (v : vl var loc lang) :=
-    forall i u x, In x (floc_vl (open_wvl_vl i u v)) ->
-      In x (floc_wvl u) \/ In x (floc_vl v).
+  Definition close_flloc_vl `{Eq lbl} `{Eq loc} (v : vl var lbl loc lang) :=
+    forall i ℓ x, In x (flloc_vl (close_vl i ℓ v)) ->
+      (x <> ℓ /\ In x (flloc_vl v)).
 
-  Definition open_wvl_floc_vnt (E : vnt var loc lang) :=
-    forall i u x, In x (floc_vnt (open_wvl_vnt i u E)) ->
-      In x (floc_wvl u) \/ In x (floc_vnt E).
-  
-  Lemma open_wvl_floc :
-    (forall w, open_wvl_floc_wvl w) /\
-    (forall σ, open_wvl_floc_nv σ) /\
-    (forall v, open_wvl_floc_vl v) /\
-    (forall E, open_wvl_floc_vnt E).
+  Definition close_flloc_vnt `{Eq lbl} `{Eq loc} (E : vnt var lbl loc lang) :=
+    forall i ℓ x, In x (flloc_vnt (close_vnt i ℓ E)) ->
+      (x <> ℓ /\ In x (flloc_vnt E)).
+
+  Lemma close_flloc `{Eq lbl} `{Eq loc} :
+    (forall w, close_flloc_wvl w) /\
+    (forall σ, close_flloc_nv σ) /\
+    (forall v, close_flloc_vl v) /\
+    (forall E, close_flloc_vnt E).
   Proof.
     apply pre_val_ind; ii; ss.
     all: repeat match goal with
     | _ => solve [eauto]
-    | H : open_wvl_floc_wvl _ |- _ => solve [exploit H; eauto; ii; des; auto]
-    | H : open_wvl_floc_nv _ |- _ => solve [exploit H; eauto; ii; des; auto]
-    | H : open_wvl_floc_vl _ |- _ => solve [exploit H; eauto; ii; des; auto]
-    | H : open_wvl_floc_vnt _ |- _ => solve [exploit H; eauto; ii; des; auto]
+    | H : close_flloc_wvl _ |- _ => solve [exploit H; eauto; ii; des; auto]
+    | H : close_flloc_nv _ |- _ => solve [exploit H; eauto; ii; des; auto]
+    | H : close_flloc_vl _ |- _ => solve [exploit H; eauto; ii; des; auto]
+    | H : close_flloc_vnt _ |- _ => solve [exploit H; eauto; ii; des; auto]
+    | _ => progress (rewrite in_app_iff in *)
+    | _ => progress (des; clarify)
+    | _ => progress (repeat des_hyp)
+    | _ => progress (eqb2eq nat; clarify)
+    | _ => progress (eqb2eq lbl; clarify)
+    | _ => progress (eqb2eq loc; clarify)
+    | _ => progress (ss)
+    end.
+    all: split; auto; ii; des_ifs.
+  Qed.
+
+  Definition trans_floc_wvl (w : wvl var lbl loc lang) :=
+    floc_wvl w = List.map fst (flloc_wvl w).
+
+  Definition trans_floc_nv (σ : nv var lbl loc lang) :=
+    floc_nv σ = List.map fst (flloc_nv σ).
+
+  Definition trans_floc_vl (v : vl var lbl loc lang) :=
+    floc_vl v = List.map fst (flloc_vl v).
+
+  Definition trans_floc_vnt (E : vnt var lbl loc lang) :=
+    floc_vnt E = List.map fst (flloc_vnt E).
+
+  Lemma trans_floc :
+    (forall w, trans_floc_wvl w) /\
+    (forall σ, trans_floc_nv σ) /\
+    (forall v, trans_floc_vl v) /\
+    (forall E, trans_floc_vnt E).
+  Proof.
+    apply pre_val_ind; red; ii; repeat rw; ss;
+    try des_goal; ss; repeat rw; auto;
+    rewrite map_app; auto.
+  Qed.
+
+  Definition open_loc_flloc_wvl (w : wvl var lbl loc lang) :=
+    forall i u x, In x (flloc_wvl (open_loc_wvl i u w)) ->
+      x = u \/ In x (flloc_wvl w).
+
+  Definition open_loc_flloc_nv (σ : nv var lbl loc lang) :=
+    forall i u x, In x (flloc_nv (open_loc_nv i u σ)) ->
+      x = u \/ In x (flloc_nv σ).
+
+  Definition open_loc_flloc_vl (v : vl var lbl loc lang) :=
+    forall i u x, In x (flloc_vl (open_loc_vl i u v)) ->
+      x = u \/ In x (flloc_vl v).
+
+  Definition open_loc_flloc_vnt (E : vnt var lbl loc lang) :=
+    forall i u x, In x (flloc_vnt (open_loc_vnt i u E)) ->
+      x = u \/ In x (flloc_vnt E).
+ 
+  Lemma open_loc_flloc :
+    (forall w, open_loc_flloc_wvl w) /\
+    (forall σ, open_loc_flloc_nv σ) /\
+    (forall v, open_loc_flloc_vl v) /\
+    (forall E, open_loc_flloc_vnt E).
+  Proof.
+    apply pre_val_ind; ii; ss.
+    all: repeat match goal with
+    | _ => solve [eauto]
+    | H : open_loc_flloc_wvl _ |- _ => solve [exploit H; eauto; ii; des; auto]
+    | H : open_loc_flloc_nv _ |- _ => solve [exploit H; eauto; ii; des; auto]
+    | H : open_loc_flloc_vl _ |- _ => solve [exploit H; eauto; ii; des; auto]
+    | H : open_loc_flloc_vnt _ |- _ => solve [exploit H; eauto; ii; des; auto]
     | _ => progress (rewrite in_app_iff in *)
     | _ => progress (des; clarify)
     | _ => progress (des_ifs)
-    | _ => progress (eqb2eq loc; clarify)
     | _ => progress (eqb2eq nat; clarify)
     | _ => progress (ss)
     end.
   Qed.
 
-  Definition open_wvl_inc_floc_wvl (w : wvl var loc lang) :=
-    forall i u x, In x (floc_wvl w) ->
-      In x (floc_wvl (open_wvl_wvl i u w)).
+  Definition open_wvl_flloc_wvl (w : wvl var lbl loc lang) :=
+    forall i u x, In x (flloc_wvl (open_wvl_wvl i u w)) ->
+      In x (flloc_wvl u) \/ In x (flloc_wvl w).
 
-  Definition open_wvl_inc_floc_nv (σ : nv var loc lang) :=
-    forall i u x, In x (floc_nv σ) ->
-      In x (floc_nv (open_wvl_nv i u σ)).
+  Definition open_wvl_flloc_nv (σ : nv var lbl loc lang) :=
+    forall i u x, In x (flloc_nv (open_wvl_nv i u σ)) ->
+      In x (flloc_wvl u) \/ In x (flloc_nv σ).
 
-  Definition open_wvl_inc_floc_vl (v : vl var loc lang) :=
-    forall i u x, In x (floc_vl v) ->
-      In x (floc_vl (open_wvl_vl i u v)).
+  Definition open_wvl_flloc_vl (v : vl var lbl loc lang) :=
+    forall i u x, In x (flloc_vl (open_wvl_vl i u v)) ->
+      In x (flloc_wvl u) \/ In x (flloc_vl v).
 
-  Definition open_wvl_inc_floc_vnt (E : vnt var loc lang) :=
-    forall i u x, In x (floc_vnt E) ->
-      In x (floc_vnt (open_wvl_vnt i u E)).
+  Definition open_wvl_flloc_vnt (E : vnt var lbl loc lang) :=
+    forall i u x, In x (flloc_vnt (open_wvl_vnt i u E)) ->
+      In x (flloc_wvl u) \/ In x (flloc_vnt E).
+ 
+  Lemma open_wvl_flloc :
+    (forall w, open_wvl_flloc_wvl w) /\
+    (forall σ, open_wvl_flloc_nv σ) /\
+    (forall v, open_wvl_flloc_vl v) /\
+    (forall E, open_wvl_flloc_vnt E).
+  Proof.
+    apply pre_val_ind; ii; ss.
+    all: repeat match goal with
+    | _ => solve [eauto]
+    | H : open_wvl_flloc_wvl _ |- _ => solve [exploit H; eauto; ii; des; auto]
+    | H : open_wvl_flloc_nv _ |- _ => solve [exploit H; eauto; ii; des; auto]
+    | H : open_wvl_flloc_vl _ |- _ => solve [exploit H; eauto; ii; des; auto]
+    | H : open_wvl_flloc_vnt _ |- _ => solve [exploit H; eauto; ii; des; auto]
+    | _ => progress (rewrite in_app_iff in *)
+    | _ => progress (des; clarify)
+    | _ => progress (des_ifs)
+    | _ => progress (eqb2eq nat; clarify)
+    | _ => progress (ss)
+    end.
+  Qed.
+
+  Definition open_wvl_inc_flloc_wvl (w : wvl var lbl loc lang) :=
+    forall i u x, In x (flloc_wvl w) ->
+      In x (flloc_wvl (open_wvl_wvl i u w)).
+
+  Definition open_wvl_inc_flloc_nv (σ : nv var lbl loc lang) :=
+    forall i u x, In x (flloc_nv σ) ->
+      In x (flloc_nv (open_wvl_nv i u σ)).
+
+  Definition open_wvl_inc_flloc_vl (v : vl var lbl loc lang) :=
+    forall i u x, In x (flloc_vl v) ->
+      In x (flloc_vl (open_wvl_vl i u v)).
+
+  Definition open_wvl_inc_flloc_vnt (E : vnt var lbl loc lang) :=
+    forall i u x, In x (flloc_vnt E) ->
+      In x (flloc_vnt (open_wvl_vnt i u E)).
   
-  Lemma open_wvl_inc_floc :
-    (forall w, open_wvl_inc_floc_wvl w) /\
-    (forall σ, open_wvl_inc_floc_nv σ) /\
-    (forall v, open_wvl_inc_floc_vl v) /\
-    (forall E, open_wvl_inc_floc_vnt E).
+  Lemma open_wvl_inc_flloc :
+    (forall w, open_wvl_inc_flloc_wvl w) /\
+    (forall σ, open_wvl_inc_flloc_nv σ) /\
+    (forall v, open_wvl_inc_flloc_vl v) /\
+    (forall E, open_wvl_inc_flloc_vnt E).
   Proof.
     apply pre_val_ind; ii; ss.
     all: repeat first [
-      des_goal; eqb2eq loc; clarify|
       des_goal; eqb2eq nat; clarify|
+      des_goal; clarify|
       rewrite in_app_iff in *; auto].
     all: repeat match goal with
     | _ => solve [eauto]
-    | H : open_wvl_inc_floc_wvl _ |- _ => solve [exploit H; eauto; ii; des; auto]
-    | H : open_wvl_inc_floc_nv _ |- _ => solve [exploit H; eauto; ii; des; auto]
-    | H : open_wvl_inc_floc_vl _ |- _ => solve [exploit H; eauto; ii; des; auto]
-    | H : open_wvl_inc_floc_vnt _ |- _ => solve [exploit H; eauto; ii; des; auto]
+    | H : open_wvl_inc_flloc_wvl _ |- _ => solve [exploit H; eauto; ii; des; auto]
+    | H : open_wvl_inc_flloc_nv _ |- _ => solve [exploit H; eauto; ii; des; auto]
+    | H : open_wvl_inc_flloc_vl _ |- _ => solve [exploit H; eauto; ii; des; auto]
+    | H : open_wvl_inc_flloc_vnt _ |- _ => solve [exploit H; eauto; ii; des; auto]
     | _ => progress (des; clarify)
     | _ => progress (ss)
     end.
   Qed.
 
-  Definition close_floc_wvl `{Eq loc} (w : wvl var loc lang) :=
-    forall i ℓ x, In x (floc_wvl (close_wvl i ℓ w)) ->
-      (x <> ℓ /\ In x (floc_wvl w)).
-
-  Definition close_floc_nv `{Eq loc} (σ : nv var loc lang) :=
-    forall i ℓ x, In x (floc_nv (close_nv i ℓ σ)) ->
-      (x <> ℓ /\ In x (floc_nv σ)).
-
-  Definition close_floc_vl `{Eq loc} (v : vl var loc lang) :=
-    forall i ℓ x, In x (floc_vl (close_vl i ℓ v)) ->
-      (x <> ℓ /\ In x (floc_vl v)).
-
-  Definition close_floc_vnt `{Eq loc} (E : vnt var loc lang) :=
-    forall i ℓ x, In x (floc_vnt (close_vnt i ℓ E)) ->
-      (x <> ℓ /\ In x (floc_vnt E)).
-
-  Lemma close_floc `{Eq loc} :
-    (forall w, close_floc_wvl w) /\
-    (forall σ, close_floc_nv σ) /\
-    (forall v, close_floc_vl v) /\
-    (forall E, close_floc_vnt E).
-  Proof.
-    apply pre_val_ind; ii; ss.
-    all: repeat match goal with
-    | _ => solve [eauto]
-    | H : close_floc_wvl _ |- _ => solve [exploit H; eauto; ii; des; auto]
-    | H : close_floc_nv _ |- _ => solve [exploit H; eauto; ii; des; auto]
-    | H : close_floc_vl _ |- _ => solve [exploit H; eauto; ii; des; auto]
-    | H : close_floc_vnt _ |- _ => solve [exploit H; eauto; ii; des; auto]
-    | _ => progress (rewrite in_app_iff in *)
-    | _ => progress (des; clarify)
-    | _ => progress (des_ifs)
-    | _ => progress (eqb2eq loc; clarify)
-    | _ => progress (eqb2eq nat; clarify)
-    | _ => progress (ss)
-    end.
-  Qed.
-
-  Definition open_inc_floc_wvl (w : wvl var loc lang) :=
+  Definition open_inc_floc_wvl (w : wvl var lbl loc lang) :=
     forall i ℓ x, In x (floc_wvl w) -> In x (floc_wvl (open_loc_wvl i ℓ w)).
 
-  Definition open_inc_floc_nv (σ : nv var loc lang) :=
+  Definition open_inc_floc_nv (σ : nv var lbl loc lang) :=
     forall i ℓ x, In x (floc_nv σ) -> In x (floc_nv (open_loc_nv i ℓ σ)).
 
-  Definition open_inc_floc_vl (v : vl var loc lang) :=
+  Definition open_inc_floc_vl (v : vl var lbl loc lang) :=
     forall i ℓ x, In x (floc_vl v) -> In x (floc_vl (open_loc_vl i ℓ v)).
 
-  Definition open_inc_floc_vnt (E : vnt var loc lang) :=
+  Definition open_inc_floc_vnt (E : vnt var lbl loc lang) :=
     forall i ℓ x, In x (floc_vnt E) -> In x (floc_vnt (open_loc_vnt i ℓ E)).
 
   Lemma open_inc_floc :
@@ -182,37 +242,36 @@ Section SubstFacts.
     | _ => progress (rewrite in_app_iff in *)
     | _ => progress (des; clarify)
     | _ => progress (des_ifs)
-    | _ => progress (eqb2eq loc; clarify)
     | _ => progress (eqb2eq nat; clarify)
     | _ => progress (ss)
     end.
   Qed.
 
-  Definition subst_intro_wvl `{Eq loc} (w : wvl var loc lang) :=
-    forall i ℓ u (FRESH : ~ In ℓ (floc_wvl w)),
+  Definition subst_intro_wvl `{Eq lbl} `{Eq loc} (w : wvl var lbl loc lang) :=
+    forall i ℓ p u (FRESH : ~ In ℓ (floc_wvl w)),
       open_wvl_wvl i u w =
-      subst_wvl_wvl u ℓ (open_loc_wvl i ℓ w)
+      subst_wvl_wvl u (ℓ, p) (open_loc_wvl i (ℓ, p) w)
   .
 
-  Definition subst_intro_nv `{Eq loc} (σ : nv var loc lang) :=
-    forall i ℓ u (FRESH : ~ In ℓ (floc_nv σ)),
+  Definition subst_intro_nv `{Eq lbl} `{Eq loc} (σ : nv var lbl loc lang) :=
+    forall i ℓ p u (FRESH : ~ In ℓ (floc_nv σ)),
       open_wvl_nv i u σ =
-      subst_wvl_nv u ℓ (open_loc_nv i ℓ σ)
+      subst_wvl_nv u (ℓ, p) (open_loc_nv i (ℓ, p) σ)
   .
 
-  Definition subst_intro_vl `{Eq loc} (v : vl var loc lang) :=
-    forall i ℓ u (FRESH : ~ In ℓ (floc_vl v)),
+  Definition subst_intro_vl `{Eq lbl} `{Eq loc} (v : vl var lbl loc lang) :=
+    forall i ℓ p u (FRESH : ~ In ℓ (floc_vl v)),
       open_wvl_vl i u v =
-      subst_wvl_vl u ℓ (open_loc_vl i ℓ v)
+      subst_wvl_vl u (ℓ, p) (open_loc_vl i (ℓ, p) v)
   .
 
-  Definition subst_intro_vnt `{Eq loc} (E : vnt var loc lang) :=
-    forall i ℓ u (FRESH : ~ In ℓ (floc_vnt E)),
+  Definition subst_intro_vnt `{Eq lbl} `{Eq loc} (E : vnt var lbl loc lang) :=
+    forall i ℓ p u (FRESH : ~ In ℓ (floc_vnt E)),
       open_wvl_vnt i u E =
-      subst_wvl_vnt u ℓ (open_loc_vnt i ℓ E)
+      subst_wvl_vnt u (ℓ, p) (open_loc_vnt i (ℓ, p) E)
   .
 
-  Lemma subst_intro `{Eq loc} :
+  Lemma subst_intro `{Eq lbl} `{Eq loc} :
     (forall w, subst_intro_wvl w) /\
     (forall σ, subst_intro_nv σ) /\
     (forall v, subst_intro_vl v) /\
@@ -222,61 +281,62 @@ Section SubstFacts.
     all:try (cbn; f_equal; solve [auto]).
     - des_goal.
       + eqb2eq nat. subst.
-        rewrite eqb_refl. f_equal. auto.
+        repeat rewrite eqb_refl. s. f_equal. auto.
       + f_equal. auto.
-    - des_goal.
+    - des_hyp; split_nIn; des_goal.
       + eqb2eq loc. contradict.
       + f_equal. auto.
     - split_nIn; f_equal; auto.
     - split_nIn; f_equal; auto.
   Qed.
 
-  Definition open_loc_close_wvl `{Eq loc} (w : wvl var loc lang) :=
+  Definition open_loc_close_wvl `{Eq lbl} `{Eq loc} (w : wvl var lbl loc lang) :=
     forall i ℓ, close_wvl i ℓ (open_loc_wvl i ℓ w) = close_wvl i ℓ w.
 
-  Definition open_loc_close_nv `{Eq loc} (σ : nv var loc lang) :=
+  Definition open_loc_close_nv `{Eq lbl} `{Eq loc} (σ : nv var lbl loc lang) :=
     forall i ℓ, close_nv i ℓ (open_loc_nv i ℓ σ) = close_nv i ℓ σ.
 
-  Definition open_loc_close_vl `{Eq loc} (v : vl var loc lang) :=
+  Definition open_loc_close_vl `{Eq lbl} `{Eq loc} (v : vl var lbl loc lang) :=
     forall i ℓ, close_vl i ℓ (open_loc_vl i ℓ v) = close_vl i ℓ v.
 
-  Definition open_loc_close_vnt `{Eq loc} (E : vnt var loc lang) :=
+  Definition open_loc_close_vnt `{Eq lbl} `{Eq loc} (E : vnt var lbl loc lang) :=
     forall i ℓ, close_vnt i ℓ (open_loc_vnt i ℓ E) = close_vnt i ℓ E.
 
-  Lemma open_loc_close `{Eq loc} :
+  Lemma open_loc_close `{Eq lbl} `{Eq loc} :
     (forall w, open_loc_close_wvl w) /\
     (forall σ, open_loc_close_nv σ) /\
     (forall v, open_loc_close_vl v) /\
     (forall E, open_loc_close_vnt E).
   Proof.
     apply pre_val_ind; ii; ss; repeat des_goal; repeat rw; eauto.
-    all:rewrite eqb_refl in *; eqb2eq nat; clarify.
+    all:repeat des_hyp; rewrite eqb_refl in *; eqb2eq nat; clarify.
   Qed.
 
-  Definition close_fresh_wvl `{Eq loc} (w : wvl var loc lang) :=
-    forall i ℓ (FRESH : ~ In ℓ (floc_wvl w)),
-      close_wvl i ℓ w = w.
+  Definition close_fresh_wvl `{Eq lbl} `{Eq loc} (w : wvl var lbl loc lang) :=
+    forall i ℓ p (FRESH : ~ In ℓ (floc_wvl w)),
+      close_wvl i (ℓ, p) w = w.
 
-  Definition close_fresh_nv `{Eq loc} (σ : nv var loc lang) :=
-    forall i ℓ (FRESH : ~ In ℓ (floc_nv σ)),
-      close_nv i ℓ σ = σ.
+  Definition close_fresh_nv `{Eq lbl} `{Eq loc} (σ : nv var lbl loc lang) :=
+    forall i ℓ p (FRESH : ~ In ℓ (floc_nv σ)),
+      close_nv i (ℓ, p) σ = σ.
 
-  Definition close_fresh_vl `{Eq loc} (v : vl var loc lang) :=
-    forall i ℓ (FRESH : ~ In ℓ (floc_vl v)),
-      close_vl i ℓ v = v.
+  Definition close_fresh_vl `{Eq lbl} `{Eq loc} (v : vl var lbl loc lang) :=
+    forall i ℓ p (FRESH : ~ In ℓ (floc_vl v)),
+      close_vl i (ℓ, p) v = v.
 
-  Definition close_fresh_vnt `{Eq loc} (E : vnt var loc lang) :=
-    forall i ℓ (FRESH : ~ In ℓ (floc_vnt E)),
-      close_vnt i ℓ E = E.
+  Definition close_fresh_vnt `{Eq lbl} `{Eq loc} (E : vnt var lbl loc lang) :=
+    forall i ℓ p (FRESH : ~ In ℓ (floc_vnt E)),
+      close_vnt i (ℓ, p) E = E.
 
-  Lemma close_fresh `{Eq loc} :
+  Lemma close_fresh `{Eq lbl} `{Eq loc} :
     (forall w, close_fresh_wvl w) /\
     (forall σ, close_fresh_nv σ) /\
     (forall v, close_fresh_vl v) /\
     (forall E, close_fresh_vnt E).
   Proof.
-    apply pre_val_ind; ii; ss; split_nIn;
-    try (progress des_ifs; eqb2eq loc; clarify).
+    apply pre_val_ind; ii; ss; repeat des_hyp; split_nIn;
+    repeat des_goal; repeat des_hyp;
+    try eqb2eq loc; try eqb2eq lbl; clarify.
     all: repeat match goal with
     | RR : close_fresh_wvl _ |- _ => erewrite RR; eauto
     | RR : close_fresh_nv _ |- _ => erewrite RR; eauto
@@ -285,30 +345,31 @@ Section SubstFacts.
     end.
   Qed.
 
-  Definition subst_loc_fresh_wvl `{Eq loc} (w : wvl var loc lang) :=
-    forall ν ℓ (FRESH : ~ In ℓ (floc_wvl w)),
-      subst_loc_wvl ν ℓ w = w.
+  Definition subst_loc_fresh_wvl `{Eq lbl} `{Eq loc} (w : wvl var lbl loc lang) :=
+    forall ν ℓ p (FRESH : ~ In ℓ (floc_wvl w)),
+      subst_loc_wvl ν (ℓ, p) w = w.
 
-  Definition subst_loc_fresh_nv `{Eq loc} (σ : nv var loc lang) :=
-    forall ν ℓ (FRESH : ~ In ℓ (floc_nv σ)),
-      subst_loc_nv ν ℓ σ = σ.
+  Definition subst_loc_fresh_nv `{Eq lbl} `{Eq loc} (σ : nv var lbl loc lang) :=
+    forall ν ℓ p (FRESH : ~ In ℓ (floc_nv σ)),
+      subst_loc_nv ν (ℓ, p) σ = σ.
 
-  Definition subst_loc_fresh_vl `{Eq loc} (v : vl var loc lang) :=
-    forall ν ℓ (FRESH : ~ In ℓ (floc_vl v)),
-      subst_loc_vl ν ℓ v = v.
+  Definition subst_loc_fresh_vl `{Eq lbl} `{Eq loc} (v : vl var lbl loc lang) :=
+    forall ν ℓ p (FRESH : ~ In ℓ (floc_vl v)),
+      subst_loc_vl ν (ℓ, p) v = v.
 
-  Definition subst_loc_fresh_vnt `{Eq loc} (E : vnt var loc lang) :=
-    forall ν ℓ (FRESH : ~ In ℓ (floc_vnt E)),
-      subst_loc_vnt ν ℓ E = E.
+  Definition subst_loc_fresh_vnt `{Eq lbl} `{Eq loc} (E : vnt var lbl loc lang) :=
+    forall ν ℓ p (FRESH : ~ In ℓ (floc_vnt E)),
+      subst_loc_vnt ν (ℓ, p) E = E.
 
-  Lemma subst_loc_fresh `{Eq loc} :
+  Lemma subst_loc_fresh `{Eq lbl} `{Eq loc} :
     (forall w, subst_loc_fresh_wvl w) /\
     (forall σ, subst_loc_fresh_nv σ) /\
     (forall v, subst_loc_fresh_vl v) /\
     (forall E, subst_loc_fresh_vnt E).
   Proof.
-    apply pre_val_ind; ii; ss; split_nIn;
-    try (progress des_ifs; eqb2eq loc; clarify).
+    apply pre_val_ind; ii; ss; repeat des_hyp; split_nIn;
+    repeat des_goal; repeat des_hyp;
+    try eqb2eq loc; try eqb2eq lbl; clarify.
     all: repeat match goal with
     | RR : subst_loc_fresh_wvl _ |- _ => erewrite RR; eauto
     | RR : subst_loc_fresh_nv _ |- _ => erewrite RR; eauto
@@ -317,30 +378,31 @@ Section SubstFacts.
     end.
   Qed.
 
-  Definition subst_wvl_fresh_wvl `{Eq loc} (w : wvl var loc lang) :=
-    forall ν ℓ (FRESH : ~ In ℓ (floc_wvl w)),
-      subst_wvl_wvl ν ℓ w = w.
+  Definition subst_wvl_fresh_wvl `{Eq lbl} `{Eq loc} (w : wvl var lbl loc lang) :=
+    forall ν ℓ p (FRESH : ~ In ℓ (floc_wvl w)),
+      subst_wvl_wvl ν (ℓ, p) w = w.
 
-  Definition subst_wvl_fresh_nv `{Eq loc} (σ : nv var loc lang) :=
-    forall ν ℓ (FRESH : ~ In ℓ (floc_nv σ)),
-      subst_wvl_nv ν ℓ σ = σ.
+  Definition subst_wvl_fresh_nv `{Eq lbl} `{Eq loc} (σ : nv var lbl loc lang) :=
+    forall ν ℓ p (FRESH : ~ In ℓ (floc_nv σ)),
+      subst_wvl_nv ν (ℓ, p) σ = σ.
 
-  Definition subst_wvl_fresh_vl `{Eq loc} (v : vl var loc lang) :=
-    forall ν ℓ (FRESH : ~ In ℓ (floc_vl v)),
-      subst_wvl_vl ν ℓ v = v.
+  Definition subst_wvl_fresh_vl `{Eq lbl} `{Eq loc} (v : vl var lbl loc lang) :=
+    forall ν ℓ p (FRESH : ~ In ℓ (floc_vl v)),
+      subst_wvl_vl ν (ℓ, p) v = v.
 
-  Definition subst_wvl_fresh_vnt `{Eq loc} (E : vnt var loc lang) :=
-    forall ν ℓ (FRESH : ~ In ℓ (floc_vnt E)),
-      subst_wvl_vnt ν ℓ E = E.
+  Definition subst_wvl_fresh_vnt `{Eq lbl} `{Eq loc} (E : vnt var lbl loc lang) :=
+    forall ν ℓ p (FRESH : ~ In ℓ (floc_vnt E)),
+      subst_wvl_vnt ν (ℓ, p) E = E.
 
-  Lemma subst_wvl_fresh `{Eq loc} :
+  Lemma subst_wvl_fresh `{Eq lbl} `{Eq loc} :
     (forall w, subst_wvl_fresh_wvl w) /\
     (forall σ, subst_wvl_fresh_nv σ) /\
     (forall v, subst_wvl_fresh_vl v) /\
     (forall E, subst_wvl_fresh_vnt E).
   Proof.
-    apply pre_val_ind; ii; ss; split_nIn;
-    try (progress des_ifs; eqb2eq loc; clarify).
+    apply pre_val_ind; ii; ss; repeat des_hyp; split_nIn;
+    repeat des_goal; repeat des_hyp;
+    try eqb2eq loc; try eqb2eq lbl; clarify.
     all: repeat match goal with
     | RR : subst_wvl_fresh_wvl _ |- _ => erewrite RR; eauto
     | RR : subst_wvl_fresh_nv _ |- _ => erewrite RR; eauto
@@ -349,42 +411,41 @@ Section SubstFacts.
     end.
   Qed.
 
-  Definition close_open_wvl_wvl `{Eq loc} (w : wvl var loc lang) :=
-    forall i j ℓ u
+  Definition close_open_wvl_wvl `{Eq lbl} `{Eq loc} (w : wvl var lbl loc lang) :=
+    forall i j ℓ p u
       (NEQ : i <> j)
       (FRESH : ~ In ℓ (floc_wvl u)),
-    open_wvl_wvl i u (close_wvl j ℓ w) = close_wvl j ℓ (open_wvl_wvl i u w).
+    open_wvl_wvl i u (close_wvl j (ℓ, p) w) = close_wvl j (ℓ, p) (open_wvl_wvl i u w).
 
-  Definition close_open_wvl_nv `{Eq loc} (σ : nv var loc lang) :=
-    forall i j ℓ u
+  Definition close_open_wvl_nv `{Eq lbl} `{Eq loc} (σ : nv var lbl loc lang) :=
+    forall i j ℓ p u
       (NEQ : i <> j)
       (FRESH : ~ In ℓ (floc_wvl u)),
-    open_wvl_nv i u (close_nv j ℓ σ) = close_nv j ℓ (open_wvl_nv i u σ).
+    open_wvl_nv i u (close_nv j (ℓ, p) σ) = close_nv j (ℓ, p) (open_wvl_nv i u σ).
 
-  Definition close_open_wvl_vl `{Eq loc} (v : vl var loc lang) :=
-    forall i j ℓ u
+  Definition close_open_wvl_vl `{Eq lbl} `{Eq loc} (v : vl var lbl loc lang) :=
+    forall i j ℓ p u
       (NEQ : i <> j)
       (FRESH : ~ In ℓ (floc_wvl u)),
-    open_wvl_vl i u (close_vl j ℓ v) = close_vl j ℓ (open_wvl_vl i u v).
+    open_wvl_vl i u (close_vl j (ℓ, p) v) = close_vl j (ℓ, p) (open_wvl_vl i u v).
 
-  Definition close_open_wvl_vnt `{Eq loc} (E : vnt var loc lang) :=
-    forall i j ℓ u
+  Definition close_open_wvl_vnt `{Eq lbl} `{Eq loc} (E : vnt var lbl loc lang) :=
+    forall i j ℓ p u
       (NEQ : i <> j)
       (FRESH : ~ In ℓ (floc_wvl u)),
-    open_wvl_vnt i u (close_vnt j ℓ E) = close_vnt j ℓ (open_wvl_vnt i u E).
+    open_wvl_vnt i u (close_vnt j (ℓ, p) E) = close_vnt j (ℓ, p) (open_wvl_vnt i u E).
 
-  Lemma close_open_wvl `{Eq loc} :
+  Lemma close_open_wvl `{Eq lbl} `{Eq loc} :
     (forall w, close_open_wvl_wvl w) /\
     (forall σ, close_open_wvl_nv σ) /\
     (forall v, close_open_wvl_vl v) /\
     (forall E, close_open_wvl_vnt E).
   Proof.
-    apply pre_val_ind; ii; ss.
-    all: repeat first [
-      des_goal; eqb2eq loc; clarify|
-      des_goal; eqb2eq nat; clarify].
+    apply pre_val_ind; ii; ss; repeat des_hyp; split_nIn;
+    repeat des_goal; repeat des_hyp;
+    try eqb2eq nat; try eqb2eq loc; try eqb2eq lbl; clarify.
     all: try match goal with
-    | _ : ~ In ?ℓ (floc_wvl ?u) |- context [close_wvl _ ?ℓ ?u] =>
+    | _ : ~ In ?ℓ (floc_wvl ?u) |- context [close_wvl _ (?ℓ, _) ?u] =>
       assert (close_fresh_wvl u) as RR by apply close_fresh;
       rewrite RR; eauto
     end.
@@ -396,40 +457,39 @@ Section SubstFacts.
     end.
   Qed.
 
-  Definition close_open_loc_wvl `{Eq loc} (w : wvl var loc lang) :=
+  Definition close_open_loc_wvl `{Eq lbl} `{Eq loc} (w : wvl var lbl loc lang) :=
     forall i j ℓ ν
       (NEQ : i <> j)
       (FRESH : ℓ <> ν),
     open_loc_wvl i ν (close_wvl j ℓ w) = close_wvl j ℓ (open_loc_wvl i ν w).
 
-  Definition close_open_loc_nv `{Eq loc} (σ : nv var loc lang) :=
+  Definition close_open_loc_nv `{Eq lbl} `{Eq loc} (σ : nv var lbl loc lang) :=
     forall i j ℓ ν
       (NEQ : i <> j)
       (FRESH : ℓ <> ν),
     open_loc_nv i ν (close_nv j ℓ σ) = close_nv j ℓ (open_loc_nv i ν σ).
 
-  Definition close_open_loc_vl `{Eq loc} (v : vl var loc lang) :=
+  Definition close_open_loc_vl `{Eq lbl} `{Eq loc} (v : vl var lbl loc lang) :=
     forall i j ℓ ν
       (NEQ : i <> j)
       (FRESH : ℓ <> ν),
     open_loc_vl i ν (close_vl j ℓ v) = close_vl j ℓ (open_loc_vl i ν v).
 
-  Definition close_open_loc_vnt `{Eq loc} (E : vnt var loc lang) :=
+  Definition close_open_loc_vnt `{Eq lbl} `{Eq loc} (E : vnt var lbl loc lang) :=
     forall i j ℓ ν
       (NEQ : i <> j)
       (FRESH : ℓ <> ν),
     open_loc_vnt i ν (close_vnt j ℓ E) = close_vnt j ℓ (open_loc_vnt i ν E).
 
-  Lemma close_open_loc `{Eq loc} :
+  Lemma close_open_loc `{Eq lbl} `{Eq loc} :
     (forall w, close_open_loc_wvl w) /\
     (forall σ, close_open_loc_nv σ) /\
     (forall v, close_open_loc_vl v) /\
     (forall E, close_open_loc_vnt E).
   Proof.
-    apply pre_val_ind; ii; ss.
-    all: repeat first [
-      des_goal; eqb2eq loc; clarify|
-      des_goal; eqb2eq nat; clarify].
+    apply pre_val_ind; ii; ss; repeat des_hyp; split_nIn;
+    repeat des_goal; repeat des_hyp;
+    try eqb2eq nat; try eqb2eq loc; try eqb2eq lbl; clarify.
     all: repeat match goal with
     | RR : close_open_loc_wvl _ |- _ => erewrite RR; eauto
     | RR : close_open_loc_nv _ |- _ => erewrite RR; eauto
@@ -438,19 +498,19 @@ Section SubstFacts.
     end.
   Qed.
 
-  Definition open_wvl_lc_wvl `{Eq loc} (w : wvl var loc lang) (W : wvalue w) :=
+  Definition open_wvl_lc_wvl `{Eq lbl} `{Eq loc} (w : wvl var lbl loc lang) (W : wvalue w) :=
     forall i u, open_wvl_wvl i u w = w.
 
-  Definition open_wvl_lc_nv `{Eq loc} (σ : nv var loc lang) (Σ : env σ) :=
+  Definition open_wvl_lc_nv `{Eq lbl} `{Eq loc} (σ : nv var lbl loc lang) (Σ : env σ) :=
     forall i u, open_wvl_nv i u σ = σ.
 
-  Definition open_wvl_lc_vl `{Eq loc} (v : vl var loc lang) (V : value v) :=
+  Definition open_wvl_lc_vl `{Eq lbl} `{Eq loc} (v : vl var lbl loc lang) (V : value v) :=
     forall i u, open_wvl_vl i u v = v.
 
-  Definition open_wvl_lc_vnt `{Eq loc} (E : vnt var loc lang) (EE : event E) :=
+  Definition open_wvl_lc_vnt `{Eq lbl} `{Eq loc} (E : vnt var lbl loc lang) (EE : event E) :=
     forall i u, open_wvl_vnt i u E = E.
-  
-  Lemma open_wvl_lc `{Name loc} :
+ 
+  Lemma open_wvl_lc `{Eq lbl} `{Name loc} :
     (forall w W, open_wvl_lc_wvl w W) /\
     (forall σ Σ, open_wvl_lc_nv σ Σ) /\
     (forall v V, open_wvl_lc_vl v V) /\
@@ -458,8 +518,8 @@ Section SubstFacts.
   Proof.
     apply val_ind; ii; ss; repeat rw; eauto.
     gensym_tac (L ++ (floc_wvl u) ++ (floc_vl v)) ℓ.
-    replace v with (close_vl 0 ℓ (open_loc_vl 0 ℓ v)) at 1.
-    assert (close_open_wvl_vl (open_loc_vl 0 ℓ v)) as RR by apply close_open_wvl.
+    replace v with (close_vl 0 (ℓ, p) (open_loc_vl 0 (ℓ, p) v)) at 1.
+    assert (close_open_wvl_vl (open_loc_vl 0 (ℓ, p) v)) as RR by apply close_open_wvl.
     erewrite RR; eauto.
     match goal with RR : forall _, ~ In _ _ -> _ |- _ => rewrite RR; f_equal end.
     all: try match goal with
@@ -470,28 +530,29 @@ Section SubstFacts.
     auto.
   Qed.
 
-  Definition open_loc_lc_wvl `{Eq loc} (w : wvl var loc lang) (W : wvalue w) :=
+  Definition open_loc_lc_wvl `{Eq lbl} `{Eq loc} (w : wvl var lbl loc lang) (W : wvalue w) :=
     forall i ℓ, open_loc_wvl i ℓ w = w.
 
-  Definition open_loc_lc_nv `{Eq loc} (σ : nv var loc lang) (Σ : env σ) :=
+  Definition open_loc_lc_nv `{Eq lbl} `{Eq loc} (σ : nv var lbl loc lang) (Σ : env σ) :=
     forall i ℓ, open_loc_nv i ℓ σ = σ.
 
-  Definition open_loc_lc_vl `{Eq loc} (v : vl var loc lang) (V : value v) :=
+  Definition open_loc_lc_vl `{Eq lbl} `{Eq loc} (v : vl var lbl loc lang) (V : value v) :=
     forall i ℓ, open_loc_vl i ℓ v = v.
 
-  Definition open_loc_lc_vnt `{Eq loc} (E : vnt var loc lang) (EE : event E) :=
+  Definition open_loc_lc_vnt `{Eq lbl} `{Eq loc} (E : vnt var lbl loc lang) (EE : event E) :=
     forall i ℓ, open_loc_vnt i ℓ E = E.
 
-  Lemma open_loc_lc `{Name loc} :
+  Lemma open_loc_lc `{Eq lbl} `{Name loc} :
     (forall w W, open_loc_lc_wvl w W) /\
     (forall σ Σ, open_loc_lc_nv σ Σ) /\
     (forall v V, open_loc_lc_vl v V) /\
     (forall E EE, open_loc_lc_vnt E EE).
   Proof.
     apply val_ind; ii; ss; repeat rw; eauto.
+    destruct ℓ as [ℓ p'].
     gensym_tac (ℓ :: L ++ (floc_vl v)) ν.
-    replace v with (close_vl 0 ν (open_loc_vl 0 ν v)) at 1.
-    assert (close_open_loc_vl (open_loc_vl 0 ν v)) as RR by apply close_open_loc.
+    replace v with (close_vl 0 (ν, p) (open_loc_vl 0 (ν, p) v)) at 1.
+    assert (close_open_loc_vl (open_loc_vl 0 (ν, p) v)) as RR by apply close_open_loc.
     erewrite RR; eauto.
     match goal with RR : forall _, ~ In _ _ -> _ |- _ => rewrite RR; f_equal end.
     all: try match goal with
@@ -499,43 +560,42 @@ Section SubstFacts.
       assert (open_loc_close_vl v) by apply open_loc_close; rw;
       assert (close_fresh_vl v) by apply close_fresh; rw; auto
     end.
-    auto.
+    all: ii; clarify; auto.
   Qed.
 
-  Definition open_wvl_subst_wvl_wvl `{Eq loc} (w : wvl var loc lang) :=
+  Definition open_wvl_subst_wvl_wvl `{Eq lbl} `{Eq loc} (w : wvl var lbl loc lang) :=
     forall i ℓ u' u (U : wvalue u),
       subst_wvl_wvl u ℓ (open_wvl_wvl i u' w) =
       open_wvl_wvl i (subst_wvl_wvl u ℓ u') (subst_wvl_wvl u ℓ w)
   .
 
-  Definition open_wvl_subst_wvl_nv `{Eq loc} (σ : nv var loc lang) :=
+  Definition open_wvl_subst_wvl_nv `{Eq lbl} `{Eq loc} (σ : nv var lbl loc lang) :=
     forall i ℓ u' u (U : wvalue u),
       subst_wvl_nv u ℓ (open_wvl_nv i u' σ) =
       open_wvl_nv i (subst_wvl_wvl u ℓ u') (subst_wvl_nv u ℓ σ)
   .
 
-  Definition open_wvl_subst_wvl_vl `{Eq loc} (v : vl var loc lang) :=
+  Definition open_wvl_subst_wvl_vl `{Eq lbl} `{Eq loc} (v : vl var lbl loc lang) :=
     forall i ℓ u' u (U : wvalue u),
       subst_wvl_vl u ℓ (open_wvl_vl i u' v) =
       open_wvl_vl i (subst_wvl_wvl u ℓ u') (subst_wvl_vl u ℓ v)
   .
 
-  Definition open_wvl_subst_wvl_vnt `{Eq loc} (E : vnt var loc lang) :=
+  Definition open_wvl_subst_wvl_vnt `{Eq lbl} `{Eq loc} (E : vnt var lbl loc lang) :=
     forall i ℓ u' u (U : wvalue u),
       subst_wvl_vnt u ℓ (open_wvl_vnt i u' E) =
       open_wvl_vnt i (subst_wvl_wvl u ℓ u') (subst_wvl_vnt u ℓ E)
   .
  
-  Lemma open_wvl_subst_wvl `{Name loc} :
+  Lemma open_wvl_subst_wvl `{Eq lbl} `{Name loc} :
     (forall w, open_wvl_subst_wvl_wvl w) /\
     (forall σ, open_wvl_subst_wvl_nv σ) /\
     (forall v, open_wvl_subst_wvl_vl v) /\
     (forall E, open_wvl_subst_wvl_vnt E).
   Proof.
-    apply pre_val_ind; ii; ss.
-    all: repeat first [
-      des_goal; eqb2eq loc; clarify|
-      des_goal; eqb2eq nat; clarify].
+    apply pre_val_ind; ii; ss; repeat des_hyp; split_nIn;
+    repeat des_goal; repeat des_hyp;
+    try eqb2eq nat; try eqb2eq loc; try eqb2eq lbl; clarify.
     all: repeat match goal with
     | RR : open_wvl_subst_wvl_wvl _ |- _ => erewrite RR; eauto
     | RR : open_wvl_subst_wvl_nv _ |- _ => erewrite RR; eauto
@@ -546,40 +606,39 @@ Section SubstFacts.
     rw. eauto.
   Qed.
 
-  Definition open_wvl_subst_loc_wvl `{Eq loc} (w : wvl var loc lang) :=
+  Definition open_wvl_subst_loc_wvl `{Eq lbl} `{Eq loc} (w : wvl var lbl loc lang) :=
     forall i ℓ u ν,
       subst_loc_wvl ν ℓ (open_wvl_wvl i u w) =
       open_wvl_wvl i (subst_loc_wvl ν ℓ u) (subst_loc_wvl ν ℓ w)
   .
 
-  Definition open_wvl_subst_loc_nv `{Eq loc} (σ : nv var loc lang) :=
+  Definition open_wvl_subst_loc_nv `{Eq lbl} `{Eq loc} (σ : nv var lbl loc lang) :=
     forall i ℓ u ν,
       subst_loc_nv ν ℓ (open_wvl_nv i u σ) =
       open_wvl_nv i (subst_loc_wvl ν ℓ u) (subst_loc_nv ν ℓ σ)
   .
 
-  Definition open_wvl_subst_loc_vl `{Eq loc} (v : vl var loc lang) :=
+  Definition open_wvl_subst_loc_vl `{Eq lbl} `{Eq loc} (v : vl var lbl loc lang) :=
     forall i ℓ u ν,
       subst_loc_vl ν ℓ (open_wvl_vl i u v) =
       open_wvl_vl i (subst_loc_wvl ν ℓ u) (subst_loc_vl ν ℓ v)
   .
 
-  Definition open_wvl_subst_loc_vnt `{Eq loc} (E : vnt var loc lang) :=
+  Definition open_wvl_subst_loc_vnt `{Eq lbl} `{Eq loc} (E : vnt var lbl loc lang) :=
     forall i ℓ u ν,
       subst_loc_vnt ν ℓ (open_wvl_vnt i u E) =
       open_wvl_vnt i (subst_loc_wvl ν ℓ u) (subst_loc_vnt ν ℓ E)
   .
 
-  Lemma open_wvl_subst_loc `{Eq loc} :
+  Lemma open_wvl_subst_loc `{Eq lbl} `{Eq loc} :
     (forall w, open_wvl_subst_loc_wvl w) /\
     (forall σ, open_wvl_subst_loc_nv σ) /\
     (forall v, open_wvl_subst_loc_vl v) /\
     (forall E, open_wvl_subst_loc_vnt E).
   Proof.
-    apply pre_val_ind; ii; ss.
-    all: repeat first [
-      des_goal; eqb2eq loc; clarify|
-      des_goal; eqb2eq nat; clarify].
+    apply pre_val_ind; ii; ss; repeat des_hyp; split_nIn;
+    repeat des_goal; repeat des_hyp;
+    try eqb2eq nat; try eqb2eq loc; try eqb2eq lbl; clarify.
     all: repeat match goal with
     | RR : open_wvl_subst_loc_wvl _ |- _ => erewrite RR; eauto
     | RR : open_wvl_subst_loc_nv _ |- _ => erewrite RR; eauto
@@ -588,40 +647,39 @@ Section SubstFacts.
     end.
   Qed.
 
-  Definition open_loc_subst_wvl_wvl `{Eq loc} (w : wvl var loc lang) :=
+  Definition open_loc_subst_wvl_wvl `{Eq lbl} `{Eq loc} (w : wvl var lbl loc lang) :=
     forall i ℓ ν u (U : wvalue u) (NEQ : ℓ <> ν),
       subst_wvl_wvl u ℓ (open_loc_wvl i ν w) =
       open_loc_wvl i ν (subst_wvl_wvl u ℓ w)
   .
 
-  Definition open_loc_subst_wvl_nv `{Eq loc} (σ : nv var loc lang) :=
+  Definition open_loc_subst_wvl_nv `{Eq lbl} `{Eq loc} (σ : nv var lbl loc lang) :=
     forall i ℓ ν u (U : wvalue u) (NEQ : ℓ <> ν),
       subst_wvl_nv u ℓ (open_loc_nv i ν σ) =
       open_loc_nv i ν (subst_wvl_nv u ℓ σ)
   .
 
-  Definition open_loc_subst_wvl_vl `{Eq loc} (v : vl var loc lang) :=
+  Definition open_loc_subst_wvl_vl `{Eq lbl} `{Eq loc} (v : vl var lbl loc lang) :=
     forall i ℓ ν u (U : wvalue u) (NEQ : ℓ <> ν),
       subst_wvl_vl u ℓ (open_loc_vl i ν v) =
       open_loc_vl i ν (subst_wvl_vl u ℓ v)
   .
   
-  Definition open_loc_subst_wvl_vnt `{Eq loc} (E : vnt var loc lang) :=
+  Definition open_loc_subst_wvl_vnt `{Eq lbl} `{Eq loc} (E : vnt var lbl loc lang) :=
     forall i ℓ ν u (U : wvalue u) (NEQ : ℓ <> ν),
       subst_wvl_vnt u ℓ (open_loc_vnt i ν E) =
       open_loc_vnt i ν (subst_wvl_vnt u ℓ E)
   .
 
-  Lemma open_loc_subst_wvl `{Name loc} :
+  Lemma open_loc_subst_wvl `{Eq lbl} `{Name loc} :
     (forall w, open_loc_subst_wvl_wvl w) /\
     (forall σ, open_loc_subst_wvl_nv σ) /\
     (forall v, open_loc_subst_wvl_vl v) /\
     (forall E, open_loc_subst_wvl_vnt E).
   Proof.
-    apply pre_val_ind; ii; ss.
-    all: repeat first [
-      des_goal; eqb2eq loc; clarify|
-      des_goal; eqb2eq nat; clarify].
+    apply pre_val_ind; ii; ss; repeat des_hyp; split_nIn;
+    repeat des_goal; repeat des_hyp;
+    try eqb2eq nat; try eqb2eq loc; try eqb2eq lbl; clarify.
     all: repeat match goal with
     | RR : open_loc_subst_wvl_wvl _ |- _ => erewrite RR; eauto
     | RR : open_loc_subst_wvl_nv _ |- _ => erewrite RR; eauto
@@ -632,40 +690,39 @@ Section SubstFacts.
     rw. eauto.
   Qed.
 
-  Definition open_loc_subst_loc_wvl `{Eq loc} (w : wvl var loc lang) :=
+  Definition open_loc_subst_loc_wvl `{Eq lbl} `{Eq loc} (w : wvl var lbl loc lang) :=
     forall i ℓ ℓ' ν,
       subst_loc_wvl ν ℓ (open_loc_wvl i ℓ' w) =
       open_loc_wvl i (if eqb ℓ ℓ' then ν else ℓ') (subst_loc_wvl ν ℓ w)
   .
 
-  Definition open_loc_subst_loc_nv `{Eq loc} (σ : nv var loc lang) :=
+  Definition open_loc_subst_loc_nv `{Eq lbl} `{Eq loc} (σ : nv var lbl loc lang) :=
     forall i ℓ ℓ' ν,
       subst_loc_nv ν ℓ (open_loc_nv i ℓ' σ) =
       open_loc_nv i (if eqb ℓ ℓ' then ν else ℓ') (subst_loc_nv ν ℓ σ)
   .
 
-  Definition open_loc_subst_loc_vl `{Eq loc} (v : vl var loc lang) :=
+  Definition open_loc_subst_loc_vl `{Eq lbl} `{Eq loc} (v : vl var lbl loc lang) :=
     forall i ℓ ℓ' ν,
       subst_loc_vl ν ℓ (open_loc_vl i ℓ' v) =
       open_loc_vl i (if eqb ℓ ℓ' then ν else ℓ') (subst_loc_vl ν ℓ v)
   .
 
-  Definition open_loc_subst_loc_vnt `{Eq loc} (E : vnt var loc lang) :=
+  Definition open_loc_subst_loc_vnt `{Eq lbl} `{Eq loc} (E : vnt var lbl loc lang) :=
     forall i ℓ ℓ' ν,
       subst_loc_vnt ν ℓ (open_loc_vnt i ℓ' E) =
       open_loc_vnt i (if eqb ℓ ℓ' then ν else ℓ') (subst_loc_vnt ν ℓ E)
   .
 
-  Lemma open_loc_subst_loc `{Eq loc} :
+  Lemma open_loc_subst_loc `{Eq lbl} `{Eq loc} :
     (forall w, open_loc_subst_loc_wvl w) /\
     (forall σ, open_loc_subst_loc_nv σ) /\
     (forall v, open_loc_subst_loc_vl v) /\
     (forall E, open_loc_subst_loc_vnt E).
   Proof.
-    apply pre_val_ind; ii; ss.
-    all: repeat first [
-      des_goal; eqb2eq loc; clarify|
-      des_goal; eqb2eq nat; clarify].
+    apply pre_val_ind; ii; ss; repeat des_hyp; split_nIn;
+    repeat des_goal; repeat des_hyp;
+    try eqb2eq nat; try eqb2eq loc; try eqb2eq lbl; clarify.
     all: repeat match goal with
     | RR : open_loc_subst_loc_wvl _ |- _ => erewrite RR; eauto
     | RR : open_loc_subst_loc_nv _ |- _ => erewrite RR; eauto
@@ -674,36 +731,36 @@ Section SubstFacts.
     end.
     all: repeat first [
       rewrite eqb_refl; auto |
-      des_goal; eqb2eq loc; clarify].
+      des_goal | des_hyp | eqb2eq loc; clarify | eqb2eq lbl; clarify | ss].
   Qed.
 
-  Definition subst_wvl_close_wvl `{Eq loc} (w : wvl var loc lang) :=
-    forall i ℓ ν u
-      (NEQ : ℓ <> ν)
+  Definition subst_wvl_close_wvl `{Eq lbl} `{Eq loc} (w : wvl var lbl loc lang) :=
+    forall i ℓ p ν u
+      (NEQ : (ℓ, p) <> ν)
       (FRESH : ~ In ℓ (floc_wvl u)),
-    close_wvl i ℓ (subst_wvl_wvl u ν w) =
-    subst_wvl_wvl u ν (close_wvl i ℓ w).
+    close_wvl i (ℓ, p) (subst_wvl_wvl u ν w) =
+    subst_wvl_wvl u ν (close_wvl i (ℓ, p) w).
 
-  Definition subst_wvl_close_nv `{Eq loc} (σ : nv var loc lang) :=
-    forall i ℓ ν u
-      (NEQ : ℓ <> ν)
+  Definition subst_wvl_close_nv `{Eq lbl} `{Eq loc} (σ : nv var lbl loc lang) :=
+    forall i ℓ p ν u
+      (NEQ : (ℓ, p) <> ν)
       (FRESH : ~ In ℓ (floc_wvl u)),
-    close_nv i ℓ (subst_wvl_nv u ν σ) =
-    subst_wvl_nv u ν (close_nv i ℓ σ).
+    close_nv i (ℓ, p) (subst_wvl_nv u ν σ) =
+    subst_wvl_nv u ν (close_nv i (ℓ, p) σ).
 
-  Definition subst_wvl_close_vl `{Eq loc} (v : vl var loc lang) :=
-    forall i ℓ ν u
-      (NEQ : ℓ <> ν)
+  Definition subst_wvl_close_vl `{Eq lbl} `{Eq loc} (v : vl var lbl loc lang) :=
+    forall i ℓ p ν u
+      (NEQ : (ℓ, p) <> ν)
       (FRESH : ~ In ℓ (floc_wvl u)),
-    close_vl i ℓ (subst_wvl_vl u ν v) =
-    subst_wvl_vl u ν (close_vl i ℓ v).
+    close_vl i (ℓ, p) (subst_wvl_vl u ν v) =
+    subst_wvl_vl u ν (close_vl i (ℓ, p) v).
 
-  Definition subst_wvl_close_vnt `{Eq loc} (E : vnt var loc lang) :=
-    forall i ℓ ν u
-      (NEQ : ℓ <> ν)
+  Definition subst_wvl_close_vnt `{Eq lbl} `{Eq loc} (E : vnt var lbl loc lang) :=
+    forall i ℓ p ν u
+      (NEQ : (ℓ, p) <> ν)
       (FRESH : ~ In ℓ (floc_wvl u)),
-    close_vnt i ℓ (subst_wvl_vnt u ν E) =
-    subst_wvl_vnt u ν (close_vnt i ℓ E).
+    close_vnt i (ℓ, p) (subst_wvl_vnt u ν E) =
+    subst_wvl_vnt u ν (close_vnt i (ℓ, p) E).
 
   Ltac subst_wvl_close_tac :=
     repeat match goal with
@@ -713,41 +770,42 @@ Section SubstFacts.
     | H : subst_wvl_close_vnt _ |- _ => rewrite H; eauto
     end.
 
-  Lemma subst_wvl_close `{Eq loc} :
+  Lemma subst_wvl_close `{Eq lbl} `{Eq loc} :
     (forall w, subst_wvl_close_wvl w) /\
     (forall σ, subst_wvl_close_nv σ) /\
     (forall v, subst_wvl_close_vl v) /\
     (forall E, subst_wvl_close_vnt E).
   Proof.
     apply pre_val_ind; ii; ss; subst_wvl_close_tac.
-    repeat des_goal; repeat eqb2eq loc; clarify;
+    repeat des_goal; repeat des_hyp;
+    repeat eqb2eq loc; repeat eqb2eq lbl; clarify;
     subst_wvl_close_tac.
-    assert (close_fresh_wvl u) by apply close_fresh.
-    rw; eauto.
+    all: assert (close_fresh_wvl u) by apply close_fresh.
+    all: rw; eauto.
   Qed.
 
-  Definition subst_loc_close_wvl `{Eq loc} (w : wvl var loc lang) :=
+  Definition subst_loc_close_wvl `{Eq lbl} `{Eq loc} (w : wvl var lbl loc lang) :=
     forall i ℓ ν u
       (NEQ : ℓ <> ν)
       (FRESH : ℓ <> u),
     close_wvl i ℓ (subst_loc_wvl u ν w) =
     subst_loc_wvl u ν (close_wvl i ℓ w).
 
-  Definition subst_loc_close_nv `{Eq loc} (σ : nv var loc lang) :=
+  Definition subst_loc_close_nv `{Eq lbl} `{Eq loc} (σ : nv var lbl loc lang) :=
     forall i ℓ ν u
       (NEQ : ℓ <> ν)
       (FRESH : ℓ <> u),
     close_nv i ℓ (subst_loc_nv u ν σ) =
     subst_loc_nv u ν (close_nv i ℓ σ).
 
-  Definition subst_loc_close_vl `{Eq loc} (v : vl var loc lang) :=
+  Definition subst_loc_close_vl `{Eq lbl} `{Eq loc} (v : vl var lbl loc lang) :=
     forall i ℓ ν u
       (NEQ : ℓ <> ν)
       (FRESH : ℓ <> u),
     close_vl i ℓ (subst_loc_vl u ν v) =
     subst_loc_vl u ν (close_vl i ℓ v).
 
-  Definition subst_loc_close_vnt `{Eq loc} (E : vnt var loc lang) :=
+  Definition subst_loc_close_vnt `{Eq lbl} `{Eq loc} (E : vnt var lbl loc lang) :=
     forall i ℓ ν u
       (NEQ : ℓ <> ν)
       (FRESH : ℓ <> u),
@@ -762,339 +820,266 @@ Section SubstFacts.
     | H : subst_loc_close_vnt _ |- _ => rewrite H; eauto
     end.
 
-  Lemma subst_loc_close `{Eq loc} :
+  Lemma subst_loc_close `{Eq lbl} `{Eq loc} :
     (forall w, subst_loc_close_wvl w) /\
     (forall σ, subst_loc_close_nv σ) /\
     (forall v, subst_loc_close_vl v) /\
     (forall E, subst_loc_close_vnt E).
   Proof.
     apply pre_val_ind; ii; ss; subst_loc_close_tac.
-    repeat des_goal; repeat eqb2eq loc; clarify;
+    repeat des_goal; repeat des_hyp;
+    repeat eqb2eq loc; repeat eqb2eq lbl; clarify;
     subst_loc_close_tac.
   Qed.
-  
-  Definition floc_subst_loc_wvl `{Eq loc} (w : wvl var loc lang) :=
-    forall ℓ u x
-      (IN : In x (floc_wvl (subst_loc_wvl u ℓ w))),
-    (x <> ℓ /\ In x (floc_wvl w)) \/ x = u.
 
-  Definition floc_subst_loc_nv `{Eq loc} (σ : nv var loc lang) :=
-    forall ℓ u x
-      (IN : In x (floc_nv (subst_loc_nv u ℓ σ))),
-    (x <> ℓ /\ In x (floc_nv σ)) \/ x = u.
-
-  Definition floc_subst_loc_vl `{Eq loc} (v : vl var loc lang) :=
-    forall ℓ u x
-      (IN : In x (floc_vl (subst_loc_vl u ℓ v))),
-    (x <> ℓ /\ In x (floc_vl v)) \/ x = u.
-
-  Definition floc_subst_loc_vnt `{Eq loc} (E : vnt var loc lang) :=
-    forall ℓ u x
-      (IN : In x (floc_vnt (subst_loc_vnt u ℓ E))),
-    (x <> ℓ /\ In x (floc_vnt E)) \/ x = u.
-
-  Lemma floc_subst_loc `{Eq loc} :
-    (forall w, floc_subst_loc_wvl w) /\
-    (forall σ, floc_subst_loc_nv σ) /\
-    (forall v, floc_subst_loc_vl v) /\
-    (forall E, floc_subst_loc_vnt E).
-  Proof.
-    apply pre_val_ind; ii; ss;
-    try solve [exploit H0; eauto].
-    all: repeat des_hyp; repeat rewrite in_app_iff in *; des;
-    repeat eqb2eq loc; subst; try solve [auto];
-    match goal with
-    | H : floc_subst_loc_nv _ |- _ => solve [exploit H; eauto; ii; des; auto]
-    | H : floc_subst_loc_wvl _ |- _ => solve [exploit H; eauto; ii; des; auto]
-    | H : floc_subst_loc_vl _ |- _ => solve [exploit H; eauto; ii; des; auto]
-    | H : floc_subst_loc_vnt _ |- _ => solve [exploit H; eauto; ii; des; auto]
-    end.
-  Qed.
-
-  Definition floc_subst_wvl_wvl `{Eq loc} (w : wvl var loc lang) :=
-    forall ℓ u x
-      (IN : In x (floc_wvl (subst_wvl_wvl u ℓ w))),
-    (x <> ℓ /\ In x (floc_wvl w)) \/ In x (floc_wvl u).
-
-  Definition floc_subst_wvl_nv `{Eq loc} (σ : nv var loc lang) :=
-    forall ℓ u x
-      (IN : In x (floc_nv (subst_wvl_nv u ℓ σ))),
-    (x <> ℓ /\ In x (floc_nv σ)) \/ In x (floc_wvl u).
-
-  Definition floc_subst_wvl_vl `{Eq loc} (v : vl var loc lang) :=
-    forall ℓ u x
-      (IN : In x (floc_vl (subst_wvl_vl u ℓ v))),
-    (x <> ℓ /\ In x (floc_vl v)) \/ In x (floc_wvl u).
-
-  Definition floc_subst_wvl_vnt `{Eq loc} (E : vnt var loc lang) :=
-    forall ℓ u x
-      (IN : In x (floc_vnt (subst_wvl_vnt u ℓ E))),
-    (x <> ℓ /\ In x (floc_vnt E)) \/ In x (floc_wvl u).
-
-  Lemma floc_subst_wvl `{Eq loc} :
-    (forall w, floc_subst_wvl_wvl w) /\
-    (forall σ, floc_subst_wvl_nv σ) /\
-    (forall v, floc_subst_wvl_vl v) /\
-    (forall E, floc_subst_wvl_vnt E).
-  Proof.
-    apply pre_val_ind; ii; ss;
-    try solve [exploit H0; eauto].
-    all: repeat des_hyp; repeat rewrite in_app_iff in *; des;
-    repeat eqb2eq loc; subst; try solve [auto];
-    match goal with
-    | H : floc_subst_wvl_nv _ |- _ => solve [exploit H; eauto; ii; des; auto]
-    | H : floc_subst_wvl_wvl _ |- _ => solve [exploit H; eauto; ii; des; auto]
-    | H : floc_subst_wvl_vl _ |- _ => solve [exploit H; eauto; ii; des; auto]
-    | H : floc_subst_wvl_vnt _ |- _ => solve [exploit H; eauto; ii; des; auto]
-    end.
-  Qed.
-
-  Definition close_open_loc_eq_wvl `{Eq loc} (w : wvl var loc lang) :=
+  Definition close_open_loc_eq_wvl `{Eq lbl} `{Eq loc} (w : wvl var lbl loc lang) :=
     forall i ℓ ν,
       open_loc_wvl i ν (close_wvl i ℓ w) =
       subst_loc_wvl ν ℓ (open_loc_wvl i ℓ w).
 
-  Definition close_open_loc_eq_nv `{Eq loc} (σ : nv var loc lang) :=
+  Definition close_open_loc_eq_nv `{Eq lbl} `{Eq loc} (σ : nv var lbl loc lang) :=
     forall i ℓ ν,
       open_loc_nv i ν (close_nv i ℓ σ) =
       subst_loc_nv ν ℓ (open_loc_nv i ℓ σ).
 
-  Definition close_open_loc_eq_vl `{Eq loc} (v : vl var loc lang) :=
+  Definition close_open_loc_eq_vl `{Eq lbl} `{Eq loc} (v : vl var lbl loc lang) :=
     forall i ℓ ν,
       open_loc_vl i ν (close_vl i ℓ v) =
       subst_loc_vl ν ℓ (open_loc_vl i ℓ v).
 
-  Definition close_open_loc_eq_vnt `{Eq loc} (E : vnt var loc lang) :=
+  Definition close_open_loc_eq_vnt `{Eq lbl} `{Eq loc} (E : vnt var lbl loc lang) :=
     forall i ℓ ν,
       open_loc_vnt i ν (close_vnt i ℓ E) =
       subst_loc_vnt ν ℓ (open_loc_vnt i ℓ E).
 
-  Lemma close_open_loc_eq `{Eq loc} :
+  Lemma close_open_loc_eq `{Eq lbl} `{Eq loc} :
     (forall w, close_open_loc_eq_wvl w) /\
     (forall σ, close_open_loc_eq_nv σ) /\
     (forall v, close_open_loc_eq_vl v) /\
     (forall E, close_open_loc_eq_vnt E).
   Proof.
     apply pre_val_ind; ii; ss; try solve [repeat rw; eauto];
-    des_ifs; first [eqb2eq nat | eqb2eq loc]; clarify.
-    - rw. s. rewrite eqb_refl. eauto.
-    - rw. s. eauto.
-    - s. rewrite Nat.eqb_refl. rw. eauto.
-    - s. rw. eauto.
+    repeat des_goal; repeat des_hyp;
+    repeat first [eqb2eq nat | eqb2eq loc | eqb2eq lbl]; clarify;
+    try solve [rw; eauto].
   Qed.
 
-  Definition subst_loc_lc_wvl `{Eq loc} (w : wvl var loc lang) (W : wvalue w) :=
+  Definition subst_loc_lc_wvl `{Eq lbl} `{Eq loc} (w : wvl var lbl loc lang) (W : wvalue w) :=
     forall ℓ ν, wvalue (subst_loc_wvl ν ℓ w).
 
-  Definition subst_loc_lc_nv `{Eq loc} (σ : nv var loc lang) (Σ : env σ) :=
+  Definition subst_loc_lc_nv `{Eq lbl} `{Eq loc} (σ : nv var lbl loc lang) (Σ : env σ) :=
     forall ℓ ν, env (subst_loc_nv ν ℓ σ).
 
-  Definition subst_loc_lc_vl `{Eq loc} (v : vl var loc lang) (V : value v) :=
+  Definition subst_loc_lc_vl `{Eq lbl} `{Eq loc} (v : vl var lbl loc lang) (V : value v) :=
     forall ℓ ν, value (subst_loc_vl ν ℓ v).
 
-  Definition subst_loc_lc_vnt `{Eq loc} (E : vnt var loc lang) (EE : event E) :=
+  Definition subst_loc_lc_vnt `{Eq lbl} `{Eq loc} (E : vnt var lbl loc lang) (EE : event E) :=
     forall ℓ ν, event (subst_loc_vnt ν ℓ E).
 
-  Lemma subst_loc_lc `{Eq loc} :
+  Lemma subst_loc_lc `{Eq lbl} `{Eq loc} :
     (forall w W, subst_loc_lc_wvl w W) /\
     (forall σ Σ, subst_loc_lc_nv σ Σ) /\
     (forall v V, subst_loc_lc_vl v V) /\
     (forall E EE, subst_loc_lc_vnt E EE).
   Proof.
     apply val_ind; ii; ss;
-    try (des_ifs; eqb2eq loc);
+    try (repeat des_goal; repeat des_hyp;
+      repeat first [eqb2eq loc | eqb2eq lbl]; clarify);
     try solve [econstructor; eauto].
     econstructor.
-    instantiate (1 := ℓ :: L). ii. split_nIn.
+    instantiate (1 := fst ℓ :: L). ii. split_nIn.
     exploit VAL; eauto. ii.
     match goal with H : forall _, ~ In _ _ -> _ |- _ => exploit H; eauto end.
     instantiate (1 := ℓ). instantiate (1 := ν).
     assert (open_loc_subst_loc_vl v) by apply open_loc_subst_loc.
-    rw. des_ifs; eqb2eq loc; clarify.
+    rw. des_ifs. destruct ℓ; ss; des_hyp; eqb2eq loc; clarify.
   Qed.
 
-  Definition subst_wvl_lc_wvl `{Eq loc} (w : wvl var loc lang) (W : wvalue w) :=
+  Definition subst_wvl_lc_wvl `{Eq lbl} `{Eq loc} (w : wvl var lbl loc lang) (W : wvalue w) :=
     forall ℓ u (U : wvalue u), wvalue (subst_wvl_wvl u ℓ w).
 
-  Definition subst_wvl_lc_nv `{Eq loc} (σ : nv var loc lang) (Σ : env σ) :=
+  Definition subst_wvl_lc_nv `{Eq lbl} `{Eq loc} (σ : nv var lbl loc lang) (Σ : env σ) :=
     forall ℓ u (U : wvalue u), env (subst_wvl_nv u ℓ σ).
 
-  Definition subst_wvl_lc_vl `{Eq loc} (v : vl var loc lang) (V : value v) :=
+  Definition subst_wvl_lc_vl `{Eq lbl} `{Eq loc} (v : vl var lbl loc lang) (V : value v) :=
     forall ℓ u (U : wvalue u), value (subst_wvl_vl u ℓ v).
 
-  Definition subst_wvl_lc_vnt `{Eq loc} (E : vnt var loc lang) (EE : event E) :=
+  Definition subst_wvl_lc_vnt `{Eq lbl} `{Eq loc} (E : vnt var lbl loc lang) (EE : event E) :=
     forall ℓ u (U : wvalue u), event (subst_wvl_vnt u ℓ E).
 
-  Lemma subst_wvl_lc `{Name loc} :
+  Lemma subst_wvl_lc `{Eq lbl} `{Name loc} :
     (forall w W, subst_wvl_lc_wvl w W) /\
     (forall σ Σ, subst_wvl_lc_nv σ Σ) /\
     (forall v V, subst_wvl_lc_vl v V) /\
     (forall E EE, subst_wvl_lc_vnt E EE).
   Proof.
     apply val_ind; ii; ss;
-    try (des_ifs; eqb2eq loc);
+    try (repeat des_goal; repeat des_hyp;
+      repeat first [eqb2eq loc | eqb2eq lbl]; clarify);
     try solve [econstructor; eauto].
     econstructor.
-    instantiate (1 := ℓ :: L). ii. split_nIn.
+    instantiate (1 := fst ℓ :: L). ii. split_nIn.
     exploit VAL; eauto. ii.
     match goal with H : forall _, ~ In _ _ -> _ |- _ => exploit H; eauto end.
     instantiate (1 := ℓ).
     assert (open_loc_subst_wvl_vl v) by eapply open_loc_subst_wvl.
-    rw; eauto.
+    rw; eauto. destruct ℓ; ss; ii; clarify.
   Qed.
 
-  Definition map_close_wvl `{Eq loc} (w : wvl var loc lang) :=
-    forall i ℓ φ (INJ : oto φ),
-      map_wvl φ (close_wvl i ℓ w) = close_wvl i (φ ℓ) (map_wvl φ w).
+  Definition map_close_wvl `{Eq lbl} `{Eq loc} (w : wvl var lbl loc lang) :=
+    forall i ℓ p φ (INJ : oto φ),
+      map_wvl φ (close_wvl i (ℓ, p) w) = close_wvl i (φ ℓ, p) (map_wvl φ w).
 
-  Definition map_close_nv `{Eq loc} (σ : nv var loc lang) :=
-    forall i ℓ φ (INJ : oto φ),
-      map_nv φ (close_nv i ℓ σ) = close_nv i (φ ℓ) (map_nv φ σ).
+  Definition map_close_nv `{Eq lbl} `{Eq loc} (σ : nv var lbl loc lang) :=
+    forall i ℓ p φ (INJ : oto φ),
+      map_nv φ (close_nv i (ℓ, p) σ) = close_nv i (φ ℓ, p) (map_nv φ σ).
 
-  Definition map_close_vl `{Eq loc} (v : vl var loc lang) :=
-    forall i ℓ φ (INJ : oto φ),
-      map_vl φ (close_vl i ℓ v) = close_vl i (φ ℓ) (map_vl φ v).
+  Definition map_close_vl `{Eq lbl} `{Eq loc} (v : vl var lbl loc lang) :=
+    forall i ℓ p φ (INJ : oto φ),
+      map_vl φ (close_vl i (ℓ, p) v) = close_vl i (φ ℓ, p) (map_vl φ v).
 
-  Definition map_close_vnt `{Eq loc} (E : vnt var loc lang) :=
-    forall i ℓ φ (INJ : oto φ),
-      map_vnt φ (close_vnt i ℓ E) = close_vnt i (φ ℓ) (map_vnt φ E).
+  Definition map_close_vnt `{Eq lbl} `{Eq loc} (E : vnt var lbl loc lang) :=
+    forall i ℓ p φ (INJ : oto φ),
+      map_vnt φ (close_vnt i (ℓ, p) E) = close_vnt i (φ ℓ, p) (map_vnt φ E).
 
-  Lemma map_close `{Eq loc} :
+  Lemma map_close `{Eq lbl} `{Eq loc} :
     (forall w, map_close_wvl w) /\
     (forall σ, map_close_nv σ) /\
     (forall v, map_close_vl v) /\
     (forall E, map_close_vnt E).
   Proof.
     apply pre_val_ind; ii; ss; unfold oto in INJ; repeat rw; eauto.
-    des_ifs.
-    all: repeat (eqb2eq loc; clarify; ss).
+    repeat des_goal; repeat des_hyp.
+    all: repeat first [eqb2eq loc | eqb2eq lbl]; clarify; ss.
     all: repeat rw; eauto.
-    apply INJ in Heq0; clarify.
+    all: match goal with
+    | H : ?φ _ = ?φ _ |- _ => apply INJ in H; clarify
+    end.
   Qed.
 
-  Definition map_open_wvl_wvl `{Eq loc} (w : wvl var loc lang) :=
+  Definition map_open_wvl_wvl `{Eq lbl} `{Eq loc} (w : wvl var lbl loc lang) :=
     forall i u φ,
       map_wvl φ (open_wvl_wvl i u w) = open_wvl_wvl i (map_wvl φ u) (map_wvl φ w).
 
-  Definition map_open_wvl_nv `{Eq loc} (σ : nv var loc lang) :=
+  Definition map_open_wvl_nv `{Eq lbl} `{Eq loc} (σ : nv var lbl loc lang) :=
     forall i u φ,
       map_nv φ (open_wvl_nv i u σ) = open_wvl_nv i (map_wvl φ u) (map_nv φ σ).
 
-  Definition map_open_wvl_vl `{Eq loc} (v : vl var loc lang) :=
+  Definition map_open_wvl_vl `{Eq lbl} `{Eq loc} (v : vl var lbl loc lang) :=
     forall i u φ,
       map_vl φ (open_wvl_vl i u v) = open_wvl_vl i (map_wvl φ u) (map_vl φ v).
 
-  Definition map_open_wvl_vnt `{Eq loc} (E : vnt var loc lang) :=
+  Definition map_open_wvl_vnt `{Eq lbl} `{Eq loc} (E : vnt var lbl loc lang) :=
     forall i u φ,
       map_vnt φ (open_wvl_vnt i u E) = open_wvl_vnt i (map_wvl φ u) (map_vnt φ E).
 
-  Lemma map_open_wvl `{Eq loc} :
+  Lemma map_open_wvl `{Eq lbl} `{Eq loc} :
     (forall w, map_open_wvl_wvl w) /\
     (forall σ, map_open_wvl_nv σ) /\
     (forall v, map_open_wvl_vl v) /\
     (forall E, map_open_wvl_vnt E).
   Proof.
     apply pre_val_ind; ii; ss; repeat rw; eauto.
-    des_ifs.
-    all: repeat (eqb2eq nat; clarify; ss).
-    all: repeat rw; eauto.
+    repeat des_goal; repeat des_hyp.
+    all: repeat first [eqb2eq loc | eqb2eq lbl]; clarify; ss.
+    all: repeat rw; repeat des_goal; eauto.
   Qed.
 
-  Definition map_open_loc_wvl `{Eq loc} (w : wvl var loc lang) :=
-    forall i u φ,
-      map_wvl φ (open_loc_wvl i u w) = open_loc_wvl i (φ u) (map_wvl φ w).
+  Definition map_open_loc_wvl `{Eq lbl} `{Eq loc} (w : wvl var lbl loc lang) :=
+    forall i u p φ,
+      map_wvl φ (open_loc_wvl i (u, p) w) = open_loc_wvl i (φ u, p) (map_wvl φ w).
 
-  Definition map_open_loc_nv `{Eq loc} (σ : nv var loc lang) :=
-    forall i u φ,
-      map_nv φ (open_loc_nv i u σ) = open_loc_nv i (φ u) (map_nv φ σ).
+  Definition map_open_loc_nv `{Eq lbl} `{Eq loc} (σ : nv var lbl loc lang) :=
+    forall i u p φ,
+      map_nv φ (open_loc_nv i (u, p) σ) = open_loc_nv i (φ u, p) (map_nv φ σ).
 
-  Definition map_open_loc_vl `{Eq loc} (v : vl var loc lang) :=
-    forall i u φ,
-      map_vl φ (open_loc_vl i u v) = open_loc_vl i (φ u) (map_vl φ v).
+  Definition map_open_loc_vl `{Eq lbl} `{Eq loc} (v : vl var lbl loc lang) :=
+    forall i u p φ,
+      map_vl φ (open_loc_vl i (u, p) v) = open_loc_vl i (φ u, p) (map_vl φ v).
 
-  Definition map_open_loc_vnt `{Eq loc} (E : vnt var loc lang) :=
-    forall i u φ,
-      map_vnt φ (open_loc_vnt i u E) = open_loc_vnt i (φ u) (map_vnt φ E).
+  Definition map_open_loc_vnt `{Eq lbl} `{Eq loc} (E : vnt var lbl loc lang) :=
+    forall i u p φ,
+      map_vnt φ (open_loc_vnt i (u, p) E) = open_loc_vnt i (φ u, p) (map_vnt φ E).
 
-  Lemma map_open_loc `{Eq loc} :
+  Lemma map_open_loc `{Eq lbl} `{Eq loc} :
     (forall w, map_open_loc_wvl w) /\
     (forall σ, map_open_loc_nv σ) /\
     (forall v, map_open_loc_vl v) /\
     (forall E, map_open_loc_vnt E).
   Proof.
     apply pre_val_ind; ii; ss; repeat rw; eauto.
-    des_ifs.
-    all: repeat (eqb2eq nat; clarify; ss).
-    all: repeat rw; eauto.
+    repeat des_goal; repeat des_hyp.
+    all: repeat first [eqb2eq loc | eqb2eq lbl]; clarify; ss.
+    all: repeat rw; repeat des_goal; eauto.
   Qed.
 
-  Definition floc_map_wvl `{Eq loc} (w : wvl var loc lang) :=
+  Definition floc_map_wvl `{Eq lbl} `{Eq loc} (w : wvl var lbl loc lang) :=
     forall ℓ φ (IN : In ℓ (floc_wvl w)),
       In (φ ℓ) (floc_wvl (map_wvl φ w)).
 
-  Definition floc_map_nv `{Eq loc} (σ : nv var loc lang) :=
+  Definition floc_map_nv `{Eq lbl} `{Eq loc} (σ : nv var lbl loc lang) :=
     forall ℓ φ (IN : In ℓ (floc_nv σ)),
       In (φ ℓ) (floc_nv (map_nv φ σ)).
 
-  Definition floc_map_vl `{Eq loc} (v : vl var loc lang) :=
+  Definition floc_map_vl `{Eq lbl} `{Eq loc} (v : vl var lbl loc lang) :=
     forall ℓ φ (IN : In ℓ (floc_vl v)),
       In (φ ℓ) (floc_vl (map_vl φ v)).
 
-  Definition floc_map_vnt `{Eq loc} (E : vnt var loc lang) :=
+  Definition floc_map_vnt `{Eq lbl} `{Eq loc} (E : vnt var lbl loc lang) :=
     forall ℓ φ (IN : In ℓ (floc_vnt E)),
       In (φ ℓ) (floc_vnt (map_vnt φ E)).
 
-  Lemma floc_map `{Eq loc} :
+  Lemma floc_map `{Eq lbl} `{Eq loc} :
     (forall w, floc_map_wvl w) /\
     (forall σ, floc_map_nv σ) /\
     (forall v, floc_map_vl v) /\
     (forall E, floc_map_vnt E).
   Proof.
-    apply pre_val_ind; ii; ss; des; clarify; auto.
-    all: rewrite in_app_iff in *; des; auto.
+    apply pre_val_ind; ii; ss; repeat des_hyp; des; clarify; ss; auto.
+    all: rewrite in_app_iff in *; des; clarify; auto.
   Qed.
 
-  Definition map_floc_wvl `{Eq loc} (w : wvl var loc lang) :=
+  Definition map_floc_wvl `{Eq lbl} `{Eq loc} (w : wvl var lbl loc lang) :=
     forall ℓ φ (INJ : oto φ)
       (IN : In (φ ℓ) (floc_wvl (map_wvl φ w))),
     In ℓ (floc_wvl w).
 
-  Definition map_floc_nv `{Eq loc} (σ : nv var loc lang) :=
+  Definition map_floc_nv `{Eq lbl} `{Eq loc} (σ : nv var lbl loc lang) :=
     forall ℓ φ (INJ : oto φ)
       (IN : In (φ ℓ) (floc_nv (map_nv φ σ))),
     In ℓ (floc_nv σ).
 
-  Definition map_floc_vl `{Eq loc} (v : vl var loc lang) :=
+  Definition map_floc_vl `{Eq lbl} `{Eq loc} (v : vl var lbl loc lang) :=
     forall ℓ φ (INJ : oto φ)
       (IN : In (φ ℓ) (floc_vl (map_vl φ v))),
     In ℓ (floc_vl v).
 
-  Definition map_floc_vnt `{Eq loc} (E : vnt var loc lang) :=
+  Definition map_floc_vnt `{Eq lbl} `{Eq loc} (E : vnt var lbl loc lang) :=
     forall ℓ φ (INJ : oto φ)
       (IN : In (φ ℓ) (floc_vnt (map_vnt φ E))),
     In ℓ (floc_vnt E).
  
-  Lemma map_floc `{Eq loc} :
+  Lemma map_floc `{Eq lbl} `{Eq loc} :
     (forall w, map_floc_wvl w) /\
     (forall σ, map_floc_nv σ) /\
     (forall v, map_floc_vl v) /\
     (forall E, map_floc_vnt E).
   Proof.
     apply pre_val_ind; ii; ss; eauto;
-    des; eauto.
+    repeat des_hyp; ss; des; eauto.
     all: rewrite in_app_iff in *; ss; des; eauto.
   Qed.
 
-  Definition map_id_is_id_wvl (w : wvl var loc lang) :=
+  Definition map_id_is_id_wvl (w : wvl var lbl loc lang) :=
     map_wvl id w = w.
 
-  Definition map_id_is_id_nv (σ : nv var loc lang) :=
+  Definition map_id_is_id_nv (σ : nv var lbl loc lang) :=
     map_nv id σ = σ.
 
-  Definition map_id_is_id_vl (v : vl var loc lang) :=
+  Definition map_id_is_id_vl (v : vl var lbl loc lang) :=
     map_vl id v = v.
 
-  Definition map_id_is_id_vnt (E : vnt var loc lang) :=
+  Definition map_id_is_id_vnt (E : vnt var lbl loc lang) :=
     map_vnt id E = E.
   
   Lemma map_id_is_id :
@@ -1103,80 +1088,92 @@ Section SubstFacts.
     (forall v, map_id_is_id_vl v) /\
     (forall E, map_id_is_id_vnt E).
   Proof.
-    apply pre_val_ind; ii; red; s; repeat rw; eauto.
+    apply pre_val_ind; ii; red; s; repeat rw; des_ifs; eauto.
   Qed.
 
-  Definition swap_is_subst_wvl `{Eq loc} (w : wvl var loc lang) :=
-    forall φ (INJ : oto φ)
-      ℓ ν (FRESH : ~ In ℓ (floc_wvl w)),
-      map_wvl (swap φ ℓ ν) w = subst_loc_wvl (φ ℓ) (φ ν) (map_wvl φ w).
+  Definition swap_is_subst_wvl `{Eq lbl} `{Eq loc} (w : wvl var lbl loc lang) :=
+    forall φ (INJ : oto φ) ℓ ν p
+      (FRESH : ~ In ℓ (floc_wvl w)) (UNIQUE : forall p', In (ν, p') (flloc_wvl w) -> p' = p),
+      map_wvl (swap φ ℓ ν) w = subst_loc_wvl (φ ℓ, p) (φ ν, p) (map_wvl φ w).
 
-  Definition swap_is_subst_nv `{Eq loc} (σ : nv var loc lang) :=
-    forall φ (INJ : oto φ)
-      ℓ ν (FRESH : ~ In ℓ (floc_nv σ)),
-      map_nv (swap φ ℓ ν) σ = subst_loc_nv (φ ℓ) (φ ν) (map_nv φ σ).
+  Definition swap_is_subst_nv `{Eq lbl} `{Eq loc} (σ : nv var lbl loc lang) :=
+    forall φ (INJ : oto φ) ℓ ν p
+      (FRESH : ~ In ℓ (floc_nv σ)) (UNIQUE : forall p', In (ν, p') (flloc_nv σ) -> p' = p),
+      map_nv (swap φ ℓ ν) σ = subst_loc_nv (φ ℓ, p) (φ ν, p) (map_nv φ σ).
 
-  Definition swap_is_subst_vl `{Eq loc} (v : vl var loc lang) :=
-    forall φ (INJ : oto φ)
-      ℓ ν (FRESH : ~ In ℓ (floc_vl v)),
-      map_vl (swap φ ℓ ν) v = subst_loc_vl (φ ℓ) (φ ν) (map_vl φ v).
+  Definition swap_is_subst_vl `{Eq lbl} `{Eq loc} (v : vl var lbl loc lang) :=
+    forall φ (INJ : oto φ) ℓ ν p
+      (FRESH : ~ In ℓ (floc_vl v)) (UNIQUE : forall p', In (ν, p') (flloc_vl v) -> p' = p),
+      map_vl (swap φ ℓ ν) v = subst_loc_vl (φ ℓ, p) (φ ν, p) (map_vl φ v).
 
-  Definition swap_is_subst_vnt `{Eq loc} (E : vnt var loc lang) :=
-    forall φ (INJ : oto φ)
-      ℓ ν (FRESH : ~ In ℓ (floc_vnt E)),
-      map_vnt (swap φ ℓ ν) E = subst_loc_vnt (φ ℓ) (φ ν) (map_vnt φ E).
+  Definition swap_is_subst_vnt `{Eq lbl} `{Eq loc} (E : vnt var lbl loc lang) :=
+    forall φ (INJ : oto φ) ℓ ν p
+      (FRESH : ~ In ℓ (floc_vnt E)) (UNIQUE : forall p', In (ν, p') (flloc_vnt E) -> p' = p),
+      map_vnt (swap φ ℓ ν) E = subst_loc_vnt (φ ℓ, p) (φ ν, p) (map_vnt φ E).
 
-  Lemma swap_is_subst `{Eq loc} :
+  Lemma swap_is_subst `{Eq lbl} `{Eq loc} :
     (forall w, swap_is_subst_wvl w) /\
     (forall σ, swap_is_subst_nv σ) /\
     (forall v, swap_is_subst_vl v) /\
     (forall E, swap_is_subst_vnt E).
   Proof.
-    apply pre_val_ind; ii; ss; unfold oto in INJ; repeat rw; split_nIn; eauto.
-    unfold swap; des_ifs; repeat eqb2eq loc; clarify.
-    exploit INJ; eauto; ii; clarify.
+    apply pre_val_ind; ii; ss; des_ifs;
+    repeat match goal with
+    | RR : swap_is_subst_wvl _ |- _ => rewrite RR
+    | RR : swap_is_subst_nv _ |- _ => rewrite RR
+    | RR : swap_is_subst_vl _ |- _ => rewrite RR
+    | RR : swap_is_subst_vnt _ |- _ => rewrite RR
+    end; split_nIn; eauto.
+    all: try solve [ii; apply UNIQUE; rewrite in_app_iff; eauto].
+    unfold swap; repeat des_goal; repeat des_hyp;
+    repeat first [rewrite eqb_eq in * | rewrite eqb_neq in *]; clarify.
+    all: match goal with
+    | _ => solve [exfalso; try_all; symmetry; apply UNIQUE; auto]
+    | H : ?φ _ = ?φ _ |- _ => apply INJ in H; split_nIn; clarify
+    end.
   Qed.
 
-  Definition subst_loc_close_eq_wvl `{Eq loc} (w : wvl var loc lang) :=
-    forall i ℓ ν (FRESH : ~ In ℓ (floc_wvl w)),
+  Definition subst_loc_close_eq_wvl `{Eq lbl} `{Eq loc} (w : wvl var lbl loc lang) :=
+    forall i ℓ ν (FRESH : ~ In ℓ (flloc_wvl w)),
       close_wvl i ℓ (subst_loc_wvl ℓ ν w) = close_wvl i ν w.
 
-  Definition subst_loc_close_eq_nv `{Eq loc} (σ : nv var loc lang) :=
-    forall i ℓ ν (FRESH : ~ In ℓ (floc_nv σ)),
+  Definition subst_loc_close_eq_nv `{Eq lbl} `{Eq loc} (σ : nv var lbl loc lang) :=
+    forall i ℓ ν (FRESH : ~ In ℓ (flloc_nv σ)),
       close_nv i ℓ (subst_loc_nv ℓ ν σ) = close_nv i ν σ.
 
-  Definition subst_loc_close_eq_vl `{Eq loc} (v : vl var loc lang) :=
-    forall i ℓ ν (FRESH : ~ In ℓ (floc_vl v)),
+  Definition subst_loc_close_eq_vl `{Eq lbl} `{Eq loc} (v : vl var lbl loc lang) :=
+    forall i ℓ ν (FRESH : ~ In ℓ (flloc_vl v)),
       close_vl i ℓ (subst_loc_vl ℓ ν v) = close_vl i ν v.
 
-  Definition subst_loc_close_eq_vnt `{Eq loc} (E : vnt var loc lang) :=
-    forall i ℓ ν (FRESH : ~ In ℓ (floc_vnt E)),
+  Definition subst_loc_close_eq_vnt `{Eq lbl} `{Eq loc} (E : vnt var lbl loc lang) :=
+    forall i ℓ ν (FRESH : ~ In ℓ (flloc_vnt E)),
       close_vnt i ℓ (subst_loc_vnt ℓ ν E) = close_vnt i ν E.
 
-  Lemma subst_loc_close_eq `{Eq loc} :
+  Lemma subst_loc_close_eq `{Eq lbl} `{Eq loc} :
     (forall w, subst_loc_close_eq_wvl w) /\
     (forall σ, subst_loc_close_eq_nv σ) /\
     (forall v, subst_loc_close_eq_vl v) /\
     (forall E, subst_loc_close_eq_vnt E).
   Proof.
     apply pre_val_ind; ii; ss; repeat rw; split_nIn; eauto.
-    do 2 (des_ifs; eqb2eq loc; clarify; s);
-    rw; eauto.
+    repeat des_goal; repeat des_hyp;
+    repeat first [rewrite eqb_eq in * | rewrite eqb_neq in *]; clarify.
+    all: rw; eauto.
   Qed.
 
-  Definition map_ext_wvl (w : wvl var loc lang) :=
+  Definition map_ext_wvl (w : wvl var lbl loc lang) :=
     forall φ ϕ (EXT : forall ℓ (DOM : In ℓ (floc_wvl w)), φ ℓ = ϕ ℓ),
       map_wvl φ w = map_wvl ϕ w.
 
-  Definition map_ext_nv (σ : nv var loc lang) :=
+  Definition map_ext_nv (σ : nv var lbl loc lang) :=
     forall φ ϕ (EXT : forall ℓ (DOM : In ℓ (floc_nv σ)), φ ℓ = ϕ ℓ),
       map_nv φ σ = map_nv ϕ σ.
 
-  Definition map_ext_vl (v : vl var loc lang) :=
+  Definition map_ext_vl (v : vl var lbl loc lang) :=
     forall φ ϕ (EXT : forall ℓ (DOM : In ℓ (floc_vl v)), φ ℓ = ϕ ℓ),
       map_vl φ v = map_vl ϕ v.
 
-  Definition map_ext_vnt (E : vnt var loc lang) :=
+  Definition map_ext_vnt (E : vnt var lbl loc lang) :=
     forall φ ϕ (EXT : forall ℓ (DOM : In ℓ (floc_vnt E)), φ ℓ = ϕ ℓ),
       map_vnt φ E = map_vnt ϕ E.
   
@@ -1193,27 +1190,25 @@ Section SubstFacts.
     | RR : map_ext_vl _ |- _ => erewrite (RR φ ϕ); eauto
     | RR : map_ext_vnt _ |- _ => erewrite (RR φ ϕ); eauto
     end.
-    erewrite EXT; eauto.
-    all:ii; apply EXT; rewrite in_app_iff; eauto.
+    des_goal; erewrite EXT; ss; clarify; auto.
+    all:ii; apply EXT; first [des_goal | rewrite in_app_iff]; eauto.
   Qed.
 
-  Definition compose (f g : loc -> loc) ℓ := f (g ℓ).
-
-  Definition map_compose_wvl (w : wvl var loc lang) :=
+  Definition map_compose_wvl (w : wvl var lbl loc lang) :=
     forall φ ϕ,
-      map_wvl φ (map_wvl ϕ w) = map_wvl (compose φ ϕ) w.
+      map_wvl φ (map_wvl ϕ w) = map_wvl (φ <*> ϕ) w.
 
-  Definition map_compose_nv (σ : nv var loc lang) :=
+  Definition map_compose_nv (σ : nv var lbl loc lang) :=
     forall φ ϕ,
-      map_nv φ (map_nv ϕ σ) = map_nv (compose φ ϕ) σ.
+      map_nv φ (map_nv ϕ σ) = map_nv (φ <*> ϕ) σ.
 
-  Definition map_compose_vl (v : vl var loc lang) :=
+  Definition map_compose_vl (v : vl var lbl loc lang) :=
     forall φ ϕ,
-      map_vl φ (map_vl ϕ v) = map_vl (compose φ ϕ) v.
+      map_vl φ (map_vl ϕ v) = map_vl (φ <*> ϕ) v.
 
-  Definition map_compose_vnt (E : vnt var loc lang) :=
+  Definition map_compose_vnt (E : vnt var lbl loc lang) :=
     forall φ ϕ,
-      map_vnt φ (map_vnt ϕ E) = map_vnt (compose φ ϕ) E.
+      map_vnt φ (map_vnt ϕ E) = map_vnt (φ <*> ϕ) E.
 
   Lemma map_compose :
     (forall w, map_compose_wvl w) /\
@@ -1221,59 +1216,60 @@ Section SubstFacts.
     (forall v, map_compose_vl v) /\
     (forall E, map_compose_vnt E).
   Proof.
-    apply pre_val_ind; ii; ss; repeat rw; auto.
+    apply pre_val_ind; ii; ss; des_ifs; ss; repeat rw; auto.
   Qed.
 
-  Definition map_lc_wvl (w : wvl var loc lang) (W : wvalue w) :=
+  Definition map_lc_wvl (w : wvl var lbl loc lang) (W : wvalue w) :=
     forall φ, wvalue (map_wvl φ w).
 
-  Definition map_lc_nv (σ : nv var loc lang) (Σ : env σ) :=
+  Definition map_lc_nv (σ : nv var lbl loc lang) (Σ : env σ) :=
     forall φ, env (map_nv φ σ).
 
-  Definition map_lc_vl (v : vl var loc lang) (V : value v) :=
+  Definition map_lc_vl (v : vl var lbl loc lang) (V : value v) :=
     forall φ, value (map_vl φ v).
 
-  Definition map_lc_vnt (E : vnt var loc lang) (EE : event E) :=
+  Definition map_lc_vnt (E : vnt var lbl loc lang) (EE : event E) :=
     forall φ, event (map_vnt φ E).
 
-  Lemma map_lc `{Name loc} :
+  Lemma map_lc `{Eq lbl} `{Name loc} :
     (forall w W, map_lc_wvl w W) /\
     (forall σ Σ, map_lc_nv σ Σ) /\
     (forall v V, map_lc_vl v V) /\
     (forall E EE, map_lc_vnt E EE).
   Proof.
-    apply val_ind; ii; ss; econstructor; eauto.
+    apply val_ind; ii; ss; des_ifs; econstructor; eauto.
     instantiate (1 := []).
     ii. gensym_tac (L ++ floc_vl v) ν.
-    exploit H1; eauto.
+    match goal with H : forall _, ~ In _ _ -> map_lc_vl _ _ |- _ => exploit H; eauto end.
     instantiate (1 := fun x => if eqb x ν then ℓ else φ x).
-    assert (map_open_loc_vl v) by apply map_open_loc.
+    assert (map_open_loc_vl v) by eapply map_open_loc.
     rw. rewrite eqb_refl.
     assert (map_ext_vl v) as RR by apply map_ext.
-    erewrite RR; eauto.
-    ii. des_ifs; eqb2eq loc; clarify.
+    erewrite RR; eauto. clear RR.
+    ii. des_goal; first [rewrite eqb_eq in * | rewrite eqb_neq in *]; clarify.
   Qed.
 
-  Definition subst_id_wvl `{Eq loc} (w : wvl var loc lang) :=
+  Definition subst_id_wvl `{Eq lbl} `{Eq loc} (w : wvl var lbl loc lang) :=
     forall ℓ, subst_loc_wvl ℓ ℓ w = w.
 
-  Definition subst_id_nv `{Eq loc} (σ : nv var loc lang) :=
+  Definition subst_id_nv `{Eq lbl} `{Eq loc} (σ : nv var lbl loc lang) :=
     forall ℓ, subst_loc_nv ℓ ℓ σ = σ.
 
-  Definition subst_id_vl `{Eq loc} (v : vl var loc lang) :=
+  Definition subst_id_vl `{Eq lbl} `{Eq loc} (v : vl var lbl loc lang) :=
     forall ℓ, subst_loc_vl ℓ ℓ v = v.
 
-  Definition subst_id_vnt `{Eq loc} (E : vnt var loc lang) :=
+  Definition subst_id_vnt `{Eq lbl} `{Eq loc} (E : vnt var lbl loc lang) :=
     forall ℓ, subst_loc_vnt ℓ ℓ E = E.
   
-  Lemma subst_id `{Eq loc} :
+  Lemma subst_id `{Eq lbl} `{Eq loc} :
     (forall w, subst_id_wvl w) /\
     (forall σ, subst_id_nv σ) /\
     (forall v, subst_id_vl v) /\
     (forall E, subst_id_vnt E).
   Proof.
     apply pre_val_ind; ii; ss; repeat rw; eauto;
-    des_ifs; eqb2eq loc; clarify.
+    repeat des_goal; repeat des_hyp;
+    repeat first [eqb2eq loc | eqb2eq lbl]; clarify.
   Qed.
 End SubstFacts.
 
