new-semantics/coq/abstract/Syntax.v
@@ -1,3 +1,5 @@
+From Basics Require Import Basics.
+(* term *)
 Inductive tm {var lbl} :=
 | tm_var (p : lbl) (x : var)
 | tm_lam (p : lbl) (x : var) (t : tm)
@@ -7,23 +9,69 @@ Inductive tm {var lbl} :=
 | tm_bind (p : lbl) (x : var) (t1 t2 : tm)
 .
 
+(* labelled term *)
+Variant ltm {var lbl} :=
+| ltm_var (x : var)
+| ltm_lam (x : var) (p' : lbl)
+| ltm_app (p1 p2 : lbl)
+| ltm_link (p1 p2 : lbl)
+| ltm_mt
+| ltm_bind (x : var) (p1 p2 : lbl)
+.
+
 Variant val {var lbl} :=
 | v_fn (x : var) (t : @tm var lbl)
 .
 
+Variant lval {var lbl} :=
+| lv_fn (x : var) (p : lbl)
+.
+
 Definition get_lbl {var lbl} (t : @tm var lbl) :=
-match t with
-  tm_var p _ | tm_lam p _ _ | tm_app p _ _ | tm_link p _ _ | tm_mt p | tm_bind p _ _ _ => p
-end.
+  match t with
+    tm_var p _ | tm_lam p _ _ | tm_app p _ _ | tm_link p _ _ | tm_mt p | tm_bind p _ _ _ => p
+  end.
 
-Fixpoint subexpr {var lbl} (s t : @tm var lbl) :=
-s = t \/
-match t with
-| tm_app _ t1 t2 | tm_link _ t1 t2 | tm_bind _ _ t1 t2 => subexpr s t1 \/ subexpr s t2
-| tm_lam _ _ t' => subexpr s t'
-| _ => False
-end.
+Fixpoint is_repr {var lbl} (t : @tm var lbl) (g : lbl -> ltm) :=
+  match t with
+  | tm_var p x =>
+    g p = ltm_var x
+  | tm_lam p x t =>
+    g p = ltm_lam x (get_lbl t) /\ is_repr t g
+  | tm_app p t1 t2 =>
+    g p = ltm_app (get_lbl t1) (get_lbl t2) /\ is_repr t1 g /\ is_repr t2 g
+  | tm_link p t1 t2 =>
+    g p = ltm_link (get_lbl t1) (get_lbl t2) /\ is_repr t1 g /\ is_repr t2 g
+  | tm_mt p =>
+    g p = ltm_mt
+  | tm_bind p x t1 t2 =>
+    g p = ltm_bind x (get_lbl t1) (get_lbl t2) /\ is_repr t1 g /\ is_repr t2 g
+  end
+.
 
-Notation "s '∈' t" := (subexpr s t)
-  (at level 100, t at next level, right associativity).
+Notation "t '∈' g" := (is_repr t g)
+  (at level 100, g at next level, right associativity).
+
+Variant avnt {var lbl} :=
+| AInit
+| ARead (p : lbl) (x : var)
+| ACall (p1 p2 : lbl)
+.
+
+Definition abs_env {var lbl} : Type := (var -> list lbl) * list (@avnt var lbl).
+
+Definition abs_val {var lbl} : Type := @abs_env var lbl * list (@lval var lbl * lbl).
+
+Definition abs_sem {var lbl} := lbl -> (@abs_env var lbl * @abs_val var lbl).
+
+Definition geq {var lbl} (v1 v2 : @abs_val var lbl) :=
+  match v1, v2 with
+  | ((σ1, E1), λ1), ((σ2, E2), λ2) =>
+    (forall x p, In p (σ2 x) -> In p (σ1 x)) /\
+    (forall E, In E E2 -> In E E1) /\
+    (forall λ, In λ λ2 -> In λ λ1)
+  end.
+
+Notation "v1 '⊒' v2" := (geq v1 v2)
+  (at level 100, v2 at next level, right associativity).
 
