new-semantics/coq/events/Advance.v
@@ -9,28 +9,27 @@ From With_events Require Import LinkFacts.
 From With_events Require Import EquivLink.
 
 Section Advance.
-  Variable var : Type.
-  Variable loc : Type.
+  Context {var lbl loc : Type}.
 
   #[local] Coercion vl_ev : vnt >-> vl.
   #[local] Coercion vl_exp : nv >-> vl.
   #[local] Coercion wvl_v : vl >-> wvl.
 
-  Lemma advance_Eval `{Name loc} `{Eq var}
-    (σ0 σ' : nv var loc _) (Σ0 : env σ0) v' t (EVAL : σ' ⊢ t ⇓ v') :
-    forall (σ : nv var loc _) (LINK : σ0 ⋊ σ ∋ σ'),
+  Lemma advance_Eval `{Eq var} `{Eq lbl} `{Name loc} 
+    (σ0 σ' : nv var lbl loc _) (Σ0 : env σ0) v' t (EVAL : σ' ⊢ t ⇓ v') :
+    forall (σ : nv var lbl loc _) (LINK : σ0 ⋊ σ ∋ σ'),
       exists v, (σ ⊢ t ⇓ v) /\ (σ0 ⋊ v ∋ v').
   Proof.
     induction EVAL; ii; ss.
-    - exploit Link_read; eauto; ss.
+    - exploit (link_read' σ0); eauto; ss.
       intro READ'. specialize (READ' x v READ).
       des; ss.
       eexists; split; eauto.
       destruct w; ss.
       + econstructor 1; auto.
       + econstructor 2; auto.
-    - exploit Link_read; eauto; ss.
-      intro READ'. specialize (READ' x (wvl_recv v) READ).
+    - exploit (link_read' σ0); eauto; ss.
+      intro READ'. specialize (READ' x (wvl_recv p' v) READ).
       des; ss.
       eexists; split; eauto.
       destruct w; ss.
@@ -43,11 +42,11 @@ Section Advance.
       intros (v1' & EVAL1' & LINK1).
       destruct v1'; try solve [inv LINK1].
       + exists (Call E v2').
-        split. eapply Ev_appevent; eauto.
+        split. eapply ev_appevent'; eauto.
         econstructor; eauto.
       + inv LINK1.
         exploit IHEVAL3; eauto.
-        eapply Link_bval; eauto.
+        eapply link_bval'; eauto.
         intros (v' & EVAL' & LINK').
         exists v'. split; try econstructor; eauto.
     - exploit IHEVAL1; eauto.
@@ -56,8 +55,8 @@ Section Advance.
       intros (v1' & EVAL1' & LINK1).
       destruct v1'; try solve [inv LINK1].
       eexists. split.
-      eapply Ev_appevent; eauto.
-      eapply Link_CallEvent; eauto.
+      eapply ev_appevent'; eauto.
+      eapply link_CallEvent'; eauto.
     - exploit IHEVAL1; eauto.
       intros (v1' & EVAL1' & LINK1).
       destruct v1'; try solve [inv LINK1].
@@ -65,114 +64,114 @@ Section Advance.
         exploit IHEVAL2.
         econstructor; eauto.
         ii; des; eexists.
-        split. eapply Ev_linkevent; eauto. auto.
+        split. eapply ev_linkevent'; eauto. auto.
       + exploit IHEVAL2; eauto; ii; des; eexists.
-        split. eapply Ev_link; eauto.
+        split. eapply ev_link'; eauto.
         auto.
     - exploit IHEVAL1; eauto.
       intros (v1' & EVAL1' & LINK1).
       destruct v1'; try solve [inv LINK1].
       specialize (IHEVAL2 (nv_ev E)).
       exploit IHEVAL2.
-      apply Link_holeEvent; auto.
+      apply link_holeEvent'; auto.
       ii; des; eexists.
-      split. eapply Ev_linkevent; eauto. auto.
+      split. eapply ev_linkevent'; eauto. auto.
     - exists nv_mt. split; econstructor; eauto.
     - gensym_tac (L ++ floc_nv σ0 ++ floc_nv σ1 ++ floc_vl v1) ν.
       match goal with
       | IH : forall _, ~ In _ ?L -> _, ν : loc, nIN : ~ In ν ?L |- _ =>
         exploit (IH ν nIN);
-        first [eapply Link_floc; eauto | idtac]
+        first [eapply link_floc'; eauto | idtac]
       end.
       intros (v1' & EVAL1 & LINK1).
-      eapply Link_lc in LINK as Σ1. inv Σ1. inv VAL.
-      eapply Eval_lc in EVAL1 as V1; try solve [econstructor; eauto].
-      assert (forall ℓ (FREE : ~ In ℓ (floc_nv σ1)),
-        open_loc_vl 0 ℓ (close_vl 0 ν v1') = subst_loc_vl ℓ ν v1') as RR.
+      eapply link_lc' in LINK as Σ1. inv Σ1. inv VAL.
+      eapply eval_lc' in EVAL1 as V1; try solve [econstructor; eauto].
+      assert (forall ℓ p' (FREE : ~ In ℓ (floc_nv σ1)),
+        open_loc_vl 0 (ℓ, p') (close_vl 0 (ν, get_lbl t1) v1') = subst_loc_vl (ℓ, p') (ν, get_lbl t1) v1') as RR.
       { intros.
-        assert (close_open_loc_eq_vl _ _ _ v1') by eapply close_open_loc_eq. rw.
-        assert (open_loc_lc_vl _ _ _ v1' V1) by (eapply open_loc_lc; eauto). rw.
+        assert (close_open_loc_eq_vl v1') by eapply close_open_loc_eq. rw.
+        assert (open_loc_lc_vl v1' V1) by (eapply open_loc_lc; eauto). rw.
         reflexivity. }
-      assert (forall ℓ (FREE : ~ In ℓ (floc_nv σ1)),
-        Eval (nv_floc x ℓ σ1) t1 (open_loc_vl 0 ℓ (close_vl 0 ν v1'))).
-      { intros. apply Eval_subst_loc with (ν := ℓ) (ℓ' := ν) in EVAL1.
-        ss. rewrite eqb_refl in EVAL1.
-        assert (RR' : subst_loc_fresh_nv _ _ _ σ1) by eapply subst_loc_fresh.
+      assert (forall ℓ p' (FREE : ~ In ℓ (floc_nv σ1)),
+        (nv_floc x (ℓ, p') σ1 ⊢ t1 ⇓ open_loc_vl 0 (ℓ, p') (close_vl 0 (ν, get_lbl t1) v1'))).
+      { intros. apply eval_subst_loc' with (ν := (ℓ, p')) (ℓ' := (ν, get_lbl t1)) in EVAL1.
+        ss. repeat rewrite eqb_refl in EVAL1. ss.
+        assert (RR' : subst_loc_fresh_nv σ1) by eapply subst_loc_fresh.
         rewrite RR' in EVAL1; eauto.
         rewrite RR; eauto. }
-      assert (forall ℓ (FREE : ~ In ℓ (floc_nv σ1)),
-        σ0 ⋊ open_loc_vl 0 ℓ (close_vl 0 ν v1') ∋ open_loc_vl 0 ℓ v1).
-      { intros. apply Link_subst_loc with (ν := ℓ) (ℓ' := ν) in LINK1; eauto.
-        assert (open_loc_subst_loc_vl _ _ _ v1) as RR' by eapply open_loc_subst_loc.
+      assert (forall ℓ p' (FREE : ~ In ℓ (floc_nv σ1)),
+        σ0 ⋊ open_loc_vl 0 (ℓ, p') (close_vl 0 (ν, get_lbl t1) v1') ∋ open_loc_vl 0 (ℓ, p') v1).
+      { intros. apply link_subst_loc' with (ν := (ℓ, p')) (ℓ' := (ν, get_lbl t1)) in LINK1; eauto.
+        assert (open_loc_subst_loc_vl v1) as RR' by eapply open_loc_subst_loc.
         simpl in LINK1. rewrite RR' in LINK1. clear RR'.
-        rewrite eqb_refl in LINK1.
+        repeat rewrite eqb_refl in LINK1. ss.
         rewrite RR; eauto.
-        assert (subst_loc_fresh_nv _ _ _ σ0) as RR' by eapply subst_loc_fresh.
+        assert (subst_loc_fresh_nv σ0) as RR' by eapply subst_loc_fresh.
         rewrite RR' in LINK1; eauto. clear RR'.
-        assert (subst_loc_fresh_vl _ _ _ v1) as RR' by eapply subst_loc_fresh.
+        assert (subst_loc_fresh_vl v1) as RR' by eapply subst_loc_fresh.
         rewrite RR' in LINK1; eauto. }
-      assert (σ0 ⋊ wvl_recv (close_vl 0 ν v1') ∋ wvl_recv v1).
+      assert (σ0 ⋊ wvl_recv (get_lbl t1) (close_vl 0 (ν, get_lbl t1) v1') ∋ wvl_recv (get_lbl t1) v1).
       { econstructor; eauto. }
-      exploit (IHEVAL (nv_bval x (wvl_recv (close_vl 0 ν v1')) σ1)).
+      exploit (IHEVAL (nv_bval x (wvl_recv (get_lbl t1) (close_vl 0 (ν, get_lbl t1) v1')) σ1)).
       + econstructor; eauto.
       + intros (v2' & EVAL2 & LINK2).
         destruct v2'; try solve [inv LINK2].
-        * exists (nv_bval x (wvl_recv (close_vl 0 ν v1')) (nv_ev E)).
-          split. eapply Ev_bindevent; eauto.
+        * exists (nv_bval x (wvl_recv (get_lbl t1) (close_vl 0 (ν, get_lbl t1) v1')) (nv_ev E)).
+          split. eapply ev_bindevent'; eauto.
           econstructor; eauto.
           econstructor; eauto.
-        * exists (nv_bval x (wvl_recv (close_vl 0 ν v1')) σ3).
+        * exists (nv_bval x (wvl_recv (get_lbl t1) (close_vl 0 (ν, get_lbl t1) v1')) σ3).
           split. econstructor; eauto.
           econstructor; eauto.
     - gensym_tac (L ++ floc_nv σ0 ++ floc_nv σ1 ++ floc_vl v1) ν.
       match goal with
       | IH : forall _, ~ In _ ?L -> _, ν : loc, nIN : ~ In ν ?L |- _ =>
         exploit (IH ν nIN);
-        first [eapply Link_floc; eauto | idtac]
+        first [eapply link_floc'; eauto | idtac]
       end.
       intros (v1' & EVAL1 & LINK1).
-      eapply Link_lc in LINK as Σ1. inv Σ1. inv VAL.
-      eapply Eval_lc in EVAL1 as V1; try solve [econstructor; eauto].
-      assert (forall ℓ (FREE : ~ In ℓ (floc_nv σ1)),
-        open_loc_vl 0 ℓ (close_vl 0 ν v1') = subst_loc_vl ℓ ν v1') as RR.
+      eapply link_lc' in LINK as Σ1. inv Σ1. inv VAL.
+      eapply eval_lc' in EVAL1 as V1; try solve [econstructor; eauto].
+      assert (forall ℓ p' (FREE : ~ In ℓ (floc_nv σ1)),
+        open_loc_vl 0 (ℓ, p') (close_vl 0 (ν, get_lbl t1) v1') = subst_loc_vl (ℓ, p') (ν, get_lbl t1) v1') as RR.
       { intros.
-        assert (close_open_loc_eq_vl _ _ _ v1') by eapply close_open_loc_eq. rw.
-        assert (open_loc_lc_vl _ _ _ v1' V1) by (eapply open_loc_lc; eauto). rw.
+        assert (close_open_loc_eq_vl v1') by eapply close_open_loc_eq. rw.
+        assert (open_loc_lc_vl v1' V1) by (eapply open_loc_lc; eauto). rw.
         reflexivity. }
-      assert (forall ℓ (FREE : ~ In ℓ (floc_nv σ1)),
-        Eval (nv_floc x ℓ σ1) t1 (open_loc_vl 0 ℓ (close_vl 0 ν v1'))).
-      { intros. apply Eval_subst_loc with (ν := ℓ) (ℓ' := ν) in EVAL1.
-        ss. rewrite eqb_refl in EVAL1.
-        assert (RR' : subst_loc_fresh_nv _ _ _ σ1) by eapply subst_loc_fresh.
+      assert (forall ℓ p' (FREE : ~ In ℓ (floc_nv σ1)),
+        (nv_floc x (ℓ, p') σ1 ⊢ t1 ⇓ open_loc_vl 0 (ℓ, p') (close_vl 0 (ν, get_lbl t1) v1'))).
+      { intros. apply eval_subst_loc' with (ν := (ℓ, p')) (ℓ' := (ν, get_lbl t1)) in EVAL1.
+        ss. repeat rewrite eqb_refl in EVAL1. ss.
+        assert (RR' : subst_loc_fresh_nv σ1) by eapply subst_loc_fresh.
         rewrite RR' in EVAL1; eauto.
         rewrite RR; eauto. }
-      assert (forall ℓ (FREE : ~ In ℓ (floc_nv σ1)),
-        σ0 ⋊ open_loc_vl 0 ℓ (close_vl 0 ν v1') ∋ open_loc_vl 0 ℓ v1).
-      { intros. apply Link_subst_loc with (ν := ℓ) (ℓ' := ν) in LINK1; eauto.
-        assert (open_loc_subst_loc_vl _ _ _ v1) as RR' by eapply open_loc_subst_loc.
+      assert (forall ℓ p' (FREE : ~ In ℓ (floc_nv σ1)),
+        σ0 ⋊ open_loc_vl 0 (ℓ, p') (close_vl 0 (ν, get_lbl t1) v1') ∋ open_loc_vl 0 (ℓ, p') v1).
+      { intros. apply link_subst_loc' with (ν := (ℓ, p')) (ℓ' := (ν, get_lbl t1)) in LINK1; eauto.
+        assert (open_loc_subst_loc_vl v1) as RR' by eapply open_loc_subst_loc.
         simpl in LINK1. rewrite RR' in LINK1. clear RR'.
-        rewrite eqb_refl in LINK1.
+        repeat rewrite eqb_refl in LINK1. ss.
         rewrite RR; eauto.
-        assert (subst_loc_fresh_nv _ _ _ σ0) as RR' by eapply subst_loc_fresh.
+        assert (subst_loc_fresh_nv σ0) as RR' by eapply subst_loc_fresh.
         rewrite RR' in LINK1; eauto. clear RR'.
-        assert (subst_loc_fresh_vl _ _ _ v1) as RR' by eapply subst_loc_fresh.
+        assert (subst_loc_fresh_vl v1) as RR' by eapply subst_loc_fresh.
         rewrite RR' in LINK1; eauto. }
-      assert (σ0 ⋊ wvl_recv (close_vl 0 ν v1') ∋ wvl_recv v1).
+      assert (σ0 ⋊ wvl_recv (get_lbl t1) (close_vl 0 (ν, get_lbl t1) v1') ∋ wvl_recv (get_lbl t1) v1).
       { econstructor; eauto. }
-      exploit (IHEVAL (nv_bval x (wvl_recv (close_vl 0 ν v1')) σ1)).
+      exploit (IHEVAL (nv_bval x (wvl_recv (get_lbl t1) (close_vl 0 (ν, get_lbl t1) v1')) σ1)).
       + econstructor; eauto.
       + intros (v2' & EVAL2 & LINK2).
         destruct v2'; try solve [inv LINK2].
-        exists (nv_bval x (wvl_recv (close_vl 0 ν v1')) (nv_ev E)).
-        split. eapply Ev_bindevent; eauto.
+        exists (nv_bval x (wvl_recv (get_lbl t1) (close_vl 0 (ν, get_lbl t1) v1')) (nv_ev E)).
+        split. eapply ev_bindevent'; eauto.
         econstructor; eauto.
-        eapply Link_holeEvent.
+        eapply link_holeEvent'.
         assumption.
   Qed.
 
-  Theorem advance `{Name loc} `{Eq var}
-    (σ0 σ' : nv var loc _) (Σ0 : env σ0) v' t (EVAL : eval σ' t v') :
-    forall (σ : nv var loc _) (LINK : link σ0 σ σ'),
+  Theorem advance `{Eq var} `{Eq lbl} `{Name loc}
+    (σ0 σ' : nv var lbl loc _) (Σ0 : env σ0) v' t (EVAL : eval σ' t v') :
+    forall (σ : nv var lbl loc _) (LINK : link σ0 σ σ'),
       exists v, eval σ t v /\ link σ0 v v'.
   Proof.
     intros.
@@ -182,7 +181,7 @@ Section Advance.
     destruct EVAL as (v & EVAL & LINK').
     erewrite <- equiv_semantics in EVAL; eauto.
     erewrite <- equiv_link in LINK'; eauto.
-    eapply Link_lc in LINK. inv LINK. inv VAL. auto.
+    eapply link_lc' in LINK. inv LINK. inv VAL. auto.
     eapply linked_lc in LINK; eauto. inv LINK. inv VAL. auto.
   Qed.
 End Advance.
