new-semantics/coq/events/LinkFacts.v
@@ -6,8 +6,7 @@ From With_events Require Import EnvSemantics.
 From With_events Require Import LinkDefs.
 
 Section LinkFacts.
-  Variable var : Type.
-  Variable loc : Type.
+  Context {var lbl loc : Type}.
 
   #[local] Coercion vl_ev : vnt >-> vl.
   #[local] Coercion vl_exp : nv >-> vl.
@@ -23,7 +22,7 @@ Section LinkFacts.
     | _ => instantiate (1 := [])
     end.
 
-  Lemma link_lc `{Eq loc} `{Eq var} (σ0 : nv var loc _) (w : wvl var loc _) :
+  Lemma link_lc `{Eq var} `{Eq lbl} `{Eq loc} (σ0 : nv var lbl loc _) (w : wvl var lbl loc _) :
     forall w' (LINK : link σ0 w w'), wvalue w.
   Proof.
     ii. induction LINK;
@@ -36,9 +35,9 @@ Section LinkFacts.
     end.
     all: try match goal with
     | V : value ?v |- value (subst_loc_vl _ _ ?v) =>
-      assert (subst_loc_lc_vl _ _ _ v V) by eapply subst_loc_lc; auto
+      assert (subst_loc_lc_vl v V) by eapply subst_loc_lc; auto
     | |- context [subst_loc_vl ?ℓ ?ν (open_loc_vl 0 ?ν ?v)] =>
-      assert (open_loc_subst_loc_vl _ _ _ v) by eapply open_loc_subst_loc;
+      assert (open_loc_subst_loc_vl v) by eapply open_loc_subst_loc;
       rw; rewrite eqb_refl;
       f_equal; eapply subst_loc_fresh; auto
     end.
@@ -54,8 +53,8 @@ Section LinkFacts.
     | _ => instantiate (1 := [])
     end.
 
-  Lemma linked_lc `{Name loc} `{Eq var}
-    (σ0 : nv var loc _) (Σ0 : env σ0) (w : wvl var loc _) :
+  Lemma linked_lc `{Eq var} `{Eq lbl} `{Name loc} 
+    (σ0 : nv var lbl loc _) (Σ0 : env σ0) (w : wvl var lbl loc _) :
     forall w' (LINK : link σ0 w w'), wvalue w'.
   Proof.
     ii. induction LINK;
@@ -63,64 +62,93 @@ Section LinkFacts.
     linked_lc_tac; ii.
     - eapply read_env_lc in READ; auto.
       destruct w; inv READ; ss.
-      assert (subst_intro_vl _ _ _ v) by eapply subst_intro.
+      assert (subst_intro_vl v) by eapply subst_intro.
       gensym_tac (L ++ floc_vl v) ℓ.
       rw; eauto.
       eapply subst_wvl_lc; eauto.
       econstructor; eauto.
     - eapply eval_lc in EVAL; eauto.
       repeat econstructor; eauto.
-    - assert (close_open_loc_eq_vl _ _ _ v') by eapply close_open_loc_eq.
+    - assert (close_open_loc_eq_vl v') by eapply close_open_loc_eq.
       rw.
-      assert (open_loc_lc_vl _ _ _ v' VAL) by (eapply open_loc_lc; eauto).
+      assert (open_loc_lc_vl v' VAL) by (eapply open_loc_lc; eauto).
       rw.
       eapply subst_loc_lc; auto.
   Qed.
 
-  Lemma map_unroll {lang} `{Eq loc} φ (w : wvl var loc lang) :
+  Lemma map_unroll {lang} `{Eq lbl} `{Eq loc} φ (w : wvl var lbl loc lang) :
     unroll (map_wvl φ w) = map_vl φ (unroll w).
   Proof.
     destruct w; ss.
-    assert (map_open_wvl_vl _ _ _ v) by eapply map_open_wvl.
+    assert (map_open_wvl_vl v) by eapply map_open_wvl.
     rw; ss.
   Qed.
 
-  Lemma subst_loc_unroll {lang} `{Eq loc}
-    ℓ ν (w : wvl var loc lang) :
+  Lemma subst_loc_unroll {lang} `{Eq lbl} `{Eq loc}
+    ℓ ν (w : wvl var lbl loc lang) :
     unroll (subst_loc_wvl ν ℓ w) = subst_loc_vl ν ℓ (unroll w).
   Proof.
     destruct w; ss.
     match goal with
     | |- context [subst_loc_vl _ _ (open_wvl_vl _ _ ?v)] =>
-      assert (open_wvl_subst_loc_vl _ _ _ v)
+      assert (open_wvl_subst_loc_vl v)
         by (eapply open_wvl_subst_loc; eauto);
       rw; ss
     end.
   Qed.
 
-  Lemma subst_wvl_unroll {lang} `{Name loc}
-    ℓ (u w : wvl var loc lang) (U : wvalue u) :
+  Lemma subst_wvl_unroll {lang} `{Eq lbl} `{Name loc}
+    ℓ (u w : wvl var lbl loc lang) (U : wvalue u) :
     unroll (subst_wvl_wvl u ℓ w) = subst_wvl_vl u ℓ (unroll w).
   Proof.
     destruct w; ss.
     match goal with
     | |- context [subst_wvl_vl _ _ (open_wvl_vl _ _ ?v)] =>
-      assert (open_wvl_subst_wvl_vl _ _ _ v)
+      assert (open_wvl_subst_wvl_vl v)
         by (eapply open_wvl_subst_wvl; eauto);
       rw; ss
     end.
   Qed.
 
-  Lemma unroll_floc {lang} ℓ (w : wvl var loc lang) :
-    In ℓ (floc_wvl w) <-> In ℓ (floc_vl (unroll w)).
+  Lemma unroll_flloc {lang} ℓ (w : wvl var lbl loc lang) :
+    In ℓ (flloc_wvl w) <-> In ℓ (flloc_vl (unroll w)).
   Proof.
     split; intro IN; destruct w; ss.
-    - eapply open_wvl_inc_floc. auto.
-    - eapply open_wvl_floc in IN. ss; des; auto.
+    - eapply open_wvl_inc_flloc. auto.
+    - eapply open_wvl_flloc in IN. des; auto.
   Qed.
 
-  Lemma link_map `{Name loc} `{Eq var}
-    (σ0 : nv var loc _) (w w' : wvl var loc _) (LINK : link σ0 w w') :
+  Lemma link_flloc_dec `{Eq var} `{Eq lbl} `{Eq loc}
+    (σ0 : nv var lbl loc _) (w w' : wvl var lbl loc _) (LINK : link σ0 w w') :
+    forall ℓ (IN : In ℓ (flloc_wvl w')), In ℓ (flloc_nv σ0) \/ In ℓ (flloc_wvl w).
+  Proof.
+    induction LINK; ii; ss;
+    repeat rewrite in_app_iff in *; eauto.
+    - rewrite <- unroll_flloc in IN.
+      eapply read_env_flloc in READ; eauto.
+    - eapply eval_flloc_dec in EVAL; eauto; ss.
+      rewrite in_app_iff in EVAL; des.
+      + exploit IHLINK2; ii; des; eauto.
+      + exploit IHLINK1; ii; des; eauto.
+    - des.
+      exploit IHLINK1; ii; des; eauto.
+      exploit IHLINK2; ii; des; eauto.
+    - des; clarify. auto.
+      exploit IHLINK; ii; des; eauto.
+    - des.
+      exploit IHLINK1; ii; des; eauto.
+      exploit IHLINK2; ii; des; eauto.
+    - eapply close_flloc in IN. destruct IN as [nEQ IN].
+      exploit IHLINK; ii; des; eauto.
+      match goal with
+      | H : In ?ℓ (flloc_vl (open_loc_vl _ _ _)) |- _ =>
+        eapply open_loc_flloc in H; des; clarify
+      end.
+      eauto.
+  Qed.
+
+  Lemma link_map `{Eq var} `{Eq lbl} `{Name loc}
+    (σ0 : nv var lbl loc _) (w w' : wvl var lbl loc _) (LINK : link σ0 w w') :
     forall φ (INJ : oto φ),
       link (map_nv φ σ0) (map_wvl φ w) (map_wvl φ w').
   Proof.
@@ -133,7 +161,8 @@ Section LinkFacts.
       specialize (IHLINK2 φ INJ).
       eapply link_CallEval; eauto.
       eapply eval_map with (φ := φ) in EVAL; eauto.
-    - assert (map_close_vl _ _ _ v') by (eapply map_close; eauto).
+    - des_goal; ss; econstructor; eauto.
+    - assert (map_close_vl v') by (eapply map_close; eauto).
       rw; eauto.
       econstructor; eauto;
       match goal with
@@ -141,7 +170,7 @@ Section LinkFacts.
         intro IN; eapply map_floc in IN; eauto
       | _ =>
         specialize (IHLINK φ INJ);
-        assert (map_open_loc_vl _ _ _ v) as RR by (eapply map_open_loc; eauto);
+        assert (map_open_loc_vl v) as RR by (eapply map_open_loc; eauto);
         rewrite RR in *; auto
       end.
   Qed.
